\documentclass[fleqn,8pt,landscape]{jsarticle}
\special{papersize=\the\paperwidth,\the\paperheight}

%%% package

\usepackage[usenames]{color}
\usepackage{amsmath}
\usepackage{breqn}
\usepackage{graphicx}
\usepackage{amssymb}
\usepackage{bm}
\usepackage{enumitem}
\usepackage{braket}
\usepackage{multirow}
\usepackage{booktabs}
\usepackage{longtable}

%%% layout setting

\paperwidth=356.4truemm
\paperheight=252.0truemm
\textwidth=335.59999999999997truemm
\textheight=224.2truemm
\oddsidemargin=-15truemm
\topmargin=-15truemm
\footskip=7truemm

%%% fixed

\hoffset=0truemm
\voffset=0truemm
\headheight=0truemm
\headsep=0truemm
\marginparsep=0truemm
\marginparwidth=0truemm

%%% main text

\begin{document}

\setcounter{MaxMatrixCols}{32}

\renewcommand{\tablename}{Table~}
\renewcommand{\figurename}{Figure~}
\begin{center}
\LARGE
MPG No. 21.1.76\quad$6$\quad[ Type I, hexagonal ] [M tensor]
\end{center}
* Rank 0 tensor.
\begin{align*}
\begin{bmatrix} M \end{bmatrix}
\end{align*}
\begin{align*}
& M = M_{s}^{(1)}
\end{align*}
* Rank 1 tensor.
\begin{align*}
\begin{bmatrix} 0 & 0 & M_{z} \end{bmatrix}
\end{align*}
\begin{align*}
& M_{z} = M_{pz}^{(1)}
\end{align*}
* Rank 2 tensor (s).
\begin{align*}
\begin{bmatrix} M_{xx} & 0 & 0 \\ 0 & M_{xx} & 0 \\ 0 & 0 & M_{zz} \end{bmatrix}
\end{align*}
\begin{align*}
& M_{xx} = - M_{du}^{(1)} + M_{s}^{(1)} \\
& M_{zz} = 2 M_{du}^{(1)} + M_{s}^{(1)}
\end{align*}
* Rank 2 tensor (a).
\begin{align*}
\begin{bmatrix} 0 & M_{xy} & 0 \\ - M_{xy} & 0 & 0 \\ 0 & 0 & 0 \end{bmatrix}
\end{align*}
\begin{align*}
& M_{xy} = T_{pz}^{(1)}
\end{align*}
* Rank 3 tensor (s).
\begin{align*}
\begin{bmatrix} 0 & 0 & M_{xxz} \\ 0 & 0 & M_{xxz} \\ 0 & 0 & M_{zzz} \\ M_{yzx} & M_{yzy} & 0 \\ M_{yzy} & - M_{yzx} & 0 \\ 0 & 0 & 0 \end{bmatrix}
\end{align*}
\begin{align*}
& M_{xxz} = - M_{faz}^{(1)} + M_{pz}^{(1)} \\
& M_{zzz} = 2 M_{faz}^{(1)} + M_{pz}^{(1)} + 2 M_{pz}^{(2)} \\
& M_{yzx} = - 3 T_{du}^{(1)} \\
& M_{yzy} = - M_{faz}^{(1)} + M_{pz}^{(2)}
\end{align*}
* Rank 3 tensor (a).
\begin{align*}
\begin{bmatrix} M_{yzx} & M_{yzy} & 0 \\ - M_{yzy} & M_{yzx} & 0 \\ 0 & 0 & M_{xyz} \end{bmatrix}
\end{align*}
\begin{align*}
& M_{yzx} = - T_{du}^{(2)} + T_{s}^{(1)} \\
& M_{yzy} = M_{pz}^{(3)} \\
& M_{xyz} = 2 T_{du}^{(2)} + T_{s}^{(1)}
\end{align*}
* Rank 4 tensor (sss).
\begin{align*}
\begin{bmatrix} M_{xxxx} & M_{xxyy} & M_{xxzz} & 0 & 0 & 0 \\ M_{xxyy} & M_{xxxx} & M_{xxzz} & 0 & 0 & 0 \\ M_{xxzz} & M_{xxzz} & M_{zzzz} & 0 & 0 & 0 \\ 0 & 0 & 0 & M_{yzyz} & 0 & 0 \\ 0 & 0 & 0 & 0 & M_{yzyz} & 0 \\ 0 & 0 & 0 & 0 & 0 & \frac{M_{xxxx}}{2} - \frac{M_{xxyy}}{2} \end{bmatrix}
\end{align*}
\begin{align*}
& M_{xxxx} = - 2 M_{du}^{(1)} - 4 M_{du}^{(2)} + 3 M_{g0}^{(1)} + M_{s}^{(1)} + 2 M_{s}^{(2)} \\
& M_{xxyy} = - 2 M_{du}^{(1)} + M_{g0}^{(1)} + M_{s}^{(1)} \\
& M_{xxzz} = M_{du}^{(1)} - 4 M_{g0}^{(1)} + M_{s}^{(1)} \\
& M_{zzzz} = 4 M_{du}^{(1)} + 8 M_{du}^{(2)} + 8 M_{g0}^{(1)} + M_{s}^{(1)} + 2 M_{s}^{(2)} \\
& M_{yzyz} = M_{du}^{(2)} - 4 M_{g0}^{(1)} + M_{s}^{(2)}
\end{align*}
* Rank 4 tensor (ssa).
\begin{align*}
\begin{bmatrix} 0 & 0 & M_{xxzz} & 0 & 0 & M_{xxxy} \\ 0 & 0 & M_{xxzz} & 0 & 0 & - M_{xxxy} \\ - M_{xxzz} & - M_{xxzz} & 0 & 0 & 0 & 0 \\ 0 & 0 & 0 & 0 & M_{yzzx} & 0 \\ 0 & 0 & 0 & - M_{yzzx} & 0 & 0 \\ - M_{xxxy} & M_{xxxy} & 0 & 0 & 0 & 0 \end{bmatrix}
\end{align*}
\begin{align*}
& M_{xxzz} = 3 M_{du}^{(3)} \\
& M_{xxxy} = - 2 T_{faz}^{(1)} + 2 T_{pz}^{(1)} \\
& M_{yzzx} = - 4 T_{faz}^{(1)} - T_{pz}^{(1)}
\end{align*}
* Rank 4 tensor (aas).
\begin{align*}
\begin{bmatrix} M_{yzyz} & 0 & 0 \\ 0 & M_{yzyz} & 0 \\ 0 & 0 & M_{xyxy} \end{bmatrix}
\end{align*}
\begin{align*}
& M_{yzyz} = - 2 M_{du}^{(4)} + M_{s}^{(3)} \\
& M_{xyxy} = 4 M_{du}^{(4)} + M_{s}^{(3)}
\end{align*}
* Rank 4 tensor (aaa).
\begin{align*}
\begin{bmatrix} 0 & M_{yzzx} & 0 \\ - M_{yzzx} & 0 & 0 \\ 0 & 0 & 0 \end{bmatrix}
\end{align*}
\begin{align*}
& M_{yzzx} = - T_{pz}^{(2)}
\end{align*}
* Rank 4 tensor (sa).
\begin{align*}
\begin{bmatrix} 0 & 0 & M_{xxxy} \\ 0 & 0 & M_{xxxy} \\ 0 & 0 & M_{zzxy} \\ M_{yzyz} & M_{yzzx} & 0 \\ M_{yzzx} & - M_{yzyz} & 0 \\ 0 & 0 & 0 \end{bmatrix}
\end{align*}
\begin{align*}
& M_{xxxy} = - T_{faz}^{(2)} + T_{pz}^{(3)} \\
& M_{zzxy} = 2 T_{faz}^{(2)} + T_{pz}^{(3)} + 2 T_{pz}^{(4)} \\
& M_{yzyz} = - 3 M_{du}^{(5)} \\
& M_{yzzx} = - T_{faz}^{(2)} + T_{pz}^{(4)}
\end{align*}
* Rank 4 tensor (as).
\begin{align*}
\begin{bmatrix} 0 & 0 & 0 & M_{yzyz} & M_{yzzx} & 0 \\ 0 & 0 & 0 & M_{yzzx} & - M_{yzyz} & 0 \\ M_{xyxx} & M_{xyxx} & M_{xyzz} & 0 & 0 & 0 \end{bmatrix}
\end{align*}
\begin{align*}
& M_{yzyz} = - 3 M_{du}^{(6)} \\
& M_{yzzx} = - T_{faz}^{(3)} + T_{pz}^{(6)} \\
& M_{xyxx} = - T_{faz}^{(3)} + T_{pz}^{(5)} \\
& M_{xyzz} = 2 T_{faz}^{(3)} + T_{pz}^{(5)} + 2 T_{pz}^{(6)}
\end{align*}
* Rank 4 tensor (s).
\begin{align*}
\begin{bmatrix} M_{xxxx} & M_{xxyy} & M_{xxzz} & 0 & 0 & M_{xxxy} & 0 & 0 & M_{xxyx} \\ M_{xxyy} & M_{xxxx} & M_{xxzz} & 0 & 0 & - M_{xxyx} & 0 & 0 & - M_{xxxy} \\ M_{zzxx} & M_{zzxx} & M_{zzzz} & 0 & 0 & M_{zzxy} & 0 & 0 & - M_{zzxy} \\ 0 & 0 & 0 & M_{yzyz} & M_{yzzx} & 0 & M_{yzzy} & M_{yzxz} & 0 \\ 0 & 0 & 0 & - M_{yzxz} & M_{yzzy} & 0 & - M_{yzzx} & M_{yzyz} & 0 \\ - \frac{M_{xxxy}}{2} - \frac{M_{xxyx}}{2} & \frac{M_{xxxy}}{2} + \frac{M_{xxyx}}{2} & 0 & 0 & 0 & \frac{M_{xxxx}}{2} - \frac{M_{xxyy}}{2} & 0 & 0 & \frac{M_{xxxx}}{2} - \frac{M_{xxyy}}{2} \end{bmatrix}
\end{align*}
\begin{align*}
& M_{xxxx} = - 2 M_{du}^{(1)} - 4 M_{du}^{(2)} + 3 M_{g0}^{(1)} + M_{s}^{(1)} + 2 M_{s}^{(2)} \\
& M_{xxyy} = - 2 M_{du}^{(1)} + M_{g0}^{(1)} + M_{s}^{(1)} \\
& M_{xxzz} = M_{du}^{(1)} + 3 M_{du}^{(3)} - 4 M_{g0}^{(1)} + M_{s}^{(1)} \\
& M_{xxxy} = - 2 T_{faz}^{(1)} - T_{faz}^{(2)} + 2 T_{pz}^{(1)} + T_{pz}^{(3)} \\
& M_{xxyx} = - 2 T_{faz}^{(1)} + T_{faz}^{(2)} + 2 T_{pz}^{(1)} - T_{pz}^{(3)} \\
& M_{zzxx} = M_{du}^{(1)} - 3 M_{du}^{(3)} - 4 M_{g0}^{(1)} + M_{s}^{(1)} \\
& M_{zzzz} = 4 M_{du}^{(1)} + 8 M_{du}^{(2)} + 8 M_{g0}^{(1)} + M_{s}^{(1)} + 2 M_{s}^{(2)} \\
& M_{zzxy} = 2 T_{faz}^{(2)} + T_{pz}^{(3)} + 2 T_{pz}^{(4)} \\
& M_{yzyz} = M_{du}^{(2)} - 3 M_{du}^{(5)} - 4 M_{g0}^{(1)} + M_{s}^{(2)} \\
& M_{yzzx} = - 4 T_{faz}^{(1)} - T_{faz}^{(2)} - T_{pz}^{(1)} + T_{pz}^{(4)} \\
& M_{yzzy} = M_{du}^{(2)} + 3 M_{du}^{(5)} - 4 M_{g0}^{(1)} + M_{s}^{(2)} \\
& M_{yzxz} = - 4 T_{faz}^{(1)} + T_{faz}^{(2)} - T_{pz}^{(1)} - T_{pz}^{(4)}
\end{align*}
* Rank 4 tensor (a).
\begin{align*}
\begin{bmatrix} 0 & 0 & 0 & M_{yzyz} & M_{yzzx} & 0 & M_{yzzy} & M_{yzxz} & 0 \\ 0 & 0 & 0 & M_{yzxz} & - M_{yzzy} & 0 & M_{yzzx} & - M_{yzyz} & 0 \\ M_{xyxx} & M_{xyxx} & M_{xyzz} & 0 & 0 & M_{xyxy} & 0 & 0 & - M_{xyxy} \end{bmatrix}
\end{align*}
\begin{align*}
& M_{yzyz} = - 2 M_{du}^{(4)} - 3 M_{du}^{(6)} + M_{s}^{(3)} \\
& M_{yzzx} = - T_{faz}^{(3)} - T_{pz}^{(2)} + T_{pz}^{(6)} \\
& M_{yzzy} = 2 M_{du}^{(4)} - 3 M_{du}^{(6)} - M_{s}^{(3)} \\
& M_{yzxz} = - T_{faz}^{(3)} + T_{pz}^{(2)} + T_{pz}^{(6)} \\
& M_{xyxx} = - T_{faz}^{(3)} + T_{pz}^{(5)} \\
& M_{xyzz} = 2 T_{faz}^{(3)} + T_{pz}^{(5)} + 2 T_{pz}^{(6)} \\
& M_{xyxy} = 4 M_{du}^{(4)} + M_{s}^{(3)}
\end{align*}
* Rank 4 tensor (t).
\begin{align*}
\begin{bmatrix} M_{xxxx} & 0 & 0 \\ 0 & M_{xxxx} & 0 \\ 0 & 0 & M_{zzzz} \\ 0 & 0 & M_{yyzz} \\ M_{zzxx} & 0 & 0 \\ 0 & M_{xxyy} & 0 \\ 0 & M_{yzzy} & 0 \\ 0 & 0 & - \frac{M_{xxxx}}{2} + \frac{3 M_{xxyy}}{2} + M_{yyzz} - M_{yzzy} + M_{zzxx} \\ \frac{M_{xxxx}}{2} - \frac{M_{xxyy}}{2} & 0 & 0 \\ 0 & 0 & 0 \end{bmatrix}
\end{align*}
\begin{align*}
& M_{xxxx} = - 2 M_{du}^{(1)} - 4 M_{du}^{(2)} + 3 M_{g0}^{(1)} + 3 M_{s}^{(1)} \\
& M_{zzzz} = 4 M_{du}^{(1)} + 8 M_{du}^{(2)} + 8 M_{g0}^{(1)} + 3 M_{s}^{(1)} \\
& M_{yyzz} = M_{du}^{(1)} + 3 M_{du}^{(3)} - 4 M_{g0}^{(1)} + M_{s}^{(1)} \\
& M_{zzxx} = M_{du}^{(1)} - 3 M_{du}^{(3)} - 4 M_{g0}^{(1)} + M_{s}^{(1)} \\
& M_{xxyy} = - 2 M_{du}^{(1)} + M_{g0}^{(1)} + M_{s}^{(1)} \\
& M_{yzzy} = M_{du}^{(2)} + 3 M_{du}^{(5)} - 4 M_{g0}^{(1)} + M_{s}^{(1)}
\end{align*}

\end{document}
