\documentclass[fleqn,8pt,landscape]{jsarticle}
\special{papersize=\the\paperwidth,\the\paperheight}

%%% package

\usepackage[usenames]{color}
\usepackage{amsmath}
\usepackage{breqn}
\usepackage{graphicx}
\usepackage{amssymb}
\usepackage{bm}
\usepackage{enumitem}
\usepackage{braket}
\usepackage{multirow}
\usepackage{booktabs}
\usepackage{longtable}

%%% layout setting

\paperwidth=356.4truemm
\paperheight=252.0truemm
\textwidth=335.59999999999997truemm
\textheight=224.2truemm
\oddsidemargin=-15truemm
\topmargin=-15truemm
\footskip=7truemm

%%% fixed

\hoffset=0truemm
\voffset=0truemm
\headheight=0truemm
\headsep=0truemm
\marginparsep=0truemm
\marginparwidth=0truemm

%%% main text

\begin{document}

\setcounter{MaxMatrixCols}{32}

\renewcommand{\tablename}{Table~}
\renewcommand{\figurename}{Figure~}
\begin{center}
\LARGE
MPG No. 28.2.108\quad$231'$\quad[ Type II, cubic ] [G tensor]
\end{center}
* Rank 0 tensor.
\begin{align*}
\begin{bmatrix} G \end{bmatrix}
\end{align*}
\begin{align*}
& G = G_{s}^{(1)}
\end{align*}
* Rank 1 tensor.
* Rank 2 tensor (s).
\begin{align*}
\begin{bmatrix} G_{xx} & 0 & 0 \\ 0 & G_{xx} & 0 \\ 0 & 0 & G_{xx} \end{bmatrix}
\end{align*}
\begin{align*}
& G_{xx} = G_{s}^{(1)}
\end{align*}
* Rank 2 tensor (a).
* Rank 3 tensor (s).
\begin{align*}
\begin{bmatrix} 0 & 0 & 0 \\ 0 & 0 & 0 \\ 0 & 0 & 0 \\ G_{yzx} & 0 & 0 \\ 0 & G_{yzx} & 0 \\ 0 & 0 & G_{yzx} \end{bmatrix}
\end{align*}
\begin{align*}
& G_{yzx} = G_{f3}^{(1)}
\end{align*}
* Rank 3 tensor (a).
\begin{align*}
\begin{bmatrix} G_{yzx} & 0 & 0 \\ 0 & G_{yzx} & 0 \\ 0 & 0 & G_{yzx} \end{bmatrix}
\end{align*}
\begin{align*}
& G_{yzx} = Q_{s}^{(1)}
\end{align*}
* Rank 4 tensor (sss).
\begin{align*}
\begin{bmatrix} G_{xxxx} & G_{xxyy} & G_{xxyy} & 0 & 0 & 0 \\ G_{xxyy} & G_{xxxx} & G_{xxyy} & 0 & 0 & 0 \\ G_{xxyy} & G_{xxyy} & G_{xxxx} & 0 & 0 & 0 \\ 0 & 0 & 0 & G_{yzyz} & 0 & 0 \\ 0 & 0 & 0 & 0 & G_{yzyz} & 0 \\ 0 & 0 & 0 & 0 & 0 & G_{yzyz} \end{bmatrix}
\end{align*}
\begin{align*}
& G_{xxxx} = 2 G_{g}^{(1)} + G_{s}^{(1)} + 2 G_{s}^{(2)} \\
& G_{xxyy} = - G_{g}^{(1)} + G_{s}^{(1)} \\
& G_{yzyz} = - G_{g}^{(1)} + G_{s}^{(2)}
\end{align*}
* Rank 4 tensor (ssa).
\begin{align*}
\begin{bmatrix} 0 & G_{xxyy} & - G_{xxyy} & 0 & 0 & 0 \\ - G_{xxyy} & 0 & G_{xxyy} & 0 & 0 & 0 \\ G_{xxyy} & - G_{xxyy} & 0 & 0 & 0 & 0 \\ 0 & 0 & 0 & 0 & 0 & 0 \\ 0 & 0 & 0 & 0 & 0 & 0 \\ 0 & 0 & 0 & 0 & 0 & 0 \end{bmatrix}
\end{align*}
\begin{align*}
& G_{xxyy} = 4 Q_{f3}^{(1)}
\end{align*}
* Rank 4 tensor (aas).
\begin{align*}
\begin{bmatrix} G_{yzyz} & 0 & 0 \\ 0 & G_{yzyz} & 0 \\ 0 & 0 & G_{yzyz} \end{bmatrix}
\end{align*}
\begin{align*}
& G_{yzyz} = G_{s}^{(3)}
\end{align*}
* Rank 4 tensor (aaa).
* Rank 4 tensor (sa).
\begin{align*}
\begin{bmatrix} 0 & 0 & 0 \\ 0 & 0 & 0 \\ 0 & 0 & 0 \\ G_{yzyz} & 0 & 0 \\ 0 & G_{yzyz} & 0 \\ 0 & 0 & G_{yzyz} \end{bmatrix}
\end{align*}
\begin{align*}
& G_{yzyz} = Q_{f3}^{(2)}
\end{align*}
* Rank 4 tensor (as).
\begin{align*}
\begin{bmatrix} 0 & 0 & 0 & G_{yzyz} & 0 & 0 \\ 0 & 0 & 0 & 0 & G_{yzyz} & 0 \\ 0 & 0 & 0 & 0 & 0 & G_{yzyz} \end{bmatrix}
\end{align*}
\begin{align*}
& G_{yzyz} = Q_{f3}^{(3)}
\end{align*}
* Rank 4 tensor (s).
\begin{align*}
\begin{bmatrix} G_{xxxx} & G_{xxyy} & G_{xxzz} & 0 & 0 & 0 & 0 & 0 & 0 \\ G_{xxzz} & G_{xxxx} & G_{xxyy} & 0 & 0 & 0 & 0 & 0 & 0 \\ G_{xxyy} & G_{xxzz} & G_{xxxx} & 0 & 0 & 0 & 0 & 0 & 0 \\ 0 & 0 & 0 & G_{yzyz} & 0 & 0 & G_{yzzy} & 0 & 0 \\ 0 & 0 & 0 & 0 & G_{yzyz} & 0 & 0 & G_{yzzy} & 0 \\ 0 & 0 & 0 & 0 & 0 & G_{yzyz} & 0 & 0 & G_{yzzy} \end{bmatrix}
\end{align*}
\begin{align*}
& G_{xxxx} = 2 G_{g}^{(1)} + G_{s}^{(1)} + 2 G_{s}^{(2)} \\
& G_{xxyy} = - G_{g}^{(1)} + G_{s}^{(1)} + 4 Q_{f3}^{(1)} \\
& G_{xxzz} = - G_{g}^{(1)} + G_{s}^{(1)} - 4 Q_{f3}^{(1)} \\
& G_{yzyz} = - G_{g}^{(1)} + G_{s}^{(2)} + Q_{f3}^{(2)} \\
& G_{yzzy} = - G_{g}^{(1)} + G_{s}^{(2)} - Q_{f3}^{(2)}
\end{align*}
* Rank 4 tensor (a).
\begin{align*}
\begin{bmatrix} 0 & 0 & 0 & G_{yzyz} & 0 & 0 & G_{yzzy} & 0 & 0 \\ 0 & 0 & 0 & 0 & G_{yzyz} & 0 & 0 & G_{yzzy} & 0 \\ 0 & 0 & 0 & 0 & 0 & G_{yzyz} & 0 & 0 & G_{yzzy} \end{bmatrix}
\end{align*}
\begin{align*}
& G_{yzyz} = G_{s}^{(3)} + Q_{f3}^{(3)} \\
& G_{yzzy} = - G_{s}^{(3)} + Q_{f3}^{(3)}
\end{align*}
* Rank 4 tensor (t).
\begin{align*}
\begin{bmatrix} G_{xxxx} & 0 & 0 \\ 0 & G_{xxxx} & 0 \\ 0 & 0 & G_{xxxx} \\ 0 & 0 & G_{yyzz} \\ G_{yyzz} & 0 & 0 \\ 0 & G_{yyzz} & 0 \\ 0 & G_{yyzz} & 0 \\ 0 & 0 & G_{yyzz} \\ G_{yyzz} & 0 & 0 \\ 0 & 0 & 0 \end{bmatrix}
\end{align*}
\begin{align*}
& G_{xxxx} = 2 G_{g}^{(1)} + 3 G_{s}^{(1)} \\
& G_{yyzz} = - G_{g}^{(1)} + G_{s}^{(1)}
\end{align*}

\end{document}
