\documentclass[fleqn,8pt,landscape]{jsarticle}
\special{papersize=\the\paperwidth,\the\paperheight}

%%% package

\usepackage[usenames]{color}
\usepackage{amsmath}
\usepackage{breqn}
\usepackage{graphicx}
\usepackage{amssymb}
\usepackage{bm}
\usepackage{enumitem}
\usepackage{braket}
\usepackage{multirow}
\usepackage{booktabs}
\usepackage{longtable}

%%% layout setting

\paperwidth=356.4truemm
\paperheight=252.0truemm
\textwidth=335.59999999999997truemm
\textheight=224.2truemm
\oddsidemargin=-15truemm
\topmargin=-15truemm
\footskip=7truemm

%%% fixed

\hoffset=0truemm
\voffset=0truemm
\headheight=0truemm
\headsep=0truemm
\marginparsep=0truemm
\marginparwidth=0truemm

%%% main text

\begin{document}

\setcounter{MaxMatrixCols}{32}

\renewcommand{\tablename}{Table~}
\renewcommand{\figurename}{Figure~}
\begin{center}
\LARGE
MPG No. 6.3.19\quad$2'2'2$\quad(2'2'2 setting)\quad[ Type III, orthorhombic ] [G tensor]
\end{center}
* Rank 0 tensor.
\begin{align*}
\begin{bmatrix} G \end{bmatrix}
\end{align*}
\begin{align*}
& G = G_{s}^{(1)}
\end{align*}
* Rank 1 tensor.
* Rank 2 tensor (s).
\begin{align*}
\begin{bmatrix} G_{xx} & 0 & 0 \\ 0 & G_{yy} & 0 \\ 0 & 0 & G_{zz} \end{bmatrix}
\end{align*}
\begin{align*}
& G_{xx} = - G_{du}^{(1)} + G_{dv}^{(1)} + G_{s}^{(1)} \\
& G_{yy} = - G_{du}^{(1)} - G_{dv}^{(1)} + G_{s}^{(1)} \\
& G_{zz} = 2 G_{du}^{(1)} + G_{s}^{(1)}
\end{align*}
* Rank 2 tensor (a).
* Rank 3 tensor (s).
\begin{align*}
\begin{bmatrix} 0 & 0 & 0 \\ 0 & 0 & 0 \\ 0 & 0 & 0 \\ G_{yzx} & 0 & 0 \\ 0 & G_{zxy} & 0 \\ 0 & 0 & G_{xyz} \end{bmatrix}
\end{align*}
\begin{align*}
& G_{yzx} = G_{f3}^{(1)} - 3 Q_{du}^{(1)} - Q_{dv}^{(1)} \\
& G_{zxy} = G_{f3}^{(1)} + 3 Q_{du}^{(1)} - Q_{dv}^{(1)} \\
& G_{xyz} = G_{f3}^{(1)} + 2 Q_{dv}^{(1)}
\end{align*}
* Rank 3 tensor (a).
\begin{align*}
\begin{bmatrix} G_{yzx} & 0 & 0 \\ 0 & G_{zxy} & 0 \\ 0 & 0 & G_{xyz} \end{bmatrix}
\end{align*}
\begin{align*}
& G_{yzx} = - Q_{du}^{(2)} + Q_{dv}^{(2)} + Q_{s}^{(1)} \\
& G_{zxy} = - Q_{du}^{(2)} - Q_{dv}^{(2)} + Q_{s}^{(1)} \\
& G_{xyz} = 2 Q_{du}^{(2)} + Q_{s}^{(1)}
\end{align*}
* Rank 4 tensor (sss).
\begin{align*}
\begin{bmatrix} G_{xxxx} & G_{xxyy} & G_{xxzz} & 0 & 0 & 0 \\ G_{xxyy} & G_{yyyy} & G_{yyzz} & 0 & 0 & 0 \\ G_{xxzz} & G_{yyzz} & G_{zzzz} & 0 & 0 & 0 \\ 0 & 0 & 0 & G_{yzyz} & 0 & 0 \\ 0 & 0 & 0 & 0 & G_{zxzx} & 0 \\ 0 & 0 & 0 & 0 & 0 & G_{xyxy} \end{bmatrix}
\end{align*}
\begin{align*}
& G_{xxxx} = - 2 G_{du}^{(1)} - 4 G_{du}^{(2)} + 2 G_{dv}^{(1)} + 4 G_{dv}^{(2)} - G_{gu}^{(1)} + G_{gv}^{(1)} + 2 G_{g}^{(1)} + G_{s}^{(1)} + 2 G_{s}^{(2)} \\
& G_{xxyy} = - 2 G_{du}^{(1)} + 2 G_{gu}^{(1)} - G_{g}^{(1)} + G_{s}^{(1)} \\
& G_{xxzz} = G_{du}^{(1)} + G_{dv}^{(1)} - G_{gu}^{(1)} - G_{gv}^{(1)} - G_{g}^{(1)} + G_{s}^{(1)} \\
& G_{yyyy} = - 2 G_{du}^{(1)} - 4 G_{du}^{(2)} - 2 G_{dv}^{(1)} - 4 G_{dv}^{(2)} - G_{gu}^{(1)} - G_{gv}^{(1)} + 2 G_{g}^{(1)} + G_{s}^{(1)} + 2 G_{s}^{(2)} \\
& G_{yyzz} = G_{du}^{(1)} - G_{dv}^{(1)} - G_{gu}^{(1)} + G_{gv}^{(1)} - G_{g}^{(1)} + G_{s}^{(1)} \\
& G_{zzzz} = 4 G_{du}^{(1)} + 8 G_{du}^{(2)} + 2 G_{gu}^{(1)} + 2 G_{g}^{(1)} + G_{s}^{(1)} + 2 G_{s}^{(2)} \\
& G_{yzyz} = G_{du}^{(2)} - G_{dv}^{(2)} - G_{gu}^{(1)} + G_{gv}^{(1)} - G_{g}^{(1)} + G_{s}^{(2)} \\
& G_{zxzx} = G_{du}^{(2)} + G_{dv}^{(2)} - G_{gu}^{(1)} - G_{gv}^{(1)} - G_{g}^{(1)} + G_{s}^{(2)} \\
& G_{xyxy} = - 2 G_{du}^{(2)} + 2 G_{gu}^{(1)} - G_{g}^{(1)} + G_{s}^{(2)}
\end{align*}
* Rank 4 tensor (ssa).
\begin{align*}
\begin{bmatrix} 0 & G_{xxyy} & G_{xxzz} & 0 & 0 & 0 \\ - G_{xxyy} & 0 & G_{yyzz} & 0 & 0 & 0 \\ - G_{xxzz} & - G_{yyzz} & 0 & 0 & 0 & 0 \\ 0 & 0 & 0 & 0 & 0 & 0 \\ 0 & 0 & 0 & 0 & 0 & 0 \\ 0 & 0 & 0 & 0 & 0 & 0 \end{bmatrix}
\end{align*}
\begin{align*}
& G_{xxyy} = - 2 G_{dv}^{(3)} + 4 Q_{f3}^{(1)} \\
& G_{xxzz} = 3 G_{du}^{(3)} - G_{dv}^{(3)} - 4 Q_{f3}^{(1)} \\
& G_{yyzz} = 3 G_{du}^{(3)} + G_{dv}^{(3)} + 4 Q_{f3}^{(1)}
\end{align*}
* Rank 4 tensor (aas).
\begin{align*}
\begin{bmatrix} G_{yzyz} & 0 & 0 \\ 0 & G_{zxzx} & 0 \\ 0 & 0 & G_{xyxy} \end{bmatrix}
\end{align*}
\begin{align*}
& G_{yzyz} = - 2 G_{du}^{(4)} + 2 G_{dv}^{(4)} + G_{s}^{(3)} \\
& G_{zxzx} = - 2 G_{du}^{(4)} - 2 G_{dv}^{(4)} + G_{s}^{(3)} \\
& G_{xyxy} = 4 G_{du}^{(4)} + G_{s}^{(3)}
\end{align*}
* Rank 4 tensor (aaa).
* Rank 4 tensor (sa).
\begin{align*}
\begin{bmatrix} 0 & 0 & 0 \\ 0 & 0 & 0 \\ 0 & 0 & 0 \\ G_{yzyz} & 0 & 0 \\ 0 & G_{zxzx} & 0 \\ 0 & 0 & G_{xyxy} \end{bmatrix}
\end{align*}
\begin{align*}
& G_{yzyz} = - 3 G_{du}^{(5)} - G_{dv}^{(5)} + Q_{f3}^{(2)} \\
& G_{zxzx} = 3 G_{du}^{(5)} - G_{dv}^{(5)} + Q_{f3}^{(2)} \\
& G_{xyxy} = 2 G_{dv}^{(5)} + Q_{f3}^{(2)}
\end{align*}
* Rank 4 tensor (as).
\begin{align*}
\begin{bmatrix} 0 & 0 & 0 & G_{yzyz} & 0 & 0 \\ 0 & 0 & 0 & 0 & G_{zxzx} & 0 \\ 0 & 0 & 0 & 0 & 0 & G_{xyxy} \end{bmatrix}
\end{align*}
\begin{align*}
& G_{yzyz} = - 3 G_{du}^{(6)} - G_{dv}^{(6)} + Q_{f3}^{(3)} \\
& G_{zxzx} = 3 G_{du}^{(6)} - G_{dv}^{(6)} + Q_{f3}^{(3)} \\
& G_{xyxy} = 2 G_{dv}^{(6)} + Q_{f3}^{(3)}
\end{align*}
* Rank 4 tensor (s).
\begin{align*}
\begin{bmatrix} G_{xxxx} & G_{xxyy} & G_{xxzz} & 0 & 0 & 0 & 0 & 0 & 0 \\ G_{yyxx} & G_{yyyy} & G_{yyzz} & 0 & 0 & 0 & 0 & 0 & 0 \\ G_{zzxx} & G_{zzyy} & G_{zzzz} & 0 & 0 & 0 & 0 & 0 & 0 \\ 0 & 0 & 0 & G_{yzyz} & 0 & 0 & G_{yzzy} & 0 & 0 \\ 0 & 0 & 0 & 0 & G_{zxzx} & 0 & 0 & G_{zxxz} & 0 \\ 0 & 0 & 0 & 0 & 0 & G_{xyxy} & 0 & 0 & G_{xyyx} \end{bmatrix}
\end{align*}
\begin{align*}
& G_{xxxx} = - 2 G_{du}^{(1)} - 4 G_{du}^{(2)} + 2 G_{dv}^{(1)} + 4 G_{dv}^{(2)} - G_{gu}^{(1)} + G_{gv}^{(1)} + 2 G_{g}^{(1)} + G_{s}^{(1)} + 2 G_{s}^{(2)} \\
& G_{xxyy} = - 2 G_{du}^{(1)} - 2 G_{dv}^{(3)} + 2 G_{gu}^{(1)} - G_{g}^{(1)} + G_{s}^{(1)} + 4 Q_{f3}^{(1)} \\
& G_{xxzz} = G_{du}^{(1)} + 3 G_{du}^{(3)} + G_{dv}^{(1)} - G_{dv}^{(3)} - G_{gu}^{(1)} - G_{gv}^{(1)} - G_{g}^{(1)} + G_{s}^{(1)} - 4 Q_{f3}^{(1)} \\
& G_{yyxx} = - 2 G_{du}^{(1)} + 2 G_{dv}^{(3)} + 2 G_{gu}^{(1)} - G_{g}^{(1)} + G_{s}^{(1)} - 4 Q_{f3}^{(1)} \\
& G_{yyyy} = - 2 G_{du}^{(1)} - 4 G_{du}^{(2)} - 2 G_{dv}^{(1)} - 4 G_{dv}^{(2)} - G_{gu}^{(1)} - G_{gv}^{(1)} + 2 G_{g}^{(1)} + G_{s}^{(1)} + 2 G_{s}^{(2)} \\
& G_{yyzz} = G_{du}^{(1)} + 3 G_{du}^{(3)} - G_{dv}^{(1)} + G_{dv}^{(3)} - G_{gu}^{(1)} + G_{gv}^{(1)} - G_{g}^{(1)} + G_{s}^{(1)} + 4 Q_{f3}^{(1)} \\
& G_{zzxx} = G_{du}^{(1)} - 3 G_{du}^{(3)} + G_{dv}^{(1)} + G_{dv}^{(3)} - G_{gu}^{(1)} - G_{gv}^{(1)} - G_{g}^{(1)} + G_{s}^{(1)} + 4 Q_{f3}^{(1)} \\
& G_{zzyy} = G_{du}^{(1)} - 3 G_{du}^{(3)} - G_{dv}^{(1)} - G_{dv}^{(3)} - G_{gu}^{(1)} + G_{gv}^{(1)} - G_{g}^{(1)} + G_{s}^{(1)} - 4 Q_{f3}^{(1)} \\
& G_{zzzz} = 4 G_{du}^{(1)} + 8 G_{du}^{(2)} + 2 G_{gu}^{(1)} + 2 G_{g}^{(1)} + G_{s}^{(1)} + 2 G_{s}^{(2)} \\
& G_{yzyz} = G_{du}^{(2)} - 3 G_{du}^{(5)} - G_{dv}^{(2)} - G_{dv}^{(5)} - G_{gu}^{(1)} + G_{gv}^{(1)} - G_{g}^{(1)} + G_{s}^{(2)} + Q_{f3}^{(2)} \\
& G_{yzzy} = G_{du}^{(2)} + 3 G_{du}^{(5)} - G_{dv}^{(2)} + G_{dv}^{(5)} - G_{gu}^{(1)} + G_{gv}^{(1)} - G_{g}^{(1)} + G_{s}^{(2)} - Q_{f3}^{(2)} \\
& G_{zxzx} = G_{du}^{(2)} + 3 G_{du}^{(5)} + G_{dv}^{(2)} - G_{dv}^{(5)} - G_{gu}^{(1)} - G_{gv}^{(1)} - G_{g}^{(1)} + G_{s}^{(2)} + Q_{f3}^{(2)} \\
& G_{zxxz} = G_{du}^{(2)} - 3 G_{du}^{(5)} + G_{dv}^{(2)} + G_{dv}^{(5)} - G_{gu}^{(1)} - G_{gv}^{(1)} - G_{g}^{(1)} + G_{s}^{(2)} - Q_{f3}^{(2)} \\
& G_{xyxy} = - 2 G_{du}^{(2)} + 2 G_{dv}^{(5)} + 2 G_{gu}^{(1)} - G_{g}^{(1)} + G_{s}^{(2)} + Q_{f3}^{(2)} \\
& G_{xyyx} = - 2 G_{du}^{(2)} - 2 G_{dv}^{(5)} + 2 G_{gu}^{(1)} - G_{g}^{(1)} + G_{s}^{(2)} - Q_{f3}^{(2)}
\end{align*}
* Rank 4 tensor (a).
\begin{align*}
\begin{bmatrix} 0 & 0 & 0 & G_{yzyz} & 0 & 0 & G_{yzzy} & 0 & 0 \\ 0 & 0 & 0 & 0 & G_{zxzx} & 0 & 0 & G_{zxxz} & 0 \\ 0 & 0 & 0 & 0 & 0 & G_{xyxy} & 0 & 0 & G_{xyyx} \end{bmatrix}
\end{align*}
\begin{align*}
& G_{yzyz} = - 2 G_{du}^{(4)} - 3 G_{du}^{(6)} + 2 G_{dv}^{(4)} - G_{dv}^{(6)} + G_{s}^{(3)} + Q_{f3}^{(3)} \\
& G_{yzzy} = 2 G_{du}^{(4)} - 3 G_{du}^{(6)} - 2 G_{dv}^{(4)} - G_{dv}^{(6)} - G_{s}^{(3)} + Q_{f3}^{(3)} \\
& G_{zxzx} = - 2 G_{du}^{(4)} + 3 G_{du}^{(6)} - 2 G_{dv}^{(4)} - G_{dv}^{(6)} + G_{s}^{(3)} + Q_{f3}^{(3)} \\
& G_{zxxz} = 2 G_{du}^{(4)} + 3 G_{du}^{(6)} + 2 G_{dv}^{(4)} - G_{dv}^{(6)} - G_{s}^{(3)} + Q_{f3}^{(3)} \\
& G_{xyxy} = 4 G_{du}^{(4)} + 2 G_{dv}^{(6)} + G_{s}^{(3)} + Q_{f3}^{(3)} \\
& G_{xyyx} = - 4 G_{du}^{(4)} + 2 G_{dv}^{(6)} - G_{s}^{(3)} + Q_{f3}^{(3)}
\end{align*}
* Rank 4 tensor (t).
\begin{align*}
\begin{bmatrix} G_{xxxx} & 0 & 0 \\ 0 & G_{yyyy} & 0 \\ 0 & 0 & G_{zzzz} \\ 0 & 0 & G_{yyzz} \\ G_{zzxx} & 0 & 0 \\ 0 & G_{xxyy} & 0 \\ 0 & G_{yzzy} & 0 \\ 0 & 0 & G_{zxxz} \\ G_{xxyy} + G_{yyzz} - G_{yzzy} - G_{zxxz} + G_{zzxx} & 0 & 0 \\ 0 & 0 & 0 \end{bmatrix}
\end{align*}
\begin{align*}
& G_{xxxx} = - 2 G_{du}^{(1)} - 4 G_{du}^{(2)} + 2 G_{dv}^{(1)} + 4 G_{dv}^{(2)} - G_{gu}^{(1)} + G_{gv}^{(1)} + 2 G_{g}^{(1)} + 3 G_{s}^{(1)} \\
& G_{yyyy} = - 2 G_{du}^{(1)} - 4 G_{du}^{(2)} - 2 G_{dv}^{(1)} - 4 G_{dv}^{(2)} - G_{gu}^{(1)} - G_{gv}^{(1)} + 2 G_{g}^{(1)} + 3 G_{s}^{(1)} \\
& G_{zzzz} = 4 G_{du}^{(1)} + 8 G_{du}^{(2)} + 2 G_{gu}^{(1)} + 2 G_{g}^{(1)} + 3 G_{s}^{(1)} \\
& G_{yyzz} = G_{du}^{(1)} + 3 G_{du}^{(3)} - G_{dv}^{(1)} + G_{dv}^{(3)} - G_{gu}^{(1)} + G_{gv}^{(1)} - G_{g}^{(1)} + G_{s}^{(1)} \\
& G_{zzxx} = G_{du}^{(1)} - 3 G_{du}^{(3)} + G_{dv}^{(1)} + G_{dv}^{(3)} - G_{gu}^{(1)} - G_{gv}^{(1)} - G_{g}^{(1)} + G_{s}^{(1)} \\
& G_{xxyy} = - 2 G_{du}^{(1)} - 2 G_{dv}^{(3)} + 2 G_{gu}^{(1)} - G_{g}^{(1)} + G_{s}^{(1)} \\
& G_{yzzy} = G_{du}^{(2)} + 3 G_{du}^{(5)} - G_{dv}^{(2)} + G_{dv}^{(5)} - G_{gu}^{(1)} + G_{gv}^{(1)} - G_{g}^{(1)} + G_{s}^{(1)} \\
& G_{zxxz} = G_{du}^{(2)} - 3 G_{du}^{(5)} + G_{dv}^{(2)} + G_{dv}^{(5)} - G_{gu}^{(1)} - G_{gv}^{(1)} - G_{g}^{(1)} + G_{s}^{(1)}
\end{align*}

\end{document}
