\documentclass[fleqn,8pt,landscape]{jsarticle}
\special{papersize=\the\paperwidth,\the\paperheight}

%%% package

\usepackage[usenames]{color}
\usepackage{amsmath}
\usepackage{breqn}
\usepackage{graphicx}
\usepackage{amssymb}
\usepackage{bm}
\usepackage{enumitem}
\usepackage{braket}
\usepackage{multirow}
\usepackage{booktabs}
\usepackage{longtable}

%%% layout setting

\paperwidth=356.4truemm
\paperheight=252.0truemm
\textwidth=335.59999999999997truemm
\textheight=224.2truemm
\oddsidemargin=-15truemm
\topmargin=-15truemm
\footskip=7truemm

%%% fixed

\hoffset=0truemm
\voffset=0truemm
\headheight=0truemm
\headsep=0truemm
\marginparsep=0truemm
\marginparwidth=0truemm

%%% main text

\begin{document}

\setcounter{MaxMatrixCols}{32}

\renewcommand{\tablename}{Table~}
\renewcommand{\figurename}{Figure~}
\begin{center}
\LARGE
MPG No. 7.3.22\quad$m'm2'$\quad(m'm2' setting)\quad[ Type III, orthorhombic ] [T tensor]
\end{center}
* Rank 0 tensor.
* Rank 1 tensor.
\begin{align*}
\begin{bmatrix} T_{x} & 0 & 0 \end{bmatrix}
\end{align*}
\begin{align*}
& T_{x} = T_{px}^{(1)}
\end{align*}
* Rank 2 tensor (s).
\begin{align*}
\begin{bmatrix} 0 & 0 & T_{xz} \\ 0 & 0 & 0 \\ T_{xz} & 0 & 0 \end{bmatrix}
\end{align*}
\begin{align*}
& T_{xz} = T_{dxz}^{(1)}
\end{align*}
* Rank 2 tensor (a).
\begin{align*}
\begin{bmatrix} 0 & 0 & T_{xz} \\ 0 & 0 & 0 \\ - T_{xz} & 0 & 0 \end{bmatrix}
\end{align*}
\begin{align*}
& T_{xz} = - M_{py}^{(1)}
\end{align*}
* Rank 3 tensor (s).
\begin{align*}
\begin{bmatrix} T_{xxx} & 0 & 0 \\ T_{yyx} & 0 & 0 \\ T_{zzx} & 0 & 0 \\ 0 & 0 & 0 \\ 0 & 0 & T_{zxz} \\ 0 & T_{xyy} & 0 \end{bmatrix}
\end{align*}
\begin{align*}
& T_{xxx} = 2 T_{fax}^{(1)} + T_{px}^{(1)} + 2 T_{px}^{(2)} \\
& T_{yyx} = - 2 M_{dyz}^{(1)} - T_{fax}^{(1)} + T_{fbx}^{(1)} + T_{px}^{(1)} \\
& T_{zzx} = 2 M_{dyz}^{(1)} - T_{fax}^{(1)} - T_{fbx}^{(1)} + T_{px}^{(1)} \\
& T_{zxz} = - M_{dyz}^{(1)} - T_{fax}^{(1)} - T_{fbx}^{(1)} + T_{px}^{(2)} \\
& T_{xyy} = M_{dyz}^{(1)} - T_{fax}^{(1)} + T_{fbx}^{(1)} + T_{px}^{(2)}
\end{align*}
* Rank 3 tensor (a).
\begin{align*}
\begin{bmatrix} 0 & 0 & 0 \\ 0 & 0 & T_{zxz} \\ 0 & T_{xyy} & 0 \end{bmatrix}
\end{align*}
\begin{align*}
& T_{zxz} = M_{dyz}^{(2)} + T_{px}^{(3)} \\
& T_{xyy} = M_{dyz}^{(2)} - T_{px}^{(3)}
\end{align*}
* Rank 4 tensor (sss).
\begin{align*}
\begin{bmatrix} 0 & 0 & 0 & 0 & T_{xxzx} & 0 \\ 0 & 0 & 0 & 0 & T_{yyzx} & 0 \\ 0 & 0 & 0 & 0 & T_{zzzx} & 0 \\ 0 & 0 & 0 & 0 & 0 & T_{yzxy} \\ T_{xxzx} & T_{yyzx} & T_{zzzx} & 0 & 0 & 0 \\ 0 & 0 & 0 & T_{yzxy} & 0 & 0 \end{bmatrix}
\end{align*}
\begin{align*}
& T_{xxzx} = T_{dxz}^{(1)} + 2 T_{dxz}^{(2)} - T_{gay}^{(1)} - T_{gby}^{(1)} \\
& T_{yyzx} = T_{dxz}^{(1)} + 2 T_{gby}^{(1)} \\
& T_{zzzx} = T_{dxz}^{(1)} + 2 T_{dxz}^{(2)} + T_{gay}^{(1)} - T_{gby}^{(1)} \\
& T_{yzxy} = T_{dxz}^{(2)} + 2 T_{gby}^{(1)}
\end{align*}
* Rank 4 tensor (ssa).
\begin{align*}
\begin{bmatrix} 0 & 0 & 0 & 0 & T_{xxzx} & 0 \\ 0 & 0 & 0 & 0 & T_{yyzx} & 0 \\ 0 & 0 & 0 & 0 & T_{zzzx} & 0 \\ 0 & 0 & 0 & 0 & 0 & T_{yzxy} \\ - T_{xxzx} & - T_{yyzx} & - T_{zzzx} & 0 & 0 & 0 \\ 0 & 0 & 0 & - T_{yzxy} & 0 & 0 \end{bmatrix}
\end{align*}
\begin{align*}
& T_{xxzx} = 2 M_{fay}^{(1)} + 2 M_{fby}^{(1)} - 2 M_{py}^{(1)} + T_{dxz}^{(3)} \\
& T_{yyzx} = - 4 M_{fby}^{(1)} + T_{dxz}^{(3)} \\
& T_{zzzx} = - 2 M_{fay}^{(1)} + 2 M_{fby}^{(1)} + 2 M_{py}^{(1)} + T_{dxz}^{(3)} \\
& T_{yzxy} = 4 M_{fay}^{(1)} + M_{py}^{(1)}
\end{align*}
* Rank 4 tensor (aas).
\begin{align*}
\begin{bmatrix} 0 & 0 & T_{yzxy} \\ 0 & 0 & 0 \\ T_{yzxy} & 0 & 0 \end{bmatrix}
\end{align*}
\begin{align*}
& T_{yzxy} = 2 T_{dxz}^{(4)}
\end{align*}
* Rank 4 tensor (aaa).
\begin{align*}
\begin{bmatrix} 0 & 0 & T_{yzxy} \\ 0 & 0 & 0 \\ - T_{yzxy} & 0 & 0 \end{bmatrix}
\end{align*}
\begin{align*}
& T_{yzxy} = M_{py}^{(2)}
\end{align*}
* Rank 4 tensor (sa).
\begin{align*}
\begin{bmatrix} 0 & T_{xxzx} & 0 \\ 0 & T_{yyzx} & 0 \\ 0 & T_{zzzx} & 0 \\ 0 & 0 & T_{yzxy} \\ 0 & 0 & 0 \\ T_{xyyz} & 0 & 0 \end{bmatrix}
\end{align*}
\begin{align*}
& T_{xxzx} = - M_{fay}^{(2)} - M_{fby}^{(2)} + M_{py}^{(3)} + 2 T_{dxz}^{(5)} \\
& T_{yyzx} = 2 M_{fay}^{(2)} + M_{py}^{(3)} + 2 M_{py}^{(4)} \\
& T_{zzzx} = - M_{fay}^{(2)} + M_{fby}^{(2)} + M_{py}^{(3)} - 2 T_{dxz}^{(5)} \\
& T_{yzxy} = - M_{fay}^{(2)} + M_{fby}^{(2)} + M_{py}^{(4)} + T_{dxz}^{(5)} \\
& T_{xyyz} = - M_{fay}^{(2)} - M_{fby}^{(2)} + M_{py}^{(4)} - T_{dxz}^{(5)}
\end{align*}
* Rank 4 tensor (as).
\begin{align*}
\begin{bmatrix} 0 & 0 & 0 & 0 & 0 & T_{yzxy} \\ T_{zxxx} & T_{zxyy} & T_{zxzz} & 0 & 0 & 0 \\ 0 & 0 & 0 & T_{xyyz} & 0 & 0 \end{bmatrix}
\end{align*}
\begin{align*}
& T_{yzxy} = - M_{fay}^{(3)} - M_{fby}^{(3)} + M_{py}^{(6)} - T_{dxz}^{(6)} \\
& T_{zxxx} = - M_{fay}^{(3)} - M_{fby}^{(3)} + M_{py}^{(5)} + 2 T_{dxz}^{(6)} \\
& T_{zxyy} = 2 M_{fay}^{(3)} + M_{py}^{(5)} + 2 M_{py}^{(6)} \\
& T_{zxzz} = - M_{fay}^{(3)} + M_{fby}^{(3)} + M_{py}^{(5)} - 2 T_{dxz}^{(6)} \\
& T_{xyyz} = - M_{fay}^{(3)} + M_{fby}^{(3)} + M_{py}^{(6)} + T_{dxz}^{(6)}
\end{align*}
* Rank 4 tensor (s).
\begin{align*}
\begin{bmatrix} 0 & 0 & 0 & 0 & T_{xxzx} & 0 & 0 & T_{xxxz} & 0 \\ 0 & 0 & 0 & 0 & T_{yyzx} & 0 & 0 & T_{yyxz} & 0 \\ 0 & 0 & 0 & 0 & T_{zzzx} & 0 & 0 & T_{zzxz} & 0 \\ 0 & 0 & 0 & 0 & 0 & T_{yzxy} & 0 & 0 & T_{yzyx} \\ T_{zxxx} & T_{zxyy} & T_{zxzz} & 0 & 0 & 0 & 0 & 0 & 0 \\ 0 & 0 & 0 & T_{xyyz} & 0 & 0 & T_{xyzy} & 0 & 0 \end{bmatrix}
\end{align*}
\begin{align*}
& T_{xxzx} = 2 M_{fay}^{(1)} - M_{fay}^{(2)} + 2 M_{fby}^{(1)} - M_{fby}^{(2)} - 2 M_{py}^{(1)} + M_{py}^{(3)} + T_{dxz}^{(1)} + 2 T_{dxz}^{(2)} + T_{dxz}^{(3)} + 2 T_{dxz}^{(5)} - T_{gay}^{(1)} - T_{gby}^{(1)} \\
& T_{xxxz} = 2 M_{fay}^{(1)} + M_{fay}^{(2)} + 2 M_{fby}^{(1)} + M_{fby}^{(2)} - 2 M_{py}^{(1)} - M_{py}^{(3)} + T_{dxz}^{(1)} + 2 T_{dxz}^{(2)} + T_{dxz}^{(3)} - 2 T_{dxz}^{(5)} - T_{gay}^{(1)} - T_{gby}^{(1)} \\
& T_{yyzx} = 2 M_{fay}^{(2)} - 4 M_{fby}^{(1)} + M_{py}^{(3)} + 2 M_{py}^{(4)} + T_{dxz}^{(1)} + T_{dxz}^{(3)} + 2 T_{gby}^{(1)} \\
& T_{yyxz} = - 2 M_{fay}^{(2)} - 4 M_{fby}^{(1)} - M_{py}^{(3)} - 2 M_{py}^{(4)} + T_{dxz}^{(1)} + T_{dxz}^{(3)} + 2 T_{gby}^{(1)} \\
& T_{zzzx} = - 2 M_{fay}^{(1)} - M_{fay}^{(2)} + 2 M_{fby}^{(1)} + M_{fby}^{(2)} + 2 M_{py}^{(1)} + M_{py}^{(3)} + T_{dxz}^{(1)} + 2 T_{dxz}^{(2)} + T_{dxz}^{(3)} - 2 T_{dxz}^{(5)} + T_{gay}^{(1)} - T_{gby}^{(1)} \\
& T_{zzxz} = - 2 M_{fay}^{(1)} + M_{fay}^{(2)} + 2 M_{fby}^{(1)} - M_{fby}^{(2)} + 2 M_{py}^{(1)} - M_{py}^{(3)} + T_{dxz}^{(1)} + 2 T_{dxz}^{(2)} + T_{dxz}^{(3)} + 2 T_{dxz}^{(5)} + T_{gay}^{(1)} - T_{gby}^{(1)} \\
& T_{yzxy} = 4 M_{fay}^{(1)} - M_{fay}^{(2)} + M_{fby}^{(2)} + M_{py}^{(1)} + M_{py}^{(4)} + T_{dxz}^{(2)} + T_{dxz}^{(5)} + 2 T_{gby}^{(1)} \\
& T_{yzyx} = 4 M_{fay}^{(1)} + M_{fay}^{(2)} - M_{fby}^{(2)} + M_{py}^{(1)} - M_{py}^{(4)} + T_{dxz}^{(2)} - T_{dxz}^{(5)} + 2 T_{gby}^{(1)} \\
& T_{zxxx} = - 2 M_{fay}^{(1)} - 2 M_{fby}^{(1)} + 2 M_{py}^{(1)} + T_{dxz}^{(1)} + 2 T_{dxz}^{(2)} - T_{dxz}^{(3)} - T_{gay}^{(1)} - T_{gby}^{(1)} \\
& T_{zxyy} = 4 M_{fby}^{(1)} + T_{dxz}^{(1)} - T_{dxz}^{(3)} + 2 T_{gby}^{(1)} \\
& T_{zxzz} = 2 M_{fay}^{(1)} - 2 M_{fby}^{(1)} - 2 M_{py}^{(1)} + T_{dxz}^{(1)} + 2 T_{dxz}^{(2)} - T_{dxz}^{(3)} + T_{gay}^{(1)} - T_{gby}^{(1)} \\
& T_{xyyz} = - 4 M_{fay}^{(1)} - M_{fay}^{(2)} - M_{fby}^{(2)} - M_{py}^{(1)} + M_{py}^{(4)} + T_{dxz}^{(2)} - T_{dxz}^{(5)} + 2 T_{gby}^{(1)} \\
& T_{xyzy} = - 4 M_{fay}^{(1)} + M_{fay}^{(2)} + M_{fby}^{(2)} - M_{py}^{(1)} - M_{py}^{(4)} + T_{dxz}^{(2)} + T_{dxz}^{(5)} + 2 T_{gby}^{(1)}
\end{align*}
* Rank 4 tensor (a).
\begin{align*}
\begin{bmatrix} 0 & 0 & 0 & 0 & 0 & T_{yzxy} & 0 & 0 & T_{yzyx} \\ T_{zxxx} & T_{zxyy} & T_{zxzz} & 0 & 0 & 0 & 0 & 0 & 0 \\ 0 & 0 & 0 & T_{xyyz} & 0 & 0 & T_{xyzy} & 0 & 0 \end{bmatrix}
\end{align*}
\begin{align*}
& T_{yzxy} = - M_{fay}^{(3)} - M_{fby}^{(3)} + M_{py}^{(2)} + M_{py}^{(6)} + 2 T_{dxz}^{(4)} - T_{dxz}^{(6)} \\
& T_{yzyx} = - M_{fay}^{(3)} - M_{fby}^{(3)} - M_{py}^{(2)} + M_{py}^{(6)} - 2 T_{dxz}^{(4)} - T_{dxz}^{(6)} \\
& T_{zxxx} = - M_{fay}^{(3)} - M_{fby}^{(3)} + M_{py}^{(5)} + 2 T_{dxz}^{(6)} \\
& T_{zxyy} = 2 M_{fay}^{(3)} + M_{py}^{(5)} + 2 M_{py}^{(6)} \\
& T_{zxzz} = - M_{fay}^{(3)} + M_{fby}^{(3)} + M_{py}^{(5)} - 2 T_{dxz}^{(6)} \\
& T_{xyyz} = - M_{fay}^{(3)} + M_{fby}^{(3)} - M_{py}^{(2)} + M_{py}^{(6)} + 2 T_{dxz}^{(4)} + T_{dxz}^{(6)} \\
& T_{xyzy} = - M_{fay}^{(3)} + M_{fby}^{(3)} + M_{py}^{(2)} + M_{py}^{(6)} - 2 T_{dxz}^{(4)} + T_{dxz}^{(6)}
\end{align*}
* Rank 4 tensor (t).
\begin{align*}
\begin{bmatrix} 0 & 0 & T_{xxxz} \\ 0 & 0 & 0 \\ T_{zzzx} & 0 & 0 \\ T_{yyzx} & 0 & 0 \\ 0 & 0 & T_{zzxz} \\ 0 & 0 & 0 \\ 0 & 0 & 0 \\ T_{zxxx} & 0 & 0 \\ 0 & 0 & T_{xyyz} \\ 0 & T_{xyyz} + \frac{T_{zzxz}}{2} - \frac{T_{zzzx}}{2} & 0 \end{bmatrix}
\end{align*}
\begin{align*}
& T_{xxxz} = T_{dxz}^{(1)} + 2 T_{dxz}^{(2)} + T_{dxz}^{(3)} - 2 T_{dxz}^{(5)} - T_{gay}^{(1)} - T_{gby}^{(1)} \\
& T_{zzzx} = T_{dxz}^{(1)} + 2 T_{dxz}^{(2)} + T_{dxz}^{(3)} - 2 T_{dxz}^{(5)} + T_{gay}^{(1)} - T_{gby}^{(1)} \\
& T_{yyzx} = T_{dxz}^{(1)} + T_{dxz}^{(3)} + 2 T_{gby}^{(1)} \\
& T_{zzxz} = T_{dxz}^{(1)} + 2 T_{dxz}^{(2)} + T_{dxz}^{(3)} + 2 T_{dxz}^{(5)} + T_{gay}^{(1)} - T_{gby}^{(1)} \\
& T_{zxxx} = T_{dxz}^{(1)} + 2 T_{dxz}^{(2)} - T_{dxz}^{(3)} - T_{gay}^{(1)} - T_{gby}^{(1)} \\
& T_{xyyz} = T_{dxz}^{(2)} - T_{dxz}^{(5)} + 2 T_{gby}^{(1)}
\end{align*}

\end{document}
