\documentclass[fleqn,8pt,landscape]{jsarticle}
\special{papersize=\the\paperwidth,\the\paperheight}

%%% package

\usepackage[usenames]{color}
\usepackage{amsmath}
\usepackage{breqn}
\usepackage{graphicx}
\usepackage{amssymb}
\usepackage{bm}
\usepackage{enumitem}
\usepackage{braket}
\usepackage{multirow}
\usepackage{booktabs}
\usepackage{longtable}

%%% layout setting

\paperwidth=356.4truemm
\paperheight=252.0truemm
\textwidth=335.59999999999997truemm
\textheight=224.2truemm
\oddsidemargin=-15truemm
\topmargin=-15truemm
\footskip=7truemm

%%% fixed

\hoffset=0truemm
\voffset=0truemm
\headheight=0truemm
\headsep=0truemm
\marginparsep=0truemm
\marginparwidth=0truemm

%%% main text

\begin{document}

\setcounter{MaxMatrixCols}{32}

\renewcommand{\tablename}{Table~}
\renewcommand{\figurename}{Figure~}
\begin{center}
\LARGE
MPG No. 16.1.60\quad$3$\quad[ Type I, trigonal ] [G tensor]
\end{center}
* Rank 0 tensor.
\begin{align*}
\begin{bmatrix} G \end{bmatrix}
\end{align*}
\begin{align*}
& G = G_{s}^{(1)}
\end{align*}
* Rank 1 tensor.
\begin{align*}
\begin{bmatrix} 0 & 0 & G_{z} \end{bmatrix}
\end{align*}
\begin{align*}
& G_{z} = G_{pz}^{(1)}
\end{align*}
* Rank 2 tensor (s).
\begin{align*}
\begin{bmatrix} G_{xx} & 0 & 0 \\ 0 & G_{xx} & 0 \\ 0 & 0 & G_{zz} \end{bmatrix}
\end{align*}
\begin{align*}
& G_{xx} = - G_{du}^{(1)} + G_{s}^{(1)} \\
& G_{zz} = 2 G_{du}^{(1)} + G_{s}^{(1)}
\end{align*}
* Rank 2 tensor (a).
\begin{align*}
\begin{bmatrix} 0 & G_{xy} & 0 \\ - G_{xy} & 0 & 0 \\ 0 & 0 & 0 \end{bmatrix}
\end{align*}
\begin{align*}
& G_{xy} = Q_{pz}^{(1)}
\end{align*}
* Rank 3 tensor (s).
\begin{align*}
\begin{bmatrix} G_{xxx} & G_{xxy} & G_{xxz} \\ - G_{xxx} & - G_{xxy} & G_{xxz} \\ 0 & 0 & G_{zzz} \\ G_{yzx} & G_{yzy} & 0 \\ G_{yzy} & - G_{yzx} & 0 \\ G_{xxy} & - G_{xxx} & 0 \end{bmatrix}
\end{align*}
\begin{align*}
& G_{xxx} = G_{f2}^{(1)} \\
& G_{xxy} = G_{f1}^{(1)} \\
& G_{xxz} = - G_{faz}^{(1)} + G_{pz}^{(1)} \\
& G_{zzz} = 2 G_{faz}^{(1)} + G_{pz}^{(1)} + 2 G_{pz}^{(2)} \\
& G_{yzx} = - 3 Q_{du}^{(1)} \\
& G_{yzy} = - G_{faz}^{(1)} + G_{pz}^{(2)}
\end{align*}
* Rank 3 tensor (a).
\begin{align*}
\begin{bmatrix} G_{yzx} & G_{yzy} & 0 \\ - G_{yzy} & G_{yzx} & 0 \\ 0 & 0 & G_{xyz} \end{bmatrix}
\end{align*}
\begin{align*}
& G_{yzx} = - Q_{du}^{(2)} + Q_{s}^{(1)} \\
& G_{yzy} = G_{pz}^{(3)} \\
& G_{xyz} = 2 Q_{du}^{(2)} + Q_{s}^{(1)}
\end{align*}
* Rank 4 tensor (sss).
\begin{align*}
\begin{bmatrix} G_{xxxx} & G_{xxyy} & G_{xxzz} & G_{xxyz} & G_{xxzx} & 0 \\ G_{xxyy} & G_{xxxx} & G_{xxzz} & - G_{xxyz} & - G_{xxzx} & 0 \\ G_{xxzz} & G_{xxzz} & G_{zzzz} & 0 & 0 & 0 \\ G_{xxyz} & - G_{xxyz} & 0 & G_{yzyz} & 0 & - G_{xxzx} \\ G_{xxzx} & - G_{xxzx} & 0 & 0 & G_{yzyz} & G_{xxyz} \\ 0 & 0 & 0 & - G_{xxzx} & G_{xxyz} & \frac{G_{xxxx}}{2} - \frac{G_{xxyy}}{2} \end{bmatrix}
\end{align*}
\begin{align*}
& G_{xxxx} = - 2 G_{du}^{(1)} - 4 G_{du}^{(2)} + 3 G_{g0}^{(1)} + G_{s}^{(1)} + 2 G_{s}^{(2)} \\
& G_{xxyy} = - 2 G_{du}^{(1)} + G_{g0}^{(1)} + G_{s}^{(1)} \\
& G_{xxzz} = G_{du}^{(1)} - 4 G_{g0}^{(1)} + G_{s}^{(1)} \\
& G_{xxyz} = G_{gb}^{(1)} \\
& G_{xxzx} = G_{ga}^{(1)} \\
& G_{zzzz} = 4 G_{du}^{(1)} + 8 G_{du}^{(2)} + 8 G_{g0}^{(1)} + G_{s}^{(1)} + 2 G_{s}^{(2)} \\
& G_{yzyz} = G_{du}^{(2)} - 4 G_{g0}^{(1)} + G_{s}^{(2)}
\end{align*}
* Rank 4 tensor (ssa).
\begin{align*}
\begin{bmatrix} 0 & 0 & G_{xxzz} & G_{xxyz} & G_{xxzx} & G_{xxxy} \\ 0 & 0 & G_{xxzz} & - G_{xxyz} & - G_{xxzx} & - G_{xxxy} \\ - G_{xxzz} & - G_{xxzz} & 0 & 0 & 0 & 0 \\ - G_{xxyz} & G_{xxyz} & 0 & 0 & G_{yzzx} & G_{xxzx} \\ - G_{xxzx} & G_{xxzx} & 0 & - G_{yzzx} & 0 & - G_{xxyz} \\ - G_{xxxy} & G_{xxxy} & 0 & - G_{xxzx} & G_{xxyz} & 0 \end{bmatrix}
\end{align*}
\begin{align*}
& G_{xxzz} = 3 G_{du}^{(3)} \\
& G_{xxyz} = 2 Q_{f2}^{(1)} \\
& G_{xxzx} = - 2 Q_{f1}^{(1)} \\
& G_{xxxy} = - 2 Q_{faz}^{(1)} + 2 Q_{pz}^{(1)} \\
& G_{yzzx} = - 4 Q_{faz}^{(1)} - Q_{pz}^{(1)}
\end{align*}
* Rank 4 tensor (aas).
\begin{align*}
\begin{bmatrix} G_{yzyz} & 0 & 0 \\ 0 & G_{yzyz} & 0 \\ 0 & 0 & G_{xyxy} \end{bmatrix}
\end{align*}
\begin{align*}
& G_{yzyz} = - 2 G_{du}^{(4)} + G_{s}^{(3)} \\
& G_{xyxy} = 4 G_{du}^{(4)} + G_{s}^{(3)}
\end{align*}
* Rank 4 tensor (aaa).
\begin{align*}
\begin{bmatrix} 0 & G_{yzzx} & 0 \\ - G_{yzzx} & 0 & 0 \\ 0 & 0 & 0 \end{bmatrix}
\end{align*}
\begin{align*}
& G_{yzzx} = - Q_{pz}^{(2)}
\end{align*}
* Rank 4 tensor (sa).
\begin{align*}
\begin{bmatrix} G_{xxyz} & G_{xxzx} & G_{xxxy} \\ - G_{xxyz} & - G_{xxzx} & G_{xxxy} \\ 0 & 0 & G_{zzxy} \\ G_{yzyz} & G_{yzzx} & 0 \\ G_{yzzx} & - G_{yzyz} & 0 \\ G_{xxzx} & - G_{xxyz} & 0 \end{bmatrix}
\end{align*}
\begin{align*}
& G_{xxyz} = Q_{f2}^{(2)} \\
& G_{xxzx} = Q_{f1}^{(2)} \\
& G_{xxxy} = - Q_{faz}^{(2)} + Q_{pz}^{(3)} \\
& G_{zzxy} = 2 Q_{faz}^{(2)} + Q_{pz}^{(3)} + 2 Q_{pz}^{(4)} \\
& G_{yzyz} = - 3 G_{du}^{(5)} \\
& G_{yzzx} = - Q_{faz}^{(2)} + Q_{pz}^{(4)}
\end{align*}
* Rank 4 tensor (as).
\begin{align*}
\begin{bmatrix} G_{yzxx} & - G_{yzxx} & 0 & G_{yzyz} & G_{yzzx} & G_{yzxy} \\ G_{yzxy} & - G_{yzxy} & 0 & G_{yzzx} & - G_{yzyz} & - G_{yzxx} \\ G_{xyxx} & G_{xyxx} & G_{xyzz} & 0 & 0 & 0 \end{bmatrix}
\end{align*}
\begin{align*}
& G_{yzxx} = Q_{f2}^{(3)} \\
& G_{yzyz} = - 3 G_{du}^{(6)} \\
& G_{yzzx} = - Q_{faz}^{(3)} + Q_{pz}^{(6)} \\
& G_{yzxy} = Q_{f1}^{(3)} \\
& G_{xyxx} = - Q_{faz}^{(3)} + Q_{pz}^{(5)} \\
& G_{xyzz} = 2 Q_{faz}^{(3)} + Q_{pz}^{(5)} + 2 Q_{pz}^{(6)}
\end{align*}
* Rank 4 tensor (s).
\begin{align*}
\begin{bmatrix} G_{xxxx} & G_{xxyy} & G_{xxzz} & G_{xxyz} & G_{xxzx} & G_{xxxy} & G_{xxzy} & G_{xxxz} & G_{xxyx} \\ G_{xxyy} & G_{xxxx} & G_{xxzz} & - G_{xxyz} & - G_{xxzx} & - G_{xxyx} & - G_{xxzy} & - G_{xxxz} & - G_{xxxy} \\ G_{zzxx} & G_{zzxx} & G_{zzzz} & 0 & 0 & G_{zzxy} & 0 & 0 & - G_{zzxy} \\ G_{yzxx} & - G_{yzxx} & 0 & G_{yzyz} & G_{yzzx} & G_{yzxy} & G_{yzzy} & G_{yzxz} & G_{yzxy} \\ - G_{yzxy} & G_{yzxy} & 0 & - G_{yzxz} & G_{yzzy} & G_{yzxx} & - G_{yzzx} & G_{yzyz} & G_{yzxx} \\ - \frac{G_{xxxy}}{2} - \frac{G_{xxyx}}{2} & \frac{G_{xxxy}}{2} + \frac{G_{xxyx}}{2} & 0 & - G_{xxxz} & G_{xxzy} & \frac{G_{xxxx}}{2} - \frac{G_{xxyy}}{2} & - G_{xxzx} & G_{xxyz} & \frac{G_{xxxx}}{2} - \frac{G_{xxyy}}{2} \end{bmatrix}
\end{align*}
\begin{align*}
& G_{xxxx} = - 2 G_{du}^{(1)} - 4 G_{du}^{(2)} + 3 G_{g0}^{(1)} + G_{s}^{(1)} + 2 G_{s}^{(2)} \\
& G_{xxyy} = - 2 G_{du}^{(1)} + G_{g0}^{(1)} + G_{s}^{(1)} \\
& G_{xxzz} = G_{du}^{(1)} + 3 G_{du}^{(3)} - 4 G_{g0}^{(1)} + G_{s}^{(1)} \\
& G_{xxyz} = G_{gb}^{(1)} + 2 Q_{f2}^{(1)} + Q_{f2}^{(2)} \\
& G_{xxzx} = G_{ga}^{(1)} - 2 Q_{f1}^{(1)} + Q_{f1}^{(2)} \\
& G_{xxxy} = - 2 Q_{faz}^{(1)} - Q_{faz}^{(2)} + 2 Q_{pz}^{(1)} + Q_{pz}^{(3)} \\
& G_{xxzy} = G_{gb}^{(1)} + 2 Q_{f2}^{(1)} - Q_{f2}^{(2)} \\
& G_{xxxz} = G_{ga}^{(1)} - 2 Q_{f1}^{(1)} - Q_{f1}^{(2)} \\
& G_{xxyx} = - 2 Q_{faz}^{(1)} + Q_{faz}^{(2)} + 2 Q_{pz}^{(1)} - Q_{pz}^{(3)} \\
& G_{zzxx} = G_{du}^{(1)} - 3 G_{du}^{(3)} - 4 G_{g0}^{(1)} + G_{s}^{(1)} \\
& G_{zzzz} = 4 G_{du}^{(1)} + 8 G_{du}^{(2)} + 8 G_{g0}^{(1)} + G_{s}^{(1)} + 2 G_{s}^{(2)} \\
& G_{zzxy} = 2 Q_{faz}^{(2)} + Q_{pz}^{(3)} + 2 Q_{pz}^{(4)} \\
& G_{yzxx} = G_{gb}^{(1)} - 2 Q_{f2}^{(1)} \\
& G_{yzyz} = G_{du}^{(2)} - 3 G_{du}^{(5)} - 4 G_{g0}^{(1)} + G_{s}^{(2)} \\
& G_{yzzx} = - 4 Q_{faz}^{(1)} - Q_{faz}^{(2)} - Q_{pz}^{(1)} + Q_{pz}^{(4)} \\
& G_{yzxy} = - G_{ga}^{(1)} - 2 Q_{f1}^{(1)} \\
& G_{yzzy} = G_{du}^{(2)} + 3 G_{du}^{(5)} - 4 G_{g0}^{(1)} + G_{s}^{(2)} \\
& G_{yzxz} = - 4 Q_{faz}^{(1)} + Q_{faz}^{(2)} - Q_{pz}^{(1)} - Q_{pz}^{(4)}
\end{align*}
* Rank 4 tensor (a).
\begin{align*}
\begin{bmatrix} G_{yzxx} & - G_{yzxx} & 0 & G_{yzyz} & G_{yzzx} & G_{yzxy} & G_{yzzy} & G_{yzxz} & G_{yzxy} \\ G_{yzxy} & - G_{yzxy} & 0 & G_{yzxz} & - G_{yzzy} & - G_{yzxx} & G_{yzzx} & - G_{yzyz} & - G_{yzxx} \\ G_{xyxx} & G_{xyxx} & G_{xyzz} & 0 & 0 & G_{xyxy} & 0 & 0 & - G_{xyxy} \end{bmatrix}
\end{align*}
\begin{align*}
& G_{yzxx} = Q_{f2}^{(3)} \\
& G_{yzyz} = - 2 G_{du}^{(4)} - 3 G_{du}^{(6)} + G_{s}^{(3)} \\
& G_{yzzx} = - Q_{faz}^{(3)} - Q_{pz}^{(2)} + Q_{pz}^{(6)} \\
& G_{yzxy} = Q_{f1}^{(3)} \\
& G_{yzzy} = 2 G_{du}^{(4)} - 3 G_{du}^{(6)} - G_{s}^{(3)} \\
& G_{yzxz} = - Q_{faz}^{(3)} + Q_{pz}^{(2)} + Q_{pz}^{(6)} \\
& G_{xyxx} = - Q_{faz}^{(3)} + Q_{pz}^{(5)} \\
& G_{xyzz} = 2 Q_{faz}^{(3)} + Q_{pz}^{(5)} + 2 Q_{pz}^{(6)} \\
& G_{xyxy} = 4 G_{du}^{(4)} + G_{s}^{(3)}
\end{align*}
* Rank 4 tensor (t).
\begin{align*}
\begin{bmatrix} G_{xxxx} & 0 & G_{xxxz} \\ 0 & G_{xxxx} & G_{yyyz} \\ 0 & 0 & G_{zzzz} \\ - G_{xxxz} & G_{yyyz} & G_{yyzz} \\ G_{zzxx} & 0 & 0 \\ 0 & G_{xxyy} & - G_{yyyz} \\ 0 & G_{yzzy} & 0 \\ G_{xxxz} & - G_{yyyz} & - \frac{G_{xxxx}}{2} + \frac{3 G_{xxyy}}{2} + G_{yyzz} - G_{yzzy} + G_{zzxx} \\ \frac{G_{xxxx}}{2} - \frac{G_{xxyy}}{2} & 0 & - G_{xxxz} \\ - G_{yyyz} & - G_{xxxz} & 0 \end{bmatrix}
\end{align*}
\begin{align*}
& G_{xxxx} = - 2 G_{du}^{(1)} - 4 G_{du}^{(2)} + 3 G_{g0}^{(1)} + 3 G_{s}^{(1)} \\
& G_{xxxz} = G_{ga}^{(1)} \\
& G_{yyyz} = - G_{gb}^{(1)} \\
& G_{zzzz} = 4 G_{du}^{(1)} + 8 G_{du}^{(2)} + 8 G_{g0}^{(1)} + 3 G_{s}^{(1)} \\
& G_{yyzz} = G_{du}^{(1)} + 3 G_{du}^{(3)} - 4 G_{g0}^{(1)} + G_{s}^{(1)} \\
& G_{zzxx} = G_{du}^{(1)} - 3 G_{du}^{(3)} - 4 G_{g0}^{(1)} + G_{s}^{(1)} \\
& G_{xxyy} = - 2 G_{du}^{(1)} + G_{g0}^{(1)} + G_{s}^{(1)} \\
& G_{yzzy} = G_{du}^{(2)} + 3 G_{du}^{(5)} - 4 G_{g0}^{(1)} + G_{s}^{(1)}
\end{align*}

\end{document}
