\documentclass[fleqn,8pt,landscape]{jsarticle}
\special{papersize=\the\paperwidth,\the\paperheight}

%%% package

\usepackage[usenames]{color}
\usepackage{amsmath}
\usepackage{breqn}
\usepackage{graphicx}
\usepackage{amssymb}
\usepackage{bm}
\usepackage{enumitem}
\usepackage{braket}
\usepackage{multirow}
\usepackage{booktabs}
\usepackage{longtable}

%%% layout setting

\paperwidth=356.4truemm
\paperheight=252.0truemm
\textwidth=335.59999999999997truemm
\textheight=224.2truemm
\oddsidemargin=-15truemm
\topmargin=-15truemm
\footskip=7truemm

%%% fixed

\hoffset=0truemm
\voffset=0truemm
\headheight=0truemm
\headsep=0truemm
\marginparsep=0truemm
\marginparwidth=0truemm

%%% main text

\begin{document}

\setcounter{MaxMatrixCols}{32}

\renewcommand{\tablename}{Table~}
\renewcommand{\figurename}{Figure~}
\begin{center}
\LARGE
MPG No. 7.4.23\quad$m'm'2$\quad[ Type III, orthorhombic ] [T tensor]
\end{center}
* Rank 0 tensor.
* Rank 1 tensor.
* Rank 2 tensor (s).
\begin{align*}
\begin{bmatrix} 0 & T_{xy} & 0 \\ T_{xy} & 0 & 0 \\ 0 & 0 & 0 \end{bmatrix}
\end{align*}
\begin{align*}
& T_{xy} = T_{dxy}^{(1)}
\end{align*}
* Rank 2 tensor (a).
\begin{align*}
\begin{bmatrix} 0 & T_{xy} & 0 \\ - T_{xy} & 0 & 0 \\ 0 & 0 & 0 \end{bmatrix}
\end{align*}
\begin{align*}
& T_{xy} = M_{pz}^{(1)}
\end{align*}
* Rank 3 tensor (s).
\begin{align*}
\begin{bmatrix} 0 & 0 & 0 \\ 0 & 0 & 0 \\ 0 & 0 & 0 \\ T_{yzx} & 0 & 0 \\ 0 & T_{zxy} & 0 \\ 0 & 0 & T_{xyz} \end{bmatrix}
\end{align*}
\begin{align*}
& T_{yzx} = - 3 M_{du}^{(1)} - M_{dv}^{(1)} + T_{f3}^{(1)} \\
& T_{zxy} = 3 M_{du}^{(1)} - M_{dv}^{(1)} + T_{f3}^{(1)} \\
& T_{xyz} = 2 M_{dv}^{(1)} + T_{f3}^{(1)}
\end{align*}
* Rank 3 tensor (a).
\begin{align*}
\begin{bmatrix} T_{yzx} & 0 & 0 \\ 0 & T_{zxy} & 0 \\ 0 & 0 & T_{xyz} \end{bmatrix}
\end{align*}
\begin{align*}
& T_{yzx} = - M_{du}^{(2)} + M_{dv}^{(2)} + M_{s}^{(1)} \\
& T_{zxy} = - M_{du}^{(2)} - M_{dv}^{(2)} + M_{s}^{(1)} \\
& T_{xyz} = 2 M_{du}^{(2)} + M_{s}^{(1)}
\end{align*}
* Rank 4 tensor (sss).
\begin{align*}
\begin{bmatrix} 0 & 0 & 0 & 0 & 0 & T_{xxxy} \\ 0 & 0 & 0 & 0 & 0 & T_{yyxy} \\ 0 & 0 & 0 & 0 & 0 & T_{zzxy} \\ 0 & 0 & 0 & 0 & T_{yzzx} & 0 \\ 0 & 0 & 0 & T_{yzzx} & 0 & 0 \\ T_{xxxy} & T_{yyxy} & T_{zzxy} & 0 & 0 & 0 \end{bmatrix}
\end{align*}
\begin{align*}
& T_{xxxy} = T_{dxy}^{(1)} + 2 T_{dxy}^{(2)} + T_{gaz}^{(1)} - T_{gbz}^{(1)} \\
& T_{yyxy} = T_{dxy}^{(1)} + 2 T_{dxy}^{(2)} - T_{gaz}^{(1)} - T_{gbz}^{(1)} \\
& T_{zzxy} = T_{dxy}^{(1)} + 2 T_{gbz}^{(1)} \\
& T_{yzzx} = T_{dxy}^{(2)} + 2 T_{gbz}^{(1)}
\end{align*}
* Rank 4 tensor (ssa).
\begin{align*}
\begin{bmatrix} 0 & 0 & 0 & 0 & 0 & T_{xxxy} \\ 0 & 0 & 0 & 0 & 0 & T_{yyxy} \\ 0 & 0 & 0 & 0 & 0 & T_{zzxy} \\ 0 & 0 & 0 & 0 & T_{yzzx} & 0 \\ 0 & 0 & 0 & - T_{yzzx} & 0 & 0 \\ - T_{xxxy} & - T_{yyxy} & - T_{zzxy} & 0 & 0 & 0 \end{bmatrix}
\end{align*}
\begin{align*}
& T_{xxxy} = - 2 M_{faz}^{(1)} + 2 M_{fbz}^{(1)} + 2 M_{pz}^{(1)} + T_{dxy}^{(3)} \\
& T_{yyxy} = 2 M_{faz}^{(1)} + 2 M_{fbz}^{(1)} - 2 M_{pz}^{(1)} + T_{dxy}^{(3)} \\
& T_{zzxy} = - 4 M_{fbz}^{(1)} + T_{dxy}^{(3)} \\
& T_{yzzx} = - 4 M_{faz}^{(1)} - M_{pz}^{(1)}
\end{align*}
* Rank 4 tensor (aas).
\begin{align*}
\begin{bmatrix} 0 & T_{yzzx} & 0 \\ T_{yzzx} & 0 & 0 \\ 0 & 0 & 0 \end{bmatrix}
\end{align*}
\begin{align*}
& T_{yzzx} = 2 T_{dxy}^{(4)}
\end{align*}
* Rank 4 tensor (aaa).
\begin{align*}
\begin{bmatrix} 0 & T_{yzzx} & 0 \\ - T_{yzzx} & 0 & 0 \\ 0 & 0 & 0 \end{bmatrix}
\end{align*}
\begin{align*}
& T_{yzzx} = - M_{pz}^{(2)}
\end{align*}
* Rank 4 tensor (sa).
\begin{align*}
\begin{bmatrix} 0 & 0 & T_{xxxy} \\ 0 & 0 & T_{yyxy} \\ 0 & 0 & T_{zzxy} \\ 0 & T_{yzzx} & 0 \\ T_{zxyz} & 0 & 0 \\ 0 & 0 & 0 \end{bmatrix}
\end{align*}
\begin{align*}
& T_{xxxy} = - M_{faz}^{(2)} + M_{fbz}^{(2)} + M_{pz}^{(3)} - 2 T_{dxy}^{(5)} \\
& T_{yyxy} = - M_{faz}^{(2)} - M_{fbz}^{(2)} + M_{pz}^{(3)} + 2 T_{dxy}^{(5)} \\
& T_{zzxy} = 2 M_{faz}^{(2)} + M_{pz}^{(3)} + 2 M_{pz}^{(4)} \\
& T_{yzzx} = - M_{faz}^{(2)} - M_{fbz}^{(2)} + M_{pz}^{(4)} - T_{dxy}^{(5)} \\
& T_{zxyz} = - M_{faz}^{(2)} + M_{fbz}^{(2)} + M_{pz}^{(4)} + T_{dxy}^{(5)}
\end{align*}
* Rank 4 tensor (as).
\begin{align*}
\begin{bmatrix} 0 & 0 & 0 & 0 & T_{yzzx} & 0 \\ 0 & 0 & 0 & T_{zxyz} & 0 & 0 \\ T_{xyxx} & T_{xyyy} & T_{xyzz} & 0 & 0 & 0 \end{bmatrix}
\end{align*}
\begin{align*}
& T_{yzzx} = - M_{faz}^{(3)} + M_{fbz}^{(3)} + M_{pz}^{(6)} + T_{dxy}^{(6)} \\
& T_{zxyz} = - M_{faz}^{(3)} - M_{fbz}^{(3)} + M_{pz}^{(6)} - T_{dxy}^{(6)} \\
& T_{xyxx} = - M_{faz}^{(3)} + M_{fbz}^{(3)} + M_{pz}^{(5)} - 2 T_{dxy}^{(6)} \\
& T_{xyyy} = - M_{faz}^{(3)} - M_{fbz}^{(3)} + M_{pz}^{(5)} + 2 T_{dxy}^{(6)} \\
& T_{xyzz} = 2 M_{faz}^{(3)} + M_{pz}^{(5)} + 2 M_{pz}^{(6)}
\end{align*}
* Rank 4 tensor (s).
\begin{align*}
\begin{bmatrix} 0 & 0 & 0 & 0 & 0 & T_{xxxy} & 0 & 0 & T_{xxyx} \\ 0 & 0 & 0 & 0 & 0 & T_{yyxy} & 0 & 0 & T_{yyyx} \\ 0 & 0 & 0 & 0 & 0 & T_{zzxy} & 0 & 0 & T_{zzyx} \\ 0 & 0 & 0 & 0 & T_{yzzx} & 0 & 0 & T_{yzxz} & 0 \\ 0 & 0 & 0 & T_{zxyz} & 0 & 0 & T_{zxzy} & 0 & 0 \\ T_{xyxx} & T_{xyyy} & T_{xyzz} & 0 & 0 & 0 & 0 & 0 & 0 \end{bmatrix}
\end{align*}
\begin{align*}
& T_{xxxy} = - 2 M_{faz}^{(1)} - M_{faz}^{(2)} + 2 M_{fbz}^{(1)} + M_{fbz}^{(2)} + 2 M_{pz}^{(1)} + M_{pz}^{(3)} + T_{dxy}^{(1)} + 2 T_{dxy}^{(2)} + T_{dxy}^{(3)} - 2 T_{dxy}^{(5)} + T_{gaz}^{(1)} - T_{gbz}^{(1)} \\
& T_{xxyx} = - 2 M_{faz}^{(1)} + M_{faz}^{(2)} + 2 M_{fbz}^{(1)} - M_{fbz}^{(2)} + 2 M_{pz}^{(1)} - M_{pz}^{(3)} + T_{dxy}^{(1)} + 2 T_{dxy}^{(2)} + T_{dxy}^{(3)} + 2 T_{dxy}^{(5)} + T_{gaz}^{(1)} - T_{gbz}^{(1)} \\
& T_{yyxy} = 2 M_{faz}^{(1)} - M_{faz}^{(2)} + 2 M_{fbz}^{(1)} - M_{fbz}^{(2)} - 2 M_{pz}^{(1)} + M_{pz}^{(3)} + T_{dxy}^{(1)} + 2 T_{dxy}^{(2)} + T_{dxy}^{(3)} + 2 T_{dxy}^{(5)} - T_{gaz}^{(1)} - T_{gbz}^{(1)} \\
& T_{yyyx} = 2 M_{faz}^{(1)} + M_{faz}^{(2)} + 2 M_{fbz}^{(1)} + M_{fbz}^{(2)} - 2 M_{pz}^{(1)} - M_{pz}^{(3)} + T_{dxy}^{(1)} + 2 T_{dxy}^{(2)} + T_{dxy}^{(3)} - 2 T_{dxy}^{(5)} - T_{gaz}^{(1)} - T_{gbz}^{(1)} \\
& T_{zzxy} = 2 M_{faz}^{(2)} - 4 M_{fbz}^{(1)} + M_{pz}^{(3)} + 2 M_{pz}^{(4)} + T_{dxy}^{(1)} + T_{dxy}^{(3)} + 2 T_{gbz}^{(1)} \\
& T_{zzyx} = - 2 M_{faz}^{(2)} - 4 M_{fbz}^{(1)} - M_{pz}^{(3)} - 2 M_{pz}^{(4)} + T_{dxy}^{(1)} + T_{dxy}^{(3)} + 2 T_{gbz}^{(1)} \\
& T_{yzzx} = - 4 M_{faz}^{(1)} - M_{faz}^{(2)} - M_{fbz}^{(2)} - M_{pz}^{(1)} + M_{pz}^{(4)} + T_{dxy}^{(2)} - T_{dxy}^{(5)} + 2 T_{gbz}^{(1)} \\
& T_{yzxz} = - 4 M_{faz}^{(1)} + M_{faz}^{(2)} + M_{fbz}^{(2)} - M_{pz}^{(1)} - M_{pz}^{(4)} + T_{dxy}^{(2)} + T_{dxy}^{(5)} + 2 T_{gbz}^{(1)} \\
& T_{zxyz} = 4 M_{faz}^{(1)} - M_{faz}^{(2)} + M_{fbz}^{(2)} + M_{pz}^{(1)} + M_{pz}^{(4)} + T_{dxy}^{(2)} + T_{dxy}^{(5)} + 2 T_{gbz}^{(1)} \\
& T_{zxzy} = 4 M_{faz}^{(1)} + M_{faz}^{(2)} - M_{fbz}^{(2)} + M_{pz}^{(1)} - M_{pz}^{(4)} + T_{dxy}^{(2)} - T_{dxy}^{(5)} + 2 T_{gbz}^{(1)} \\
& T_{xyxx} = 2 M_{faz}^{(1)} - 2 M_{fbz}^{(1)} - 2 M_{pz}^{(1)} + T_{dxy}^{(1)} + 2 T_{dxy}^{(2)} - T_{dxy}^{(3)} + T_{gaz}^{(1)} - T_{gbz}^{(1)} \\
& T_{xyyy} = - 2 M_{faz}^{(1)} - 2 M_{fbz}^{(1)} + 2 M_{pz}^{(1)} + T_{dxy}^{(1)} + 2 T_{dxy}^{(2)} - T_{dxy}^{(3)} - T_{gaz}^{(1)} - T_{gbz}^{(1)} \\
& T_{xyzz} = 4 M_{fbz}^{(1)} + T_{dxy}^{(1)} - T_{dxy}^{(3)} + 2 T_{gbz}^{(1)}
\end{align*}
* Rank 4 tensor (a).
\begin{align*}
\begin{bmatrix} 0 & 0 & 0 & 0 & T_{yzzx} & 0 & 0 & T_{yzxz} & 0 \\ 0 & 0 & 0 & T_{zxyz} & 0 & 0 & T_{zxzy} & 0 & 0 \\ T_{xyxx} & T_{xyyy} & T_{xyzz} & 0 & 0 & 0 & 0 & 0 & 0 \end{bmatrix}
\end{align*}
\begin{align*}
& T_{yzzx} = - M_{faz}^{(3)} + M_{fbz}^{(3)} - M_{pz}^{(2)} + M_{pz}^{(6)} + 2 T_{dxy}^{(4)} + T_{dxy}^{(6)} \\
& T_{yzxz} = - M_{faz}^{(3)} + M_{fbz}^{(3)} + M_{pz}^{(2)} + M_{pz}^{(6)} - 2 T_{dxy}^{(4)} + T_{dxy}^{(6)} \\
& T_{zxyz} = - M_{faz}^{(3)} - M_{fbz}^{(3)} + M_{pz}^{(2)} + M_{pz}^{(6)} + 2 T_{dxy}^{(4)} - T_{dxy}^{(6)} \\
& T_{zxzy} = - M_{faz}^{(3)} - M_{fbz}^{(3)} - M_{pz}^{(2)} + M_{pz}^{(6)} - 2 T_{dxy}^{(4)} - T_{dxy}^{(6)} \\
& T_{xyxx} = - M_{faz}^{(3)} + M_{fbz}^{(3)} + M_{pz}^{(5)} - 2 T_{dxy}^{(6)} \\
& T_{xyyy} = - M_{faz}^{(3)} - M_{fbz}^{(3)} + M_{pz}^{(5)} + 2 T_{dxy}^{(6)} \\
& T_{xyzz} = 2 M_{faz}^{(3)} + M_{pz}^{(5)} + 2 M_{pz}^{(6)}
\end{align*}
* Rank 4 tensor (t).
\begin{align*}
\begin{bmatrix} 0 & T_{xxxy} & 0 \\ T_{yyyx} & 0 & 0 \\ 0 & 0 & 0 \\ 0 & 0 & 0 \\ 0 & T_{zzxy} & 0 \\ T_{xxyx} & 0 & 0 \\ T_{yzzx} & 0 & 0 \\ 0 & 0 & 0 \\ 0 & T_{xyyy} & 0 \\ 0 & 0 & \frac{T_{xxxy}}{2} - \frac{T_{xxyx}}{2} + T_{xyyy} - T_{yyyx} + T_{zzxy} \end{bmatrix}
\end{align*}
\begin{align*}
& T_{xxxy} = T_{dxy}^{(1)} + 2 T_{dxy}^{(2)} + T_{dxy}^{(3)} - 2 T_{dxy}^{(5)} + T_{gaz}^{(1)} - T_{gbz}^{(1)} \\
& T_{yyyx} = T_{dxy}^{(1)} + 2 T_{dxy}^{(2)} + T_{dxy}^{(3)} - 2 T_{dxy}^{(5)} - T_{gaz}^{(1)} - T_{gbz}^{(1)} \\
& T_{zzxy} = T_{dxy}^{(1)} + T_{dxy}^{(3)} + 2 T_{gbz}^{(1)} \\
& T_{xxyx} = T_{dxy}^{(1)} + 2 T_{dxy}^{(2)} + T_{dxy}^{(3)} + 2 T_{dxy}^{(5)} + T_{gaz}^{(1)} - T_{gbz}^{(1)} \\
& T_{yzzx} = T_{dxy}^{(2)} - T_{dxy}^{(5)} + 2 T_{gbz}^{(1)} \\
& T_{xyyy} = T_{dxy}^{(1)} + 2 T_{dxy}^{(2)} - T_{dxy}^{(3)} - T_{gaz}^{(1)} - T_{gbz}^{(1)}
\end{align*}

\end{document}
