\documentclass[fleqn,8pt,landscape]{jsarticle}
\special{papersize=\the\paperwidth,\the\paperheight}

%%% package

\usepackage[usenames]{color}
\usepackage{amsmath}
\usepackage{breqn}
\usepackage{graphicx}
\usepackage{amssymb}
\usepackage{bm}
\usepackage{enumitem}
\usepackage{braket}
\usepackage{multirow}
\usepackage{booktabs}
\usepackage{longtable}

%%% layout setting

\paperwidth=356.4truemm
\paperheight=252.0truemm
\textwidth=335.59999999999997truemm
\textheight=224.2truemm
\oddsidemargin=-15truemm
\topmargin=-15truemm
\footskip=7truemm

%%% fixed

\hoffset=0truemm
\voffset=0truemm
\headheight=0truemm
\headsep=0truemm
\marginparsep=0truemm
\marginparwidth=0truemm

%%% main text

\begin{document}

\setcounter{MaxMatrixCols}{32}

\renewcommand{\tablename}{Table~}
\renewcommand{\figurename}{Figure~}
\begin{center}
\LARGE
MPG No. 34.3.140\quad$32'$\quad(312' setting)\quad[ Type III, trigonal ] [M tensor]
\end{center}
* Rank 0 tensor.
* Rank 1 tensor.
\begin{align*}
\begin{bmatrix} 0 & 0 & M_{z} \end{bmatrix}
\end{align*}
\begin{align*}
& M_{z} = M_{pz}^{(1)}
\end{align*}
* Rank 2 tensor (s).
* Rank 2 tensor (a).
\begin{align*}
\begin{bmatrix} 0 & M_{xy} & 0 \\ - M_{xy} & 0 & 0 \\ 0 & 0 & 0 \end{bmatrix}
\end{align*}
\begin{align*}
& M_{xy} = T_{pz}^{(1)}
\end{align*}
* Rank 3 tensor (s).
\begin{align*}
\begin{bmatrix} M_{xxx} & 0 & M_{xxz} \\ - M_{xxx} & 0 & M_{xxz} \\ 0 & 0 & M_{zzz} \\ 0 & M_{yzy} & 0 \\ M_{yzy} & 0 & 0 \\ 0 & - M_{xxx} & 0 \end{bmatrix}
\end{align*}
\begin{align*}
& M_{xxx} = M_{f2}^{(1)} \\
& M_{xxz} = - M_{faz}^{(1)} + M_{pz}^{(1)} \\
& M_{zzz} = 2 M_{faz}^{(1)} + M_{pz}^{(1)} + 2 M_{pz}^{(2)} \\
& M_{yzy} = - M_{faz}^{(1)} + M_{pz}^{(2)}
\end{align*}
* Rank 3 tensor (a).
\begin{align*}
\begin{bmatrix} 0 & M_{yzy} & 0 \\ - M_{yzy} & 0 & 0 \\ 0 & 0 & 0 \end{bmatrix}
\end{align*}
\begin{align*}
& M_{yzy} = M_{pz}^{(3)}
\end{align*}
* Rank 4 tensor (sss).
\begin{align*}
\begin{bmatrix} 0 & 0 & 0 & M_{xxyz} & 0 & 0 \\ 0 & 0 & 0 & - M_{xxyz} & 0 & 0 \\ 0 & 0 & 0 & 0 & 0 & 0 \\ M_{xxyz} & - M_{xxyz} & 0 & 0 & 0 & 0 \\ 0 & 0 & 0 & 0 & 0 & M_{xxyz} \\ 0 & 0 & 0 & 0 & M_{xxyz} & 0 \end{bmatrix}
\end{align*}
\begin{align*}
& M_{xxyz} = M_{gb}^{(1)}
\end{align*}
* Rank 4 tensor (ssa).
\begin{align*}
\begin{bmatrix} 0 & 0 & 0 & M_{xxyz} & 0 & M_{xxxy} \\ 0 & 0 & 0 & - M_{xxyz} & 0 & - M_{xxxy} \\ 0 & 0 & 0 & 0 & 0 & 0 \\ - M_{xxyz} & M_{xxyz} & 0 & 0 & M_{yzzx} & 0 \\ 0 & 0 & 0 & - M_{yzzx} & 0 & - M_{xxyz} \\ - M_{xxxy} & M_{xxxy} & 0 & 0 & M_{xxyz} & 0 \end{bmatrix}
\end{align*}
\begin{align*}
& M_{xxyz} = 2 T_{f2}^{(1)} \\
& M_{xxxy} = - 2 T_{faz}^{(1)} + 2 T_{pz}^{(1)} \\
& M_{yzzx} = - 4 T_{faz}^{(1)} - T_{pz}^{(1)}
\end{align*}
* Rank 4 tensor (aas).
* Rank 4 tensor (aaa).
\begin{align*}
\begin{bmatrix} 0 & M_{yzzx} & 0 \\ - M_{yzzx} & 0 & 0 \\ 0 & 0 & 0 \end{bmatrix}
\end{align*}
\begin{align*}
& M_{yzzx} = - T_{pz}^{(2)}
\end{align*}
* Rank 4 tensor (sa).
\begin{align*}
\begin{bmatrix} M_{xxyz} & 0 & M_{xxxy} \\ - M_{xxyz} & 0 & M_{xxxy} \\ 0 & 0 & M_{zzxy} \\ 0 & M_{yzzx} & 0 \\ M_{yzzx} & 0 & 0 \\ 0 & - M_{xxyz} & 0 \end{bmatrix}
\end{align*}
\begin{align*}
& M_{xxyz} = T_{f2}^{(2)} \\
& M_{xxxy} = - T_{faz}^{(2)} + T_{pz}^{(3)} \\
& M_{zzxy} = 2 T_{faz}^{(2)} + T_{pz}^{(3)} + 2 T_{pz}^{(4)} \\
& M_{yzzx} = - T_{faz}^{(2)} + T_{pz}^{(4)}
\end{align*}
* Rank 4 tensor (as).
\begin{align*}
\begin{bmatrix} M_{yzxx} & - M_{yzxx} & 0 & 0 & M_{yzzx} & 0 \\ 0 & 0 & 0 & M_{yzzx} & 0 & - M_{yzxx} \\ M_{xyxx} & M_{xyxx} & M_{xyzz} & 0 & 0 & 0 \end{bmatrix}
\end{align*}
\begin{align*}
& M_{yzxx} = T_{f2}^{(3)} \\
& M_{yzzx} = - T_{faz}^{(3)} + T_{pz}^{(6)} \\
& M_{xyxx} = - T_{faz}^{(3)} + T_{pz}^{(5)} \\
& M_{xyzz} = 2 T_{faz}^{(3)} + T_{pz}^{(5)} + 2 T_{pz}^{(6)}
\end{align*}
* Rank 4 tensor (s).
\begin{align*}
\begin{bmatrix} 0 & 0 & 0 & M_{xxyz} & 0 & M_{xxxy} & M_{xxzy} & 0 & M_{xxyx} \\ 0 & 0 & 0 & - M_{xxyz} & 0 & - M_{xxyx} & - M_{xxzy} & 0 & - M_{xxxy} \\ 0 & 0 & 0 & 0 & 0 & M_{zzxy} & 0 & 0 & - M_{zzxy} \\ M_{yzxx} & - M_{yzxx} & 0 & 0 & M_{yzzx} & 0 & 0 & M_{yzxz} & 0 \\ 0 & 0 & 0 & - M_{yzxz} & 0 & M_{yzxx} & - M_{yzzx} & 0 & M_{yzxx} \\ - \frac{M_{xxxy}}{2} - \frac{M_{xxyx}}{2} & \frac{M_{xxxy}}{2} + \frac{M_{xxyx}}{2} & 0 & 0 & M_{xxzy} & 0 & 0 & M_{xxyz} & 0 \end{bmatrix}
\end{align*}
\begin{align*}
& M_{xxyz} = M_{gb}^{(1)} + 2 T_{f2}^{(1)} + T_{f2}^{(2)} \\
& M_{xxxy} = - 2 T_{faz}^{(1)} - T_{faz}^{(2)} + 2 T_{pz}^{(1)} + T_{pz}^{(3)} \\
& M_{xxzy} = M_{gb}^{(1)} + 2 T_{f2}^{(1)} - T_{f2}^{(2)} \\
& M_{xxyx} = - 2 T_{faz}^{(1)} + T_{faz}^{(2)} + 2 T_{pz}^{(1)} - T_{pz}^{(3)} \\
& M_{zzxy} = 2 T_{faz}^{(2)} + T_{pz}^{(3)} + 2 T_{pz}^{(4)} \\
& M_{yzxx} = M_{gb}^{(1)} - 2 T_{f2}^{(1)} \\
& M_{yzzx} = - 4 T_{faz}^{(1)} - T_{faz}^{(2)} - T_{pz}^{(1)} + T_{pz}^{(4)} \\
& M_{yzxz} = - 4 T_{faz}^{(1)} + T_{faz}^{(2)} - T_{pz}^{(1)} - T_{pz}^{(4)}
\end{align*}
* Rank 4 tensor (a).
\begin{align*}
\begin{bmatrix} M_{yzxx} & - M_{yzxx} & 0 & 0 & M_{yzzx} & 0 & 0 & M_{yzxz} & 0 \\ 0 & 0 & 0 & M_{yzxz} & 0 & - M_{yzxx} & M_{yzzx} & 0 & - M_{yzxx} \\ M_{xyxx} & M_{xyxx} & M_{xyzz} & 0 & 0 & 0 & 0 & 0 & 0 \end{bmatrix}
\end{align*}
\begin{align*}
& M_{yzxx} = T_{f2}^{(3)} \\
& M_{yzzx} = - T_{faz}^{(3)} - T_{pz}^{(2)} + T_{pz}^{(6)} \\
& M_{yzxz} = - T_{faz}^{(3)} + T_{pz}^{(2)} + T_{pz}^{(6)} \\
& M_{xyxx} = - T_{faz}^{(3)} + T_{pz}^{(5)} \\
& M_{xyzz} = 2 T_{faz}^{(3)} + T_{pz}^{(5)} + 2 T_{pz}^{(6)}
\end{align*}
* Rank 4 tensor (t).
\begin{align*}
\begin{bmatrix} 0 & 0 & 0 \\ 0 & 0 & M_{yyyz} \\ 0 & 0 & 0 \\ 0 & M_{yyyz} & 0 \\ 0 & 0 & 0 \\ 0 & 0 & - M_{yyyz} \\ 0 & 0 & 0 \\ 0 & - M_{yyyz} & 0 \\ 0 & 0 & 0 \\ - M_{yyyz} & 0 & 0 \end{bmatrix}
\end{align*}
\begin{align*}
& M_{yyyz} = - M_{gb}^{(1)}
\end{align*}

\end{document}
