\documentclass[fleqn,8pt,landscape]{jsarticle}
\special{papersize=\the\paperwidth,\the\paperheight}

%%% package

\usepackage[usenames]{color}
\usepackage{amsmath}
\usepackage{breqn}
\usepackage{graphicx}
\usepackage{amssymb}
\usepackage{bm}
\usepackage{enumitem}
\usepackage{braket}
\usepackage{multirow}
\usepackage{booktabs}
\usepackage{longtable}

%%% layout setting

\paperwidth=356.4truemm
\paperheight=252.0truemm
\textwidth=335.59999999999997truemm
\textheight=224.2truemm
\oddsidemargin=-15truemm
\topmargin=-15truemm
\footskip=7truemm

%%% fixed

\hoffset=0truemm
\voffset=0truemm
\headheight=0truemm
\headsep=0truemm
\marginparsep=0truemm
\marginparwidth=0truemm

%%% main text

\begin{document}

\setcounter{MaxMatrixCols}{32}

\renewcommand{\tablename}{Table~}
\renewcommand{\figurename}{Figure~}
\begin{center}
\LARGE
MPG No. 6.1.17\quad$222$\quad[ Type I, orthorhombic ] [T tensor]
\end{center}
* Rank 0 tensor.
\begin{align*}
\begin{bmatrix} T \end{bmatrix}
\end{align*}
\begin{align*}
& T = T_{s}^{(1)}
\end{align*}
* Rank 1 tensor.
* Rank 2 tensor (s).
\begin{align*}
\begin{bmatrix} T_{xx} & 0 & 0 \\ 0 & T_{yy} & 0 \\ 0 & 0 & T_{zz} \end{bmatrix}
\end{align*}
\begin{align*}
& T_{xx} = - T_{du}^{(1)} + T_{dv}^{(1)} + T_{s}^{(1)} \\
& T_{yy} = - T_{du}^{(1)} - T_{dv}^{(1)} + T_{s}^{(1)} \\
& T_{zz} = 2 T_{du}^{(1)} + T_{s}^{(1)}
\end{align*}
* Rank 2 tensor (a).
* Rank 3 tensor (s).
\begin{align*}
\begin{bmatrix} 0 & 0 & 0 \\ 0 & 0 & 0 \\ 0 & 0 & 0 \\ T_{yzx} & 0 & 0 \\ 0 & T_{zxy} & 0 \\ 0 & 0 & T_{xyz} \end{bmatrix}
\end{align*}
\begin{align*}
& T_{yzx} = - 3 M_{du}^{(1)} - M_{dv}^{(1)} + T_{f3}^{(1)} \\
& T_{zxy} = 3 M_{du}^{(1)} - M_{dv}^{(1)} + T_{f3}^{(1)} \\
& T_{xyz} = 2 M_{dv}^{(1)} + T_{f3}^{(1)}
\end{align*}
* Rank 3 tensor (a).
\begin{align*}
\begin{bmatrix} T_{yzx} & 0 & 0 \\ 0 & T_{zxy} & 0 \\ 0 & 0 & T_{xyz} \end{bmatrix}
\end{align*}
\begin{align*}
& T_{yzx} = - M_{du}^{(2)} + M_{dv}^{(2)} + M_{s}^{(1)} \\
& T_{zxy} = - M_{du}^{(2)} - M_{dv}^{(2)} + M_{s}^{(1)} \\
& T_{xyz} = 2 M_{du}^{(2)} + M_{s}^{(1)}
\end{align*}
* Rank 4 tensor (sss).
\begin{align*}
\begin{bmatrix} T_{xxxx} & T_{xxyy} & T_{xxzz} & 0 & 0 & 0 \\ T_{xxyy} & T_{yyyy} & T_{yyzz} & 0 & 0 & 0 \\ T_{xxzz} & T_{yyzz} & T_{zzzz} & 0 & 0 & 0 \\ 0 & 0 & 0 & T_{yzyz} & 0 & 0 \\ 0 & 0 & 0 & 0 & T_{zxzx} & 0 \\ 0 & 0 & 0 & 0 & 0 & T_{xyxy} \end{bmatrix}
\end{align*}
\begin{align*}
& T_{xxxx} = - 2 T_{du}^{(1)} - 4 T_{du}^{(2)} + 2 T_{dv}^{(1)} + 4 T_{dv}^{(2)} - T_{gu}^{(1)} + T_{gv}^{(1)} + 2 T_{g}^{(1)} + T_{s}^{(1)} + 2 T_{s}^{(2)} \\
& T_{xxyy} = - 2 T_{du}^{(1)} + 2 T_{gu}^{(1)} - T_{g}^{(1)} + T_{s}^{(1)} \\
& T_{xxzz} = T_{du}^{(1)} + T_{dv}^{(1)} - T_{gu}^{(1)} - T_{gv}^{(1)} - T_{g}^{(1)} + T_{s}^{(1)} \\
& T_{yyyy} = - 2 T_{du}^{(1)} - 4 T_{du}^{(2)} - 2 T_{dv}^{(1)} - 4 T_{dv}^{(2)} - T_{gu}^{(1)} - T_{gv}^{(1)} + 2 T_{g}^{(1)} + T_{s}^{(1)} + 2 T_{s}^{(2)} \\
& T_{yyzz} = T_{du}^{(1)} - T_{dv}^{(1)} - T_{gu}^{(1)} + T_{gv}^{(1)} - T_{g}^{(1)} + T_{s}^{(1)} \\
& T_{zzzz} = 4 T_{du}^{(1)} + 8 T_{du}^{(2)} + 2 T_{gu}^{(1)} + 2 T_{g}^{(1)} + T_{s}^{(1)} + 2 T_{s}^{(2)} \\
& T_{yzyz} = T_{du}^{(2)} - T_{dv}^{(2)} - T_{gu}^{(1)} + T_{gv}^{(1)} - T_{g}^{(1)} + T_{s}^{(2)} \\
& T_{zxzx} = T_{du}^{(2)} + T_{dv}^{(2)} - T_{gu}^{(1)} - T_{gv}^{(1)} - T_{g}^{(1)} + T_{s}^{(2)} \\
& T_{xyxy} = - 2 T_{du}^{(2)} + 2 T_{gu}^{(1)} - T_{g}^{(1)} + T_{s}^{(2)}
\end{align*}
* Rank 4 tensor (ssa).
\begin{align*}
\begin{bmatrix} 0 & T_{xxyy} & T_{xxzz} & 0 & 0 & 0 \\ - T_{xxyy} & 0 & T_{yyzz} & 0 & 0 & 0 \\ - T_{xxzz} & - T_{yyzz} & 0 & 0 & 0 & 0 \\ 0 & 0 & 0 & 0 & 0 & 0 \\ 0 & 0 & 0 & 0 & 0 & 0 \\ 0 & 0 & 0 & 0 & 0 & 0 \end{bmatrix}
\end{align*}
\begin{align*}
& T_{xxyy} = 4 M_{f3}^{(1)} - 2 T_{dv}^{(3)} \\
& T_{xxzz} = - 4 M_{f3}^{(1)} + 3 T_{du}^{(3)} - T_{dv}^{(3)} \\
& T_{yyzz} = 4 M_{f3}^{(1)} + 3 T_{du}^{(3)} + T_{dv}^{(3)}
\end{align*}
* Rank 4 tensor (aas).
\begin{align*}
\begin{bmatrix} T_{yzyz} & 0 & 0 \\ 0 & T_{zxzx} & 0 \\ 0 & 0 & T_{xyxy} \end{bmatrix}
\end{align*}
\begin{align*}
& T_{yzyz} = - 2 T_{du}^{(4)} + 2 T_{dv}^{(4)} + T_{s}^{(3)} \\
& T_{zxzx} = - 2 T_{du}^{(4)} - 2 T_{dv}^{(4)} + T_{s}^{(3)} \\
& T_{xyxy} = 4 T_{du}^{(4)} + T_{s}^{(3)}
\end{align*}
* Rank 4 tensor (aaa).
* Rank 4 tensor (sa).
\begin{align*}
\begin{bmatrix} 0 & 0 & 0 \\ 0 & 0 & 0 \\ 0 & 0 & 0 \\ T_{yzyz} & 0 & 0 \\ 0 & T_{zxzx} & 0 \\ 0 & 0 & T_{xyxy} \end{bmatrix}
\end{align*}
\begin{align*}
& T_{yzyz} = M_{f3}^{(2)} - 3 T_{du}^{(5)} - T_{dv}^{(5)} \\
& T_{zxzx} = M_{f3}^{(2)} + 3 T_{du}^{(5)} - T_{dv}^{(5)} \\
& T_{xyxy} = M_{f3}^{(2)} + 2 T_{dv}^{(5)}
\end{align*}
* Rank 4 tensor (as).
\begin{align*}
\begin{bmatrix} 0 & 0 & 0 & T_{yzyz} & 0 & 0 \\ 0 & 0 & 0 & 0 & T_{zxzx} & 0 \\ 0 & 0 & 0 & 0 & 0 & T_{xyxy} \end{bmatrix}
\end{align*}
\begin{align*}
& T_{yzyz} = M_{f3}^{(3)} - 3 T_{du}^{(6)} - T_{dv}^{(6)} \\
& T_{zxzx} = M_{f3}^{(3)} + 3 T_{du}^{(6)} - T_{dv}^{(6)} \\
& T_{xyxy} = M_{f3}^{(3)} + 2 T_{dv}^{(6)}
\end{align*}
* Rank 4 tensor (s).
\begin{align*}
\begin{bmatrix} T_{xxxx} & T_{xxyy} & T_{xxzz} & 0 & 0 & 0 & 0 & 0 & 0 \\ T_{yyxx} & T_{yyyy} & T_{yyzz} & 0 & 0 & 0 & 0 & 0 & 0 \\ T_{zzxx} & T_{zzyy} & T_{zzzz} & 0 & 0 & 0 & 0 & 0 & 0 \\ 0 & 0 & 0 & T_{yzyz} & 0 & 0 & T_{yzzy} & 0 & 0 \\ 0 & 0 & 0 & 0 & T_{zxzx} & 0 & 0 & T_{zxxz} & 0 \\ 0 & 0 & 0 & 0 & 0 & T_{xyxy} & 0 & 0 & T_{xyyx} \end{bmatrix}
\end{align*}
\begin{align*}
& T_{xxxx} = - 2 T_{du}^{(1)} - 4 T_{du}^{(2)} + 2 T_{dv}^{(1)} + 4 T_{dv}^{(2)} - T_{gu}^{(1)} + T_{gv}^{(1)} + 2 T_{g}^{(1)} + T_{s}^{(1)} + 2 T_{s}^{(2)} \\
& T_{xxyy} = 4 M_{f3}^{(1)} - 2 T_{du}^{(1)} - 2 T_{dv}^{(3)} + 2 T_{gu}^{(1)} - T_{g}^{(1)} + T_{s}^{(1)} \\
& T_{xxzz} = - 4 M_{f3}^{(1)} + T_{du}^{(1)} + 3 T_{du}^{(3)} + T_{dv}^{(1)} - T_{dv}^{(3)} - T_{gu}^{(1)} - T_{gv}^{(1)} - T_{g}^{(1)} + T_{s}^{(1)} \\
& T_{yyxx} = - 4 M_{f3}^{(1)} - 2 T_{du}^{(1)} + 2 T_{dv}^{(3)} + 2 T_{gu}^{(1)} - T_{g}^{(1)} + T_{s}^{(1)} \\
& T_{yyyy} = - 2 T_{du}^{(1)} - 4 T_{du}^{(2)} - 2 T_{dv}^{(1)} - 4 T_{dv}^{(2)} - T_{gu}^{(1)} - T_{gv}^{(1)} + 2 T_{g}^{(1)} + T_{s}^{(1)} + 2 T_{s}^{(2)} \\
& T_{yyzz} = 4 M_{f3}^{(1)} + T_{du}^{(1)} + 3 T_{du}^{(3)} - T_{dv}^{(1)} + T_{dv}^{(3)} - T_{gu}^{(1)} + T_{gv}^{(1)} - T_{g}^{(1)} + T_{s}^{(1)} \\
& T_{zzxx} = 4 M_{f3}^{(1)} + T_{du}^{(1)} - 3 T_{du}^{(3)} + T_{dv}^{(1)} + T_{dv}^{(3)} - T_{gu}^{(1)} - T_{gv}^{(1)} - T_{g}^{(1)} + T_{s}^{(1)} \\
& T_{zzyy} = - 4 M_{f3}^{(1)} + T_{du}^{(1)} - 3 T_{du}^{(3)} - T_{dv}^{(1)} - T_{dv}^{(3)} - T_{gu}^{(1)} + T_{gv}^{(1)} - T_{g}^{(1)} + T_{s}^{(1)} \\
& T_{zzzz} = 4 T_{du}^{(1)} + 8 T_{du}^{(2)} + 2 T_{gu}^{(1)} + 2 T_{g}^{(1)} + T_{s}^{(1)} + 2 T_{s}^{(2)} \\
& T_{yzyz} = M_{f3}^{(2)} + T_{du}^{(2)} - 3 T_{du}^{(5)} - T_{dv}^{(2)} - T_{dv}^{(5)} - T_{gu}^{(1)} + T_{gv}^{(1)} - T_{g}^{(1)} + T_{s}^{(2)} \\
& T_{yzzy} = - M_{f3}^{(2)} + T_{du}^{(2)} + 3 T_{du}^{(5)} - T_{dv}^{(2)} + T_{dv}^{(5)} - T_{gu}^{(1)} + T_{gv}^{(1)} - T_{g}^{(1)} + T_{s}^{(2)} \\
& T_{zxzx} = M_{f3}^{(2)} + T_{du}^{(2)} + 3 T_{du}^{(5)} + T_{dv}^{(2)} - T_{dv}^{(5)} - T_{gu}^{(1)} - T_{gv}^{(1)} - T_{g}^{(1)} + T_{s}^{(2)} \\
& T_{zxxz} = - M_{f3}^{(2)} + T_{du}^{(2)} - 3 T_{du}^{(5)} + T_{dv}^{(2)} + T_{dv}^{(5)} - T_{gu}^{(1)} - T_{gv}^{(1)} - T_{g}^{(1)} + T_{s}^{(2)} \\
& T_{xyxy} = M_{f3}^{(2)} - 2 T_{du}^{(2)} + 2 T_{dv}^{(5)} + 2 T_{gu}^{(1)} - T_{g}^{(1)} + T_{s}^{(2)} \\
& T_{xyyx} = - M_{f3}^{(2)} - 2 T_{du}^{(2)} - 2 T_{dv}^{(5)} + 2 T_{gu}^{(1)} - T_{g}^{(1)} + T_{s}^{(2)}
\end{align*}
* Rank 4 tensor (a).
\begin{align*}
\begin{bmatrix} 0 & 0 & 0 & T_{yzyz} & 0 & 0 & T_{yzzy} & 0 & 0 \\ 0 & 0 & 0 & 0 & T_{zxzx} & 0 & 0 & T_{zxxz} & 0 \\ 0 & 0 & 0 & 0 & 0 & T_{xyxy} & 0 & 0 & T_{xyyx} \end{bmatrix}
\end{align*}
\begin{align*}
& T_{yzyz} = M_{f3}^{(3)} - 2 T_{du}^{(4)} - 3 T_{du}^{(6)} + 2 T_{dv}^{(4)} - T_{dv}^{(6)} + T_{s}^{(3)} \\
& T_{yzzy} = M_{f3}^{(3)} + 2 T_{du}^{(4)} - 3 T_{du}^{(6)} - 2 T_{dv}^{(4)} - T_{dv}^{(6)} - T_{s}^{(3)} \\
& T_{zxzx} = M_{f3}^{(3)} - 2 T_{du}^{(4)} + 3 T_{du}^{(6)} - 2 T_{dv}^{(4)} - T_{dv}^{(6)} + T_{s}^{(3)} \\
& T_{zxxz} = M_{f3}^{(3)} + 2 T_{du}^{(4)} + 3 T_{du}^{(6)} + 2 T_{dv}^{(4)} - T_{dv}^{(6)} - T_{s}^{(3)} \\
& T_{xyxy} = M_{f3}^{(3)} + 4 T_{du}^{(4)} + 2 T_{dv}^{(6)} + T_{s}^{(3)} \\
& T_{xyyx} = M_{f3}^{(3)} - 4 T_{du}^{(4)} + 2 T_{dv}^{(6)} - T_{s}^{(3)}
\end{align*}
* Rank 4 tensor (t).
\begin{align*}
\begin{bmatrix} T_{xxxx} & 0 & 0 \\ 0 & T_{yyyy} & 0 \\ 0 & 0 & T_{zzzz} \\ 0 & 0 & T_{yyzz} \\ T_{zzxx} & 0 & 0 \\ 0 & T_{xxyy} & 0 \\ 0 & T_{yzzy} & 0 \\ 0 & 0 & T_{zxxz} \\ T_{xxyy} + T_{yyzz} - T_{yzzy} - T_{zxxz} + T_{zzxx} & 0 & 0 \\ 0 & 0 & 0 \end{bmatrix}
\end{align*}
\begin{align*}
& T_{xxxx} = - 2 T_{du}^{(1)} - 4 T_{du}^{(2)} + 2 T_{dv}^{(1)} + 4 T_{dv}^{(2)} - T_{gu}^{(1)} + T_{gv}^{(1)} + 2 T_{g}^{(1)} + 3 T_{s}^{(1)} \\
& T_{yyyy} = - 2 T_{du}^{(1)} - 4 T_{du}^{(2)} - 2 T_{dv}^{(1)} - 4 T_{dv}^{(2)} - T_{gu}^{(1)} - T_{gv}^{(1)} + 2 T_{g}^{(1)} + 3 T_{s}^{(1)} \\
& T_{zzzz} = 4 T_{du}^{(1)} + 8 T_{du}^{(2)} + 2 T_{gu}^{(1)} + 2 T_{g}^{(1)} + 3 T_{s}^{(1)} \\
& T_{yyzz} = T_{du}^{(1)} + 3 T_{du}^{(3)} - T_{dv}^{(1)} + T_{dv}^{(3)} - T_{gu}^{(1)} + T_{gv}^{(1)} - T_{g}^{(1)} + T_{s}^{(1)} \\
& T_{zzxx} = T_{du}^{(1)} - 3 T_{du}^{(3)} + T_{dv}^{(1)} + T_{dv}^{(3)} - T_{gu}^{(1)} - T_{gv}^{(1)} - T_{g}^{(1)} + T_{s}^{(1)} \\
& T_{xxyy} = - 2 T_{du}^{(1)} - 2 T_{dv}^{(3)} + 2 T_{gu}^{(1)} - T_{g}^{(1)} + T_{s}^{(1)} \\
& T_{yzzy} = T_{du}^{(2)} + 3 T_{du}^{(5)} - T_{dv}^{(2)} + T_{dv}^{(5)} - T_{gu}^{(1)} + T_{gv}^{(1)} - T_{g}^{(1)} + T_{s}^{(1)} \\
& T_{zxxz} = T_{du}^{(2)} - 3 T_{du}^{(5)} + T_{dv}^{(2)} + T_{dv}^{(5)} - T_{gu}^{(1)} - T_{gv}^{(1)} - T_{g}^{(1)} + T_{s}^{(1)}
\end{align*}

\end{document}
