\documentclass[fleqn,8pt,landscape]{jsarticle}
\special{papersize=\the\paperwidth,\the\paperheight}

%%% package

\usepackage[usenames]{color}
\usepackage{amsmath}
\usepackage{breqn}
\usepackage{graphicx}
\usepackage{amssymb}
\usepackage{bm}
\usepackage{enumitem}
\usepackage{braket}
\usepackage{multirow}
\usepackage{booktabs}
\usepackage{longtable}

%%% layout setting

\paperwidth=356.4truemm
\paperheight=252.0truemm
\textwidth=335.59999999999997truemm
\textheight=224.2truemm
\oddsidemargin=-15truemm
\topmargin=-15truemm
\footskip=7truemm

%%% fixed

\hoffset=0truemm
\voffset=0truemm
\headheight=0truemm
\headsep=0truemm
\marginparsep=0truemm
\marginparwidth=0truemm

%%% main text

\begin{document}

\setcounter{MaxMatrixCols}{32}

\renewcommand{\tablename}{Table~}
\renewcommand{\figurename}{Figure~}
\begin{center}
\LARGE
MPG No. 6.1.17\quad$222$\quad[ Type I, orthorhombic ] [M tensor]
\end{center}
* Rank 0 tensor.
\begin{align*}
\begin{bmatrix} M \end{bmatrix}
\end{align*}
\begin{align*}
& M = M_{s}^{(1)}
\end{align*}
* Rank 1 tensor.
* Rank 2 tensor (s).
\begin{align*}
\begin{bmatrix} M_{xx} & 0 & 0 \\ 0 & M_{yy} & 0 \\ 0 & 0 & M_{zz} \end{bmatrix}
\end{align*}
\begin{align*}
& M_{xx} = - M_{du}^{(1)} + M_{dv}^{(1)} + M_{s}^{(1)} \\
& M_{yy} = - M_{du}^{(1)} - M_{dv}^{(1)} + M_{s}^{(1)} \\
& M_{zz} = 2 M_{du}^{(1)} + M_{s}^{(1)}
\end{align*}
* Rank 2 tensor (a).
* Rank 3 tensor (s).
\begin{align*}
\begin{bmatrix} 0 & 0 & 0 \\ 0 & 0 & 0 \\ 0 & 0 & 0 \\ M_{yzx} & 0 & 0 \\ 0 & M_{zxy} & 0 \\ 0 & 0 & M_{xyz} \end{bmatrix}
\end{align*}
\begin{align*}
& M_{yzx} = M_{f3}^{(1)} - 3 T_{du}^{(1)} - T_{dv}^{(1)} \\
& M_{zxy} = M_{f3}^{(1)} + 3 T_{du}^{(1)} - T_{dv}^{(1)} \\
& M_{xyz} = M_{f3}^{(1)} + 2 T_{dv}^{(1)}
\end{align*}
* Rank 3 tensor (a).
\begin{align*}
\begin{bmatrix} M_{yzx} & 0 & 0 \\ 0 & M_{zxy} & 0 \\ 0 & 0 & M_{xyz} \end{bmatrix}
\end{align*}
\begin{align*}
& M_{yzx} = - T_{du}^{(2)} + T_{dv}^{(2)} + T_{s}^{(1)} \\
& M_{zxy} = - T_{du}^{(2)} - T_{dv}^{(2)} + T_{s}^{(1)} \\
& M_{xyz} = 2 T_{du}^{(2)} + T_{s}^{(1)}
\end{align*}
* Rank 4 tensor (sss).
\begin{align*}
\begin{bmatrix} M_{xxxx} & M_{xxyy} & M_{xxzz} & 0 & 0 & 0 \\ M_{xxyy} & M_{yyyy} & M_{yyzz} & 0 & 0 & 0 \\ M_{xxzz} & M_{yyzz} & M_{zzzz} & 0 & 0 & 0 \\ 0 & 0 & 0 & M_{yzyz} & 0 & 0 \\ 0 & 0 & 0 & 0 & M_{zxzx} & 0 \\ 0 & 0 & 0 & 0 & 0 & M_{xyxy} \end{bmatrix}
\end{align*}
\begin{align*}
& M_{xxxx} = - 2 M_{du}^{(1)} - 4 M_{du}^{(2)} + 2 M_{dv}^{(1)} + 4 M_{dv}^{(2)} - M_{gu}^{(1)} + M_{gv}^{(1)} + 2 M_{g}^{(1)} + M_{s}^{(1)} + 2 M_{s}^{(2)} \\
& M_{xxyy} = - 2 M_{du}^{(1)} + 2 M_{gu}^{(1)} - M_{g}^{(1)} + M_{s}^{(1)} \\
& M_{xxzz} = M_{du}^{(1)} + M_{dv}^{(1)} - M_{gu}^{(1)} - M_{gv}^{(1)} - M_{g}^{(1)} + M_{s}^{(1)} \\
& M_{yyyy} = - 2 M_{du}^{(1)} - 4 M_{du}^{(2)} - 2 M_{dv}^{(1)} - 4 M_{dv}^{(2)} - M_{gu}^{(1)} - M_{gv}^{(1)} + 2 M_{g}^{(1)} + M_{s}^{(1)} + 2 M_{s}^{(2)} \\
& M_{yyzz} = M_{du}^{(1)} - M_{dv}^{(1)} - M_{gu}^{(1)} + M_{gv}^{(1)} - M_{g}^{(1)} + M_{s}^{(1)} \\
& M_{zzzz} = 4 M_{du}^{(1)} + 8 M_{du}^{(2)} + 2 M_{gu}^{(1)} + 2 M_{g}^{(1)} + M_{s}^{(1)} + 2 M_{s}^{(2)} \\
& M_{yzyz} = M_{du}^{(2)} - M_{dv}^{(2)} - M_{gu}^{(1)} + M_{gv}^{(1)} - M_{g}^{(1)} + M_{s}^{(2)} \\
& M_{zxzx} = M_{du}^{(2)} + M_{dv}^{(2)} - M_{gu}^{(1)} - M_{gv}^{(1)} - M_{g}^{(1)} + M_{s}^{(2)} \\
& M_{xyxy} = - 2 M_{du}^{(2)} + 2 M_{gu}^{(1)} - M_{g}^{(1)} + M_{s}^{(2)}
\end{align*}
* Rank 4 tensor (ssa).
\begin{align*}
\begin{bmatrix} 0 & M_{xxyy} & M_{xxzz} & 0 & 0 & 0 \\ - M_{xxyy} & 0 & M_{yyzz} & 0 & 0 & 0 \\ - M_{xxzz} & - M_{yyzz} & 0 & 0 & 0 & 0 \\ 0 & 0 & 0 & 0 & 0 & 0 \\ 0 & 0 & 0 & 0 & 0 & 0 \\ 0 & 0 & 0 & 0 & 0 & 0 \end{bmatrix}
\end{align*}
\begin{align*}
& M_{xxyy} = - 2 M_{dv}^{(3)} + 4 T_{f3}^{(1)} \\
& M_{xxzz} = 3 M_{du}^{(3)} - M_{dv}^{(3)} - 4 T_{f3}^{(1)} \\
& M_{yyzz} = 3 M_{du}^{(3)} + M_{dv}^{(3)} + 4 T_{f3}^{(1)}
\end{align*}
* Rank 4 tensor (aas).
\begin{align*}
\begin{bmatrix} M_{yzyz} & 0 & 0 \\ 0 & M_{zxzx} & 0 \\ 0 & 0 & M_{xyxy} \end{bmatrix}
\end{align*}
\begin{align*}
& M_{yzyz} = - 2 M_{du}^{(4)} + 2 M_{dv}^{(4)} + M_{s}^{(3)} \\
& M_{zxzx} = - 2 M_{du}^{(4)} - 2 M_{dv}^{(4)} + M_{s}^{(3)} \\
& M_{xyxy} = 4 M_{du}^{(4)} + M_{s}^{(3)}
\end{align*}
* Rank 4 tensor (aaa).
* Rank 4 tensor (sa).
\begin{align*}
\begin{bmatrix} 0 & 0 & 0 \\ 0 & 0 & 0 \\ 0 & 0 & 0 \\ M_{yzyz} & 0 & 0 \\ 0 & M_{zxzx} & 0 \\ 0 & 0 & M_{xyxy} \end{bmatrix}
\end{align*}
\begin{align*}
& M_{yzyz} = - 3 M_{du}^{(5)} - M_{dv}^{(5)} + T_{f3}^{(2)} \\
& M_{zxzx} = 3 M_{du}^{(5)} - M_{dv}^{(5)} + T_{f3}^{(2)} \\
& M_{xyxy} = 2 M_{dv}^{(5)} + T_{f3}^{(2)}
\end{align*}
* Rank 4 tensor (as).
\begin{align*}
\begin{bmatrix} 0 & 0 & 0 & M_{yzyz} & 0 & 0 \\ 0 & 0 & 0 & 0 & M_{zxzx} & 0 \\ 0 & 0 & 0 & 0 & 0 & M_{xyxy} \end{bmatrix}
\end{align*}
\begin{align*}
& M_{yzyz} = - 3 M_{du}^{(6)} - M_{dv}^{(6)} + T_{f3}^{(3)} \\
& M_{zxzx} = 3 M_{du}^{(6)} - M_{dv}^{(6)} + T_{f3}^{(3)} \\
& M_{xyxy} = 2 M_{dv}^{(6)} + T_{f3}^{(3)}
\end{align*}
* Rank 4 tensor (s).
\begin{align*}
\begin{bmatrix} M_{xxxx} & M_{xxyy} & M_{xxzz} & 0 & 0 & 0 & 0 & 0 & 0 \\ M_{yyxx} & M_{yyyy} & M_{yyzz} & 0 & 0 & 0 & 0 & 0 & 0 \\ M_{zzxx} & M_{zzyy} & M_{zzzz} & 0 & 0 & 0 & 0 & 0 & 0 \\ 0 & 0 & 0 & M_{yzyz} & 0 & 0 & M_{yzzy} & 0 & 0 \\ 0 & 0 & 0 & 0 & M_{zxzx} & 0 & 0 & M_{zxxz} & 0 \\ 0 & 0 & 0 & 0 & 0 & M_{xyxy} & 0 & 0 & M_{xyyx} \end{bmatrix}
\end{align*}
\begin{align*}
& M_{xxxx} = - 2 M_{du}^{(1)} - 4 M_{du}^{(2)} + 2 M_{dv}^{(1)} + 4 M_{dv}^{(2)} - M_{gu}^{(1)} + M_{gv}^{(1)} + 2 M_{g}^{(1)} + M_{s}^{(1)} + 2 M_{s}^{(2)} \\
& M_{xxyy} = - 2 M_{du}^{(1)} - 2 M_{dv}^{(3)} + 2 M_{gu}^{(1)} - M_{g}^{(1)} + M_{s}^{(1)} + 4 T_{f3}^{(1)} \\
& M_{xxzz} = M_{du}^{(1)} + 3 M_{du}^{(3)} + M_{dv}^{(1)} - M_{dv}^{(3)} - M_{gu}^{(1)} - M_{gv}^{(1)} - M_{g}^{(1)} + M_{s}^{(1)} - 4 T_{f3}^{(1)} \\
& M_{yyxx} = - 2 M_{du}^{(1)} + 2 M_{dv}^{(3)} + 2 M_{gu}^{(1)} - M_{g}^{(1)} + M_{s}^{(1)} - 4 T_{f3}^{(1)} \\
& M_{yyyy} = - 2 M_{du}^{(1)} - 4 M_{du}^{(2)} - 2 M_{dv}^{(1)} - 4 M_{dv}^{(2)} - M_{gu}^{(1)} - M_{gv}^{(1)} + 2 M_{g}^{(1)} + M_{s}^{(1)} + 2 M_{s}^{(2)} \\
& M_{yyzz} = M_{du}^{(1)} + 3 M_{du}^{(3)} - M_{dv}^{(1)} + M_{dv}^{(3)} - M_{gu}^{(1)} + M_{gv}^{(1)} - M_{g}^{(1)} + M_{s}^{(1)} + 4 T_{f3}^{(1)} \\
& M_{zzxx} = M_{du}^{(1)} - 3 M_{du}^{(3)} + M_{dv}^{(1)} + M_{dv}^{(3)} - M_{gu}^{(1)} - M_{gv}^{(1)} - M_{g}^{(1)} + M_{s}^{(1)} + 4 T_{f3}^{(1)} \\
& M_{zzyy} = M_{du}^{(1)} - 3 M_{du}^{(3)} - M_{dv}^{(1)} - M_{dv}^{(3)} - M_{gu}^{(1)} + M_{gv}^{(1)} - M_{g}^{(1)} + M_{s}^{(1)} - 4 T_{f3}^{(1)} \\
& M_{zzzz} = 4 M_{du}^{(1)} + 8 M_{du}^{(2)} + 2 M_{gu}^{(1)} + 2 M_{g}^{(1)} + M_{s}^{(1)} + 2 M_{s}^{(2)} \\
& M_{yzyz} = M_{du}^{(2)} - 3 M_{du}^{(5)} - M_{dv}^{(2)} - M_{dv}^{(5)} - M_{gu}^{(1)} + M_{gv}^{(1)} - M_{g}^{(1)} + M_{s}^{(2)} + T_{f3}^{(2)} \\
& M_{yzzy} = M_{du}^{(2)} + 3 M_{du}^{(5)} - M_{dv}^{(2)} + M_{dv}^{(5)} - M_{gu}^{(1)} + M_{gv}^{(1)} - M_{g}^{(1)} + M_{s}^{(2)} - T_{f3}^{(2)} \\
& M_{zxzx} = M_{du}^{(2)} + 3 M_{du}^{(5)} + M_{dv}^{(2)} - M_{dv}^{(5)} - M_{gu}^{(1)} - M_{gv}^{(1)} - M_{g}^{(1)} + M_{s}^{(2)} + T_{f3}^{(2)} \\
& M_{zxxz} = M_{du}^{(2)} - 3 M_{du}^{(5)} + M_{dv}^{(2)} + M_{dv}^{(5)} - M_{gu}^{(1)} - M_{gv}^{(1)} - M_{g}^{(1)} + M_{s}^{(2)} - T_{f3}^{(2)} \\
& M_{xyxy} = - 2 M_{du}^{(2)} + 2 M_{dv}^{(5)} + 2 M_{gu}^{(1)} - M_{g}^{(1)} + M_{s}^{(2)} + T_{f3}^{(2)} \\
& M_{xyyx} = - 2 M_{du}^{(2)} - 2 M_{dv}^{(5)} + 2 M_{gu}^{(1)} - M_{g}^{(1)} + M_{s}^{(2)} - T_{f3}^{(2)}
\end{align*}
* Rank 4 tensor (a).
\begin{align*}
\begin{bmatrix} 0 & 0 & 0 & M_{yzyz} & 0 & 0 & M_{yzzy} & 0 & 0 \\ 0 & 0 & 0 & 0 & M_{zxzx} & 0 & 0 & M_{zxxz} & 0 \\ 0 & 0 & 0 & 0 & 0 & M_{xyxy} & 0 & 0 & M_{xyyx} \end{bmatrix}
\end{align*}
\begin{align*}
& M_{yzyz} = - 2 M_{du}^{(4)} - 3 M_{du}^{(6)} + 2 M_{dv}^{(4)} - M_{dv}^{(6)} + M_{s}^{(3)} + T_{f3}^{(3)} \\
& M_{yzzy} = 2 M_{du}^{(4)} - 3 M_{du}^{(6)} - 2 M_{dv}^{(4)} - M_{dv}^{(6)} - M_{s}^{(3)} + T_{f3}^{(3)} \\
& M_{zxzx} = - 2 M_{du}^{(4)} + 3 M_{du}^{(6)} - 2 M_{dv}^{(4)} - M_{dv}^{(6)} + M_{s}^{(3)} + T_{f3}^{(3)} \\
& M_{zxxz} = 2 M_{du}^{(4)} + 3 M_{du}^{(6)} + 2 M_{dv}^{(4)} - M_{dv}^{(6)} - M_{s}^{(3)} + T_{f3}^{(3)} \\
& M_{xyxy} = 4 M_{du}^{(4)} + 2 M_{dv}^{(6)} + M_{s}^{(3)} + T_{f3}^{(3)} \\
& M_{xyyx} = - 4 M_{du}^{(4)} + 2 M_{dv}^{(6)} - M_{s}^{(3)} + T_{f3}^{(3)}
\end{align*}
* Rank 4 tensor (t).
\begin{align*}
\begin{bmatrix} M_{xxxx} & 0 & 0 \\ 0 & M_{yyyy} & 0 \\ 0 & 0 & M_{zzzz} \\ 0 & 0 & M_{yyzz} \\ M_{zzxx} & 0 & 0 \\ 0 & M_{xxyy} & 0 \\ 0 & M_{yzzy} & 0 \\ 0 & 0 & M_{zxxz} \\ M_{xxyy} + M_{yyzz} - M_{yzzy} - M_{zxxz} + M_{zzxx} & 0 & 0 \\ 0 & 0 & 0 \end{bmatrix}
\end{align*}
\begin{align*}
& M_{xxxx} = - 2 M_{du}^{(1)} - 4 M_{du}^{(2)} + 2 M_{dv}^{(1)} + 4 M_{dv}^{(2)} - M_{gu}^{(1)} + M_{gv}^{(1)} + 2 M_{g}^{(1)} + 3 M_{s}^{(1)} \\
& M_{yyyy} = - 2 M_{du}^{(1)} - 4 M_{du}^{(2)} - 2 M_{dv}^{(1)} - 4 M_{dv}^{(2)} - M_{gu}^{(1)} - M_{gv}^{(1)} + 2 M_{g}^{(1)} + 3 M_{s}^{(1)} \\
& M_{zzzz} = 4 M_{du}^{(1)} + 8 M_{du}^{(2)} + 2 M_{gu}^{(1)} + 2 M_{g}^{(1)} + 3 M_{s}^{(1)} \\
& M_{yyzz} = M_{du}^{(1)} + 3 M_{du}^{(3)} - M_{dv}^{(1)} + M_{dv}^{(3)} - M_{gu}^{(1)} + M_{gv}^{(1)} - M_{g}^{(1)} + M_{s}^{(1)} \\
& M_{zzxx} = M_{du}^{(1)} - 3 M_{du}^{(3)} + M_{dv}^{(1)} + M_{dv}^{(3)} - M_{gu}^{(1)} - M_{gv}^{(1)} - M_{g}^{(1)} + M_{s}^{(1)} \\
& M_{xxyy} = - 2 M_{du}^{(1)} - 2 M_{dv}^{(3)} + 2 M_{gu}^{(1)} - M_{g}^{(1)} + M_{s}^{(1)} \\
& M_{yzzy} = M_{du}^{(2)} + 3 M_{du}^{(5)} - M_{dv}^{(2)} + M_{dv}^{(5)} - M_{gu}^{(1)} + M_{gv}^{(1)} - M_{g}^{(1)} + M_{s}^{(1)} \\
& M_{zxxz} = M_{du}^{(2)} - 3 M_{du}^{(5)} + M_{dv}^{(2)} + M_{dv}^{(5)} - M_{gu}^{(1)} - M_{gv}^{(1)} - M_{g}^{(1)} + M_{s}^{(1)}
\end{align*}

\end{document}
