\documentclass[fleqn,8pt,landscape]{jsarticle}
\special{papersize=\the\paperwidth,\the\paperheight}

%%% package

\usepackage[usenames]{color}
\usepackage{amsmath}
\usepackage{breqn}
\usepackage{graphicx}
\usepackage{amssymb}
\usepackage{bm}
\usepackage{enumitem}
\usepackage{braket}
\usepackage{multirow}
\usepackage{booktabs}
\usepackage{longtable}

%%% layout setting

\paperwidth=356.4truemm
\paperheight=252.0truemm
\textwidth=335.59999999999997truemm
\textheight=224.2truemm
\oddsidemargin=-15truemm
\topmargin=-15truemm
\footskip=7truemm

%%% fixed

\hoffset=0truemm
\voffset=0truemm
\headheight=0truemm
\headsep=0truemm
\marginparsep=0truemm
\marginparwidth=0truemm

%%% main text

\begin{document}

\setcounter{MaxMatrixCols}{32}

\renewcommand{\tablename}{Table~}
\renewcommand{\figurename}{Figure~}
\begin{center}
\LARGE
MPG No. 7.5.124\quad$m'm2'$\quad(mm'2' setting)\quad[ Type III, orthorhombic ] [T tensor]
\end{center}
* Rank 0 tensor.
* Rank 1 tensor.
\begin{align*}
\begin{bmatrix} 0 & T_{y} & 0 \end{bmatrix}
\end{align*}
\begin{align*}
& T_{y} = T_{py}^{(1)}
\end{align*}
* Rank 2 tensor (s).
\begin{align*}
\begin{bmatrix} 0 & 0 & 0 \\ 0 & 0 & T_{yz} \\ 0 & T_{yz} & 0 \end{bmatrix}
\end{align*}
\begin{align*}
& T_{yz} = T_{dyz}^{(1)}
\end{align*}
* Rank 2 tensor (a).
\begin{align*}
\begin{bmatrix} 0 & 0 & 0 \\ 0 & 0 & T_{yz} \\ 0 & - T_{yz} & 0 \end{bmatrix}
\end{align*}
\begin{align*}
& T_{yz} = M_{px}^{(1)}
\end{align*}
* Rank 3 tensor (s).
\begin{align*}
\begin{bmatrix} 0 & T_{xxy} & 0 \\ 0 & T_{yyy} & 0 \\ 0 & T_{zzy} & 0 \\ 0 & 0 & T_{yzz} \\ 0 & 0 & 0 \\ T_{xyx} & 0 & 0 \end{bmatrix}
\end{align*}
\begin{align*}
& T_{xxy} = 2 M_{dxz}^{(1)} - T_{fay}^{(1)} - T_{fby}^{(1)} + T_{py}^{(1)} \\
& T_{yyy} = 2 T_{fay}^{(1)} + T_{py}^{(1)} + 2 T_{py}^{(2)} \\
& T_{zzy} = - 2 M_{dxz}^{(1)} - T_{fay}^{(1)} + T_{fby}^{(1)} + T_{py}^{(1)} \\
& T_{yzz} = M_{dxz}^{(1)} - T_{fay}^{(1)} + T_{fby}^{(1)} + T_{py}^{(2)} \\
& T_{xyx} = - M_{dxz}^{(1)} - T_{fay}^{(1)} - T_{fby}^{(1)} + T_{py}^{(2)}
\end{align*}
* Rank 3 tensor (a).
\begin{align*}
\begin{bmatrix} 0 & 0 & T_{yzz} \\ 0 & 0 & 0 \\ T_{xyx} & 0 & 0 \end{bmatrix}
\end{align*}
\begin{align*}
& T_{yzz} = M_{dxz}^{(2)} - T_{py}^{(3)} \\
& T_{xyx} = M_{dxz}^{(2)} + T_{py}^{(3)}
\end{align*}
* Rank 4 tensor (sss).
\begin{align*}
\begin{bmatrix} 0 & 0 & 0 & T_{xxyz} & 0 & 0 \\ 0 & 0 & 0 & T_{yyyz} & 0 & 0 \\ 0 & 0 & 0 & T_{zzyz} & 0 & 0 \\ T_{xxyz} & T_{yyyz} & T_{zzyz} & 0 & 0 & 0 \\ 0 & 0 & 0 & 0 & 0 & T_{zxxy} \\ 0 & 0 & 0 & 0 & T_{zxxy} & 0 \end{bmatrix}
\end{align*}
\begin{align*}
& T_{xxyz} = T_{dyz}^{(1)} + 2 T_{gbx}^{(1)} \\
& T_{yyyz} = T_{dyz}^{(1)} + 2 T_{dyz}^{(2)} + T_{gax}^{(1)} - T_{gbx}^{(1)} \\
& T_{zzyz} = T_{dyz}^{(1)} + 2 T_{dyz}^{(2)} - T_{gax}^{(1)} - T_{gbx}^{(1)} \\
& T_{zxxy} = T_{dyz}^{(2)} + 2 T_{gbx}^{(1)}
\end{align*}
* Rank 4 tensor (ssa).
\begin{align*}
\begin{bmatrix} 0 & 0 & 0 & T_{xxyz} & 0 & 0 \\ 0 & 0 & 0 & T_{yyyz} & 0 & 0 \\ 0 & 0 & 0 & T_{zzyz} & 0 & 0 \\ - T_{xxyz} & - T_{yyyz} & - T_{zzyz} & 0 & 0 & 0 \\ 0 & 0 & 0 & 0 & 0 & T_{zxxy} \\ 0 & 0 & 0 & 0 & - T_{zxxy} & 0 \end{bmatrix}
\end{align*}
\begin{align*}
& T_{xxyz} = - 4 M_{fbx}^{(1)} + T_{dyz}^{(3)} \\
& T_{yyyz} = - 2 M_{fax}^{(1)} + 2 M_{fbx}^{(1)} + 2 M_{px}^{(1)} + T_{dyz}^{(3)} \\
& T_{zzyz} = 2 M_{fax}^{(1)} + 2 M_{fbx}^{(1)} - 2 M_{px}^{(1)} + T_{dyz}^{(3)} \\
& T_{zxxy} = - 4 M_{fax}^{(1)} - M_{px}^{(1)}
\end{align*}
* Rank 4 tensor (aas).
\begin{align*}
\begin{bmatrix} 0 & 0 & 0 \\ 0 & 0 & T_{zxxy} \\ 0 & T_{zxxy} & 0 \end{bmatrix}
\end{align*}
\begin{align*}
& T_{zxxy} = 2 T_{dyz}^{(4)}
\end{align*}
* Rank 4 tensor (aaa).
\begin{align*}
\begin{bmatrix} 0 & 0 & 0 \\ 0 & 0 & T_{zxxy} \\ 0 & - T_{zxxy} & 0 \end{bmatrix}
\end{align*}
\begin{align*}
& T_{zxxy} = - M_{px}^{(2)}
\end{align*}
* Rank 4 tensor (sa).
\begin{align*}
\begin{bmatrix} T_{xxyz} & 0 & 0 \\ T_{yyyz} & 0 & 0 \\ T_{zzyz} & 0 & 0 \\ 0 & 0 & 0 \\ 0 & 0 & T_{zxxy} \\ 0 & T_{xyzx} & 0 \end{bmatrix}
\end{align*}
\begin{align*}
& T_{xxyz} = 2 M_{fax}^{(2)} + M_{px}^{(3)} + 2 M_{px}^{(4)} \\
& T_{yyyz} = - M_{fax}^{(2)} + M_{fbx}^{(2)} + M_{px}^{(3)} - 2 T_{dyz}^{(5)} \\
& T_{zzyz} = - M_{fax}^{(2)} - M_{fbx}^{(2)} + M_{px}^{(3)} + 2 T_{dyz}^{(5)} \\
& T_{zxxy} = - M_{fax}^{(2)} - M_{fbx}^{(2)} + M_{px}^{(4)} - T_{dyz}^{(5)} \\
& T_{xyzx} = - M_{fax}^{(2)} + M_{fbx}^{(2)} + M_{px}^{(4)} + T_{dyz}^{(5)}
\end{align*}
* Rank 4 tensor (as).
\begin{align*}
\begin{bmatrix} T_{yzxx} & T_{yzyy} & T_{yzzz} & 0 & 0 & 0 \\ 0 & 0 & 0 & 0 & 0 & T_{zxxy} \\ 0 & 0 & 0 & 0 & T_{xyzx} & 0 \end{bmatrix}
\end{align*}
\begin{align*}
& T_{yzxx} = 2 M_{fax}^{(3)} + M_{px}^{(5)} + 2 M_{px}^{(6)} \\
& T_{yzyy} = - M_{fax}^{(3)} + M_{fbx}^{(3)} + M_{px}^{(5)} - 2 T_{dyz}^{(6)} \\
& T_{yzzz} = - M_{fax}^{(3)} - M_{fbx}^{(3)} + M_{px}^{(5)} + 2 T_{dyz}^{(6)} \\
& T_{zxxy} = - M_{fax}^{(3)} + M_{fbx}^{(3)} + M_{px}^{(6)} + T_{dyz}^{(6)} \\
& T_{xyzx} = - M_{fax}^{(3)} - M_{fbx}^{(3)} + M_{px}^{(6)} - T_{dyz}^{(6)}
\end{align*}
* Rank 4 tensor (s).
\begin{align*}
\begin{bmatrix} 0 & 0 & 0 & T_{xxyz} & 0 & 0 & T_{xxzy} & 0 & 0 \\ 0 & 0 & 0 & T_{yyyz} & 0 & 0 & T_{yyzy} & 0 & 0 \\ 0 & 0 & 0 & T_{zzyz} & 0 & 0 & T_{zzzy} & 0 & 0 \\ T_{yzxx} & T_{yzyy} & T_{yzzz} & 0 & 0 & 0 & 0 & 0 & 0 \\ 0 & 0 & 0 & 0 & 0 & T_{zxxy} & 0 & 0 & T_{zxyx} \\ 0 & 0 & 0 & 0 & T_{xyzx} & 0 & 0 & T_{xyxz} & 0 \end{bmatrix}
\end{align*}
\begin{align*}
& T_{xxyz} = 2 M_{fax}^{(2)} - 4 M_{fbx}^{(1)} + M_{px}^{(3)} + 2 M_{px}^{(4)} + T_{dyz}^{(1)} + T_{dyz}^{(3)} + 2 T_{gbx}^{(1)} \\
& T_{xxzy} = - 2 M_{fax}^{(2)} - 4 M_{fbx}^{(1)} - M_{px}^{(3)} - 2 M_{px}^{(4)} + T_{dyz}^{(1)} + T_{dyz}^{(3)} + 2 T_{gbx}^{(1)} \\
& T_{yyyz} = - 2 M_{fax}^{(1)} - M_{fax}^{(2)} + 2 M_{fbx}^{(1)} + M_{fbx}^{(2)} + 2 M_{px}^{(1)} + M_{px}^{(3)} + T_{dyz}^{(1)} + 2 T_{dyz}^{(2)} + T_{dyz}^{(3)} - 2 T_{dyz}^{(5)} + T_{gax}^{(1)} - T_{gbx}^{(1)} \\
& T_{yyzy} = - 2 M_{fax}^{(1)} + M_{fax}^{(2)} + 2 M_{fbx}^{(1)} - M_{fbx}^{(2)} + 2 M_{px}^{(1)} - M_{px}^{(3)} + T_{dyz}^{(1)} + 2 T_{dyz}^{(2)} + T_{dyz}^{(3)} + 2 T_{dyz}^{(5)} + T_{gax}^{(1)} - T_{gbx}^{(1)} \\
& T_{zzyz} = 2 M_{fax}^{(1)} - M_{fax}^{(2)} + 2 M_{fbx}^{(1)} - M_{fbx}^{(2)} - 2 M_{px}^{(1)} + M_{px}^{(3)} + T_{dyz}^{(1)} + 2 T_{dyz}^{(2)} + T_{dyz}^{(3)} + 2 T_{dyz}^{(5)} - T_{gax}^{(1)} - T_{gbx}^{(1)} \\
& T_{zzzy} = 2 M_{fax}^{(1)} + M_{fax}^{(2)} + 2 M_{fbx}^{(1)} + M_{fbx}^{(2)} - 2 M_{px}^{(1)} - M_{px}^{(3)} + T_{dyz}^{(1)} + 2 T_{dyz}^{(2)} + T_{dyz}^{(3)} - 2 T_{dyz}^{(5)} - T_{gax}^{(1)} - T_{gbx}^{(1)} \\
& T_{yzxx} = 4 M_{fbx}^{(1)} + T_{dyz}^{(1)} - T_{dyz}^{(3)} + 2 T_{gbx}^{(1)} \\
& T_{yzyy} = 2 M_{fax}^{(1)} - 2 M_{fbx}^{(1)} - 2 M_{px}^{(1)} + T_{dyz}^{(1)} + 2 T_{dyz}^{(2)} - T_{dyz}^{(3)} + T_{gax}^{(1)} - T_{gbx}^{(1)} \\
& T_{yzzz} = - 2 M_{fax}^{(1)} - 2 M_{fbx}^{(1)} + 2 M_{px}^{(1)} + T_{dyz}^{(1)} + 2 T_{dyz}^{(2)} - T_{dyz}^{(3)} - T_{gax}^{(1)} - T_{gbx}^{(1)} \\
& T_{zxxy} = - 4 M_{fax}^{(1)} - M_{fax}^{(2)} - M_{fbx}^{(2)} - M_{px}^{(1)} + M_{px}^{(4)} + T_{dyz}^{(2)} - T_{dyz}^{(5)} + 2 T_{gbx}^{(1)} \\
& T_{zxyx} = - 4 M_{fax}^{(1)} + M_{fax}^{(2)} + M_{fbx}^{(2)} - M_{px}^{(1)} - M_{px}^{(4)} + T_{dyz}^{(2)} + T_{dyz}^{(5)} + 2 T_{gbx}^{(1)} \\
& T_{xyzx} = 4 M_{fax}^{(1)} - M_{fax}^{(2)} + M_{fbx}^{(2)} + M_{px}^{(1)} + M_{px}^{(4)} + T_{dyz}^{(2)} + T_{dyz}^{(5)} + 2 T_{gbx}^{(1)} \\
& T_{xyxz} = 4 M_{fax}^{(1)} + M_{fax}^{(2)} - M_{fbx}^{(2)} + M_{px}^{(1)} - M_{px}^{(4)} + T_{dyz}^{(2)} - T_{dyz}^{(5)} + 2 T_{gbx}^{(1)}
\end{align*}
* Rank 4 tensor (a).
\begin{align*}
\begin{bmatrix} T_{yzxx} & T_{yzyy} & T_{yzzz} & 0 & 0 & 0 & 0 & 0 & 0 \\ 0 & 0 & 0 & 0 & 0 & T_{zxxy} & 0 & 0 & T_{zxyx} \\ 0 & 0 & 0 & 0 & T_{xyzx} & 0 & 0 & T_{xyxz} & 0 \end{bmatrix}
\end{align*}
\begin{align*}
& T_{yzxx} = 2 M_{fax}^{(3)} + M_{px}^{(5)} + 2 M_{px}^{(6)} \\
& T_{yzyy} = - M_{fax}^{(3)} + M_{fbx}^{(3)} + M_{px}^{(5)} - 2 T_{dyz}^{(6)} \\
& T_{yzzz} = - M_{fax}^{(3)} - M_{fbx}^{(3)} + M_{px}^{(5)} + 2 T_{dyz}^{(6)} \\
& T_{zxxy} = - M_{fax}^{(3)} + M_{fbx}^{(3)} - M_{px}^{(2)} + M_{px}^{(6)} + 2 T_{dyz}^{(4)} + T_{dyz}^{(6)} \\
& T_{zxyx} = - M_{fax}^{(3)} + M_{fbx}^{(3)} + M_{px}^{(2)} + M_{px}^{(6)} - 2 T_{dyz}^{(4)} + T_{dyz}^{(6)} \\
& T_{xyzx} = - M_{fax}^{(3)} - M_{fbx}^{(3)} + M_{px}^{(2)} + M_{px}^{(6)} + 2 T_{dyz}^{(4)} - T_{dyz}^{(6)} \\
& T_{xyxz} = - M_{fax}^{(3)} - M_{fbx}^{(3)} - M_{px}^{(2)} + M_{px}^{(6)} - 2 T_{dyz}^{(4)} - T_{dyz}^{(6)}
\end{align*}
* Rank 4 tensor (t).
\begin{align*}
\begin{bmatrix} 0 & 0 & 0 \\ 0 & 0 & T_{yyyz} \\ 0 & T_{zzzy} & 0 \\ 0 & T_{yyzy} & 0 \\ 0 & 0 & 0 \\ 0 & 0 & T_{xxyz} \\ 0 & 0 & T_{yzzz} \\ 0 & T_{zxxy} & 0 \\ 0 & 0 & 0 \\ - \frac{T_{yyyz}}{2} + \frac{T_{yyzy}}{2} + T_{zxxy} & 0 & 0 \end{bmatrix}
\end{align*}
\begin{align*}
& T_{yyyz} = T_{dyz}^{(1)} + 2 T_{dyz}^{(2)} + T_{dyz}^{(3)} - 2 T_{dyz}^{(5)} + T_{gax}^{(1)} - T_{gbx}^{(1)} \\
& T_{zzzy} = T_{dyz}^{(1)} + 2 T_{dyz}^{(2)} + T_{dyz}^{(3)} - 2 T_{dyz}^{(5)} - T_{gax}^{(1)} - T_{gbx}^{(1)} \\
& T_{yyzy} = T_{dyz}^{(1)} + 2 T_{dyz}^{(2)} + T_{dyz}^{(3)} + 2 T_{dyz}^{(5)} + T_{gax}^{(1)} - T_{gbx}^{(1)} \\
& T_{xxyz} = T_{dyz}^{(1)} + T_{dyz}^{(3)} + 2 T_{gbx}^{(1)} \\
& T_{yzzz} = T_{dyz}^{(1)} + 2 T_{dyz}^{(2)} - T_{dyz}^{(3)} - T_{gax}^{(1)} - T_{gbx}^{(1)} \\
& T_{zxxy} = T_{dyz}^{(2)} - T_{dyz}^{(5)} + 2 T_{gbx}^{(1)}
\end{align*}

\end{document}
