\documentclass[fleqn,8pt,landscape]{jsarticle}
\special{papersize=\the\paperwidth,\the\paperheight}

%%% package

\usepackage[usenames]{color}
\usepackage{amsmath}
\usepackage{breqn}
\usepackage{graphicx}
\usepackage{amssymb}
\usepackage{bm}
\usepackage{enumitem}
\usepackage{braket}
\usepackage{multirow}
\usepackage{booktabs}
\usepackage{longtable}

%%% layout setting

\paperwidth=356.4truemm
\paperheight=252.0truemm
\textwidth=335.59999999999997truemm
\textheight=224.2truemm
\oddsidemargin=-15truemm
\topmargin=-15truemm
\footskip=7truemm

%%% fixed

\hoffset=0truemm
\voffset=0truemm
\headheight=0truemm
\headsep=0truemm
\marginparsep=0truemm
\marginparwidth=0truemm

%%% main text

\begin{document}

\setcounter{MaxMatrixCols}{32}

\renewcommand{\tablename}{Table~}
\renewcommand{\figurename}{Figure~}
\begin{center}
\LARGE
MPG No. 7.5.124\quad$m'm2'$\quad(mm'2' setting)\quad[ Type III, orthorhombic ] [M tensor]
\end{center}
* Rank 0 tensor.
* Rank 1 tensor.
\begin{align*}
\begin{bmatrix} M_{x} & 0 & 0 \end{bmatrix}
\end{align*}
\begin{align*}
& M_{x} = M_{px}^{(1)}
\end{align*}
* Rank 2 tensor (s).
\begin{align*}
\begin{bmatrix} 0 & 0 & M_{xz} \\ 0 & 0 & 0 \\ M_{xz} & 0 & 0 \end{bmatrix}
\end{align*}
\begin{align*}
& M_{xz} = M_{dxz}^{(1)}
\end{align*}
* Rank 2 tensor (a).
\begin{align*}
\begin{bmatrix} 0 & 0 & M_{xz} \\ 0 & 0 & 0 \\ - M_{xz} & 0 & 0 \end{bmatrix}
\end{align*}
\begin{align*}
& M_{xz} = - T_{py}^{(1)}
\end{align*}
* Rank 3 tensor (s).
\begin{align*}
\begin{bmatrix} M_{xxx} & 0 & 0 \\ M_{yyx} & 0 & 0 \\ M_{zzx} & 0 & 0 \\ 0 & 0 & 0 \\ 0 & 0 & M_{zxz} \\ 0 & M_{xyy} & 0 \end{bmatrix}
\end{align*}
\begin{align*}
& M_{xxx} = 2 M_{fax}^{(1)} + M_{px}^{(1)} + 2 M_{px}^{(2)} \\
& M_{yyx} = - M_{fax}^{(1)} + M_{fbx}^{(1)} + M_{px}^{(1)} - 2 T_{dyz}^{(1)} \\
& M_{zzx} = - M_{fax}^{(1)} - M_{fbx}^{(1)} + M_{px}^{(1)} + 2 T_{dyz}^{(1)} \\
& M_{zxz} = - M_{fax}^{(1)} - M_{fbx}^{(1)} + M_{px}^{(2)} - T_{dyz}^{(1)} \\
& M_{xyy} = - M_{fax}^{(1)} + M_{fbx}^{(1)} + M_{px}^{(2)} + T_{dyz}^{(1)}
\end{align*}
* Rank 3 tensor (a).
\begin{align*}
\begin{bmatrix} 0 & 0 & 0 \\ 0 & 0 & M_{zxz} \\ 0 & M_{xyy} & 0 \end{bmatrix}
\end{align*}
\begin{align*}
& M_{zxz} = M_{px}^{(3)} + T_{dyz}^{(2)} \\
& M_{xyy} = - M_{px}^{(3)} + T_{dyz}^{(2)}
\end{align*}
* Rank 4 tensor (sss).
\begin{align*}
\begin{bmatrix} 0 & 0 & 0 & 0 & M_{xxzx} & 0 \\ 0 & 0 & 0 & 0 & M_{yyzx} & 0 \\ 0 & 0 & 0 & 0 & M_{zzzx} & 0 \\ 0 & 0 & 0 & 0 & 0 & M_{yzxy} \\ M_{xxzx} & M_{yyzx} & M_{zzzx} & 0 & 0 & 0 \\ 0 & 0 & 0 & M_{yzxy} & 0 & 0 \end{bmatrix}
\end{align*}
\begin{align*}
& M_{xxzx} = M_{dxz}^{(1)} + 2 M_{dxz}^{(2)} - M_{gay}^{(1)} - M_{gby}^{(1)} \\
& M_{yyzx} = M_{dxz}^{(1)} + 2 M_{gby}^{(1)} \\
& M_{zzzx} = M_{dxz}^{(1)} + 2 M_{dxz}^{(2)} + M_{gay}^{(1)} - M_{gby}^{(1)} \\
& M_{yzxy} = M_{dxz}^{(2)} + 2 M_{gby}^{(1)}
\end{align*}
* Rank 4 tensor (ssa).
\begin{align*}
\begin{bmatrix} 0 & 0 & 0 & 0 & M_{xxzx} & 0 \\ 0 & 0 & 0 & 0 & M_{yyzx} & 0 \\ 0 & 0 & 0 & 0 & M_{zzzx} & 0 \\ 0 & 0 & 0 & 0 & 0 & M_{yzxy} \\ - M_{xxzx} & - M_{yyzx} & - M_{zzzx} & 0 & 0 & 0 \\ 0 & 0 & 0 & - M_{yzxy} & 0 & 0 \end{bmatrix}
\end{align*}
\begin{align*}
& M_{xxzx} = M_{dxz}^{(3)} + 2 T_{fay}^{(1)} + 2 T_{fby}^{(1)} - 2 T_{py}^{(1)} \\
& M_{yyzx} = M_{dxz}^{(3)} - 4 T_{fby}^{(1)} \\
& M_{zzzx} = M_{dxz}^{(3)} - 2 T_{fay}^{(1)} + 2 T_{fby}^{(1)} + 2 T_{py}^{(1)} \\
& M_{yzxy} = 4 T_{fay}^{(1)} + T_{py}^{(1)}
\end{align*}
* Rank 4 tensor (aas).
\begin{align*}
\begin{bmatrix} 0 & 0 & M_{yzxy} \\ 0 & 0 & 0 \\ M_{yzxy} & 0 & 0 \end{bmatrix}
\end{align*}
\begin{align*}
& M_{yzxy} = 2 M_{dxz}^{(4)}
\end{align*}
* Rank 4 tensor (aaa).
\begin{align*}
\begin{bmatrix} 0 & 0 & M_{yzxy} \\ 0 & 0 & 0 \\ - M_{yzxy} & 0 & 0 \end{bmatrix}
\end{align*}
\begin{align*}
& M_{yzxy} = T_{py}^{(2)}
\end{align*}
* Rank 4 tensor (sa).
\begin{align*}
\begin{bmatrix} 0 & M_{xxzx} & 0 \\ 0 & M_{yyzx} & 0 \\ 0 & M_{zzzx} & 0 \\ 0 & 0 & M_{yzxy} \\ 0 & 0 & 0 \\ M_{xyyz} & 0 & 0 \end{bmatrix}
\end{align*}
\begin{align*}
& M_{xxzx} = 2 M_{dxz}^{(5)} - T_{fay}^{(2)} - T_{fby}^{(2)} + T_{py}^{(3)} \\
& M_{yyzx} = 2 T_{fay}^{(2)} + T_{py}^{(3)} + 2 T_{py}^{(4)} \\
& M_{zzzx} = - 2 M_{dxz}^{(5)} - T_{fay}^{(2)} + T_{fby}^{(2)} + T_{py}^{(3)} \\
& M_{yzxy} = M_{dxz}^{(5)} - T_{fay}^{(2)} + T_{fby}^{(2)} + T_{py}^{(4)} \\
& M_{xyyz} = - M_{dxz}^{(5)} - T_{fay}^{(2)} - T_{fby}^{(2)} + T_{py}^{(4)}
\end{align*}
* Rank 4 tensor (as).
\begin{align*}
\begin{bmatrix} 0 & 0 & 0 & 0 & 0 & M_{yzxy} \\ M_{zxxx} & M_{zxyy} & M_{zxzz} & 0 & 0 & 0 \\ 0 & 0 & 0 & M_{xyyz} & 0 & 0 \end{bmatrix}
\end{align*}
\begin{align*}
& M_{yzxy} = - M_{dxz}^{(6)} - T_{fay}^{(3)} - T_{fby}^{(3)} + T_{py}^{(6)} \\
& M_{zxxx} = 2 M_{dxz}^{(6)} - T_{fay}^{(3)} - T_{fby}^{(3)} + T_{py}^{(5)} \\
& M_{zxyy} = 2 T_{fay}^{(3)} + T_{py}^{(5)} + 2 T_{py}^{(6)} \\
& M_{zxzz} = - 2 M_{dxz}^{(6)} - T_{fay}^{(3)} + T_{fby}^{(3)} + T_{py}^{(5)} \\
& M_{xyyz} = M_{dxz}^{(6)} - T_{fay}^{(3)} + T_{fby}^{(3)} + T_{py}^{(6)}
\end{align*}
* Rank 4 tensor (s).
\begin{align*}
\begin{bmatrix} 0 & 0 & 0 & 0 & M_{xxzx} & 0 & 0 & M_{xxxz} & 0 \\ 0 & 0 & 0 & 0 & M_{yyzx} & 0 & 0 & M_{yyxz} & 0 \\ 0 & 0 & 0 & 0 & M_{zzzx} & 0 & 0 & M_{zzxz} & 0 \\ 0 & 0 & 0 & 0 & 0 & M_{yzxy} & 0 & 0 & M_{yzyx} \\ M_{zxxx} & M_{zxyy} & M_{zxzz} & 0 & 0 & 0 & 0 & 0 & 0 \\ 0 & 0 & 0 & M_{xyyz} & 0 & 0 & M_{xyzy} & 0 & 0 \end{bmatrix}
\end{align*}
\begin{align*}
& M_{xxzx} = M_{dxz}^{(1)} + 2 M_{dxz}^{(2)} + M_{dxz}^{(3)} + 2 M_{dxz}^{(5)} - M_{gay}^{(1)} - M_{gby}^{(1)} + 2 T_{fay}^{(1)} - T_{fay}^{(2)} + 2 T_{fby}^{(1)} - T_{fby}^{(2)} - 2 T_{py}^{(1)} + T_{py}^{(3)} \\
& M_{xxxz} = M_{dxz}^{(1)} + 2 M_{dxz}^{(2)} + M_{dxz}^{(3)} - 2 M_{dxz}^{(5)} - M_{gay}^{(1)} - M_{gby}^{(1)} + 2 T_{fay}^{(1)} + T_{fay}^{(2)} + 2 T_{fby}^{(1)} + T_{fby}^{(2)} - 2 T_{py}^{(1)} - T_{py}^{(3)} \\
& M_{yyzx} = M_{dxz}^{(1)} + M_{dxz}^{(3)} + 2 M_{gby}^{(1)} + 2 T_{fay}^{(2)} - 4 T_{fby}^{(1)} + T_{py}^{(3)} + 2 T_{py}^{(4)} \\
& M_{yyxz} = M_{dxz}^{(1)} + M_{dxz}^{(3)} + 2 M_{gby}^{(1)} - 2 T_{fay}^{(2)} - 4 T_{fby}^{(1)} - T_{py}^{(3)} - 2 T_{py}^{(4)} \\
& M_{zzzx} = M_{dxz}^{(1)} + 2 M_{dxz}^{(2)} + M_{dxz}^{(3)} - 2 M_{dxz}^{(5)} + M_{gay}^{(1)} - M_{gby}^{(1)} - 2 T_{fay}^{(1)} - T_{fay}^{(2)} + 2 T_{fby}^{(1)} + T_{fby}^{(2)} + 2 T_{py}^{(1)} + T_{py}^{(3)} \\
& M_{zzxz} = M_{dxz}^{(1)} + 2 M_{dxz}^{(2)} + M_{dxz}^{(3)} + 2 M_{dxz}^{(5)} + M_{gay}^{(1)} - M_{gby}^{(1)} - 2 T_{fay}^{(1)} + T_{fay}^{(2)} + 2 T_{fby}^{(1)} - T_{fby}^{(2)} + 2 T_{py}^{(1)} - T_{py}^{(3)} \\
& M_{yzxy} = M_{dxz}^{(2)} + M_{dxz}^{(5)} + 2 M_{gby}^{(1)} + 4 T_{fay}^{(1)} - T_{fay}^{(2)} + T_{fby}^{(2)} + T_{py}^{(1)} + T_{py}^{(4)} \\
& M_{yzyx} = M_{dxz}^{(2)} - M_{dxz}^{(5)} + 2 M_{gby}^{(1)} + 4 T_{fay}^{(1)} + T_{fay}^{(2)} - T_{fby}^{(2)} + T_{py}^{(1)} - T_{py}^{(4)} \\
& M_{zxxx} = M_{dxz}^{(1)} + 2 M_{dxz}^{(2)} - M_{dxz}^{(3)} - M_{gay}^{(1)} - M_{gby}^{(1)} - 2 T_{fay}^{(1)} - 2 T_{fby}^{(1)} + 2 T_{py}^{(1)} \\
& M_{zxyy} = M_{dxz}^{(1)} - M_{dxz}^{(3)} + 2 M_{gby}^{(1)} + 4 T_{fby}^{(1)} \\
& M_{zxzz} = M_{dxz}^{(1)} + 2 M_{dxz}^{(2)} - M_{dxz}^{(3)} + M_{gay}^{(1)} - M_{gby}^{(1)} + 2 T_{fay}^{(1)} - 2 T_{fby}^{(1)} - 2 T_{py}^{(1)} \\
& M_{xyyz} = M_{dxz}^{(2)} - M_{dxz}^{(5)} + 2 M_{gby}^{(1)} - 4 T_{fay}^{(1)} - T_{fay}^{(2)} - T_{fby}^{(2)} - T_{py}^{(1)} + T_{py}^{(4)} \\
& M_{xyzy} = M_{dxz}^{(2)} + M_{dxz}^{(5)} + 2 M_{gby}^{(1)} - 4 T_{fay}^{(1)} + T_{fay}^{(2)} + T_{fby}^{(2)} - T_{py}^{(1)} - T_{py}^{(4)}
\end{align*}
* Rank 4 tensor (a).
\begin{align*}
\begin{bmatrix} 0 & 0 & 0 & 0 & 0 & M_{yzxy} & 0 & 0 & M_{yzyx} \\ M_{zxxx} & M_{zxyy} & M_{zxzz} & 0 & 0 & 0 & 0 & 0 & 0 \\ 0 & 0 & 0 & M_{xyyz} & 0 & 0 & M_{xyzy} & 0 & 0 \end{bmatrix}
\end{align*}
\begin{align*}
& M_{yzxy} = 2 M_{dxz}^{(4)} - M_{dxz}^{(6)} - T_{fay}^{(3)} - T_{fby}^{(3)} + T_{py}^{(2)} + T_{py}^{(6)} \\
& M_{yzyx} = - 2 M_{dxz}^{(4)} - M_{dxz}^{(6)} - T_{fay}^{(3)} - T_{fby}^{(3)} - T_{py}^{(2)} + T_{py}^{(6)} \\
& M_{zxxx} = 2 M_{dxz}^{(6)} - T_{fay}^{(3)} - T_{fby}^{(3)} + T_{py}^{(5)} \\
& M_{zxyy} = 2 T_{fay}^{(3)} + T_{py}^{(5)} + 2 T_{py}^{(6)} \\
& M_{zxzz} = - 2 M_{dxz}^{(6)} - T_{fay}^{(3)} + T_{fby}^{(3)} + T_{py}^{(5)} \\
& M_{xyyz} = 2 M_{dxz}^{(4)} + M_{dxz}^{(6)} - T_{fay}^{(3)} + T_{fby}^{(3)} - T_{py}^{(2)} + T_{py}^{(6)} \\
& M_{xyzy} = - 2 M_{dxz}^{(4)} + M_{dxz}^{(6)} - T_{fay}^{(3)} + T_{fby}^{(3)} + T_{py}^{(2)} + T_{py}^{(6)}
\end{align*}
* Rank 4 tensor (t).
\begin{align*}
\begin{bmatrix} 0 & 0 & M_{xxxz} \\ 0 & 0 & 0 \\ M_{zzzx} & 0 & 0 \\ M_{yyzx} & 0 & 0 \\ 0 & 0 & M_{zzxz} \\ 0 & 0 & 0 \\ 0 & 0 & 0 \\ M_{zxxx} & 0 & 0 \\ 0 & 0 & M_{xyyz} \\ 0 & M_{xyyz} + \frac{M_{zzxz}}{2} - \frac{M_{zzzx}}{2} & 0 \end{bmatrix}
\end{align*}
\begin{align*}
& M_{xxxz} = M_{dxz}^{(1)} + 2 M_{dxz}^{(2)} + M_{dxz}^{(3)} - 2 M_{dxz}^{(5)} - M_{gay}^{(1)} - M_{gby}^{(1)} \\
& M_{zzzx} = M_{dxz}^{(1)} + 2 M_{dxz}^{(2)} + M_{dxz}^{(3)} - 2 M_{dxz}^{(5)} + M_{gay}^{(1)} - M_{gby}^{(1)} \\
& M_{yyzx} = M_{dxz}^{(1)} + M_{dxz}^{(3)} + 2 M_{gby}^{(1)} \\
& M_{zzxz} = M_{dxz}^{(1)} + 2 M_{dxz}^{(2)} + M_{dxz}^{(3)} + 2 M_{dxz}^{(5)} + M_{gay}^{(1)} - M_{gby}^{(1)} \\
& M_{zxxx} = M_{dxz}^{(1)} + 2 M_{dxz}^{(2)} - M_{dxz}^{(3)} - M_{gay}^{(1)} - M_{gby}^{(1)} \\
& M_{xyyz} = M_{dxz}^{(2)} - M_{dxz}^{(5)} + 2 M_{gby}^{(1)}
\end{align*}

\end{document}
