\documentclass[fleqn,8pt,landscape]{jsarticle}
\special{papersize=\the\paperwidth,\the\paperheight}

%%% package

\usepackage[usenames]{color}
\usepackage{amsmath}
\usepackage{breqn}
\usepackage{graphicx}
\usepackage{amssymb}
\usepackage{bm}
\usepackage{enumitem}
\usepackage{braket}
\usepackage{multirow}
\usepackage{booktabs}
\usepackage{longtable}

%%% layout setting

\paperwidth=356.4truemm
\paperheight=252.0truemm
\textwidth=335.59999999999997truemm
\textheight=224.2truemm
\oddsidemargin=-15truemm
\topmargin=-15truemm
\footskip=7truemm

%%% fixed

\hoffset=0truemm
\voffset=0truemm
\headheight=0truemm
\headsep=0truemm
\marginparsep=0truemm
\marginparwidth=0truemm

%%% main text

\begin{document}

\setcounter{MaxMatrixCols}{32}

\renewcommand{\tablename}{Table~}
\renewcommand{\figurename}{Figure~}
\begin{center}
\LARGE
MPG No. 4.3.11\quad$m'$\quad[ Type III, monoclinic ] [G tensor]
\end{center}
* Rank 0 tensor.
* Rank 1 tensor.
\begin{align*}
\begin{bmatrix} 0 & G_{y} & 0 \end{bmatrix}
\end{align*}
\begin{align*}
& G_{y} = G_{py}^{(1)}
\end{align*}
* Rank 2 tensor (s).
\begin{align*}
\begin{bmatrix} 0 & G_{xy} & 0 \\ G_{xy} & 0 & G_{yz} \\ 0 & G_{yz} & 0 \end{bmatrix}
\end{align*}
\begin{align*}
& G_{xy} = G_{dxy}^{(1)} \\
& G_{yz} = G_{dyz}^{(1)}
\end{align*}
* Rank 2 tensor (a).
\begin{align*}
\begin{bmatrix} 0 & G_{xy} & 0 \\ - G_{xy} & 0 & G_{yz} \\ 0 & - G_{yz} & 0 \end{bmatrix}
\end{align*}
\begin{align*}
& G_{xy} = Q_{pz}^{(1)} \\
& G_{yz} = Q_{px}^{(1)}
\end{align*}
* Rank 3 tensor (s).
\begin{align*}
\begin{bmatrix} 0 & G_{xxy} & 0 \\ 0 & G_{yyy} & 0 \\ 0 & G_{zzy} & 0 \\ G_{yzx} & 0 & G_{yzz} \\ 0 & G_{zxy} & 0 \\ G_{xyx} & 0 & G_{xyz} \end{bmatrix}
\end{align*}
\begin{align*}
& G_{xxy} = - G_{fay}^{(1)} - G_{fby}^{(1)} + G_{py}^{(1)} + 2 Q_{dxz}^{(1)} \\
& G_{yyy} = 2 G_{fay}^{(1)} + G_{py}^{(1)} + 2 G_{py}^{(2)} \\
& G_{zzy} = - G_{fay}^{(1)} + G_{fby}^{(1)} + G_{py}^{(1)} - 2 Q_{dxz}^{(1)} \\
& G_{yzx} = G_{f3}^{(1)} - 3 Q_{du}^{(1)} - Q_{dv}^{(1)} \\
& G_{yzz} = - G_{fay}^{(1)} + G_{fby}^{(1)} + G_{py}^{(2)} + Q_{dxz}^{(1)} \\
& G_{zxy} = G_{f3}^{(1)} + 3 Q_{du}^{(1)} - Q_{dv}^{(1)} \\
& G_{xyx} = - G_{fay}^{(1)} - G_{fby}^{(1)} + G_{py}^{(2)} - Q_{dxz}^{(1)} \\
& G_{xyz} = G_{f3}^{(1)} + 2 Q_{dv}^{(1)}
\end{align*}
* Rank 3 tensor (a).
\begin{align*}
\begin{bmatrix} G_{yzx} & 0 & G_{yzz} \\ 0 & G_{zxy} & 0 \\ G_{xyx} & 0 & G_{xyz} \end{bmatrix}
\end{align*}
\begin{align*}
& G_{yzx} = - Q_{du}^{(2)} + Q_{dv}^{(2)} + Q_{s}^{(1)} \\
& G_{yzz} = - G_{py}^{(3)} + Q_{dxz}^{(2)} \\
& G_{zxy} = - Q_{du}^{(2)} - Q_{dv}^{(2)} + Q_{s}^{(1)} \\
& G_{xyx} = G_{py}^{(3)} + Q_{dxz}^{(2)} \\
& G_{xyz} = 2 Q_{du}^{(2)} + Q_{s}^{(1)}
\end{align*}
* Rank 4 tensor (sss).
\begin{align*}
\begin{bmatrix} 0 & 0 & 0 & G_{xxyz} & 0 & G_{xxxy} \\ 0 & 0 & 0 & G_{yyyz} & 0 & G_{yyxy} \\ 0 & 0 & 0 & G_{zzyz} & 0 & G_{zzxy} \\ G_{xxyz} & G_{yyyz} & G_{zzyz} & 0 & G_{yzzx} & 0 \\ 0 & 0 & 0 & G_{yzzx} & 0 & G_{zxxy} \\ G_{xxxy} & G_{yyxy} & G_{zzxy} & 0 & G_{zxxy} & 0 \end{bmatrix}
\end{align*}
\begin{align*}
& G_{xxyz} = G_{dyz}^{(1)} + 2 G_{gbx}^{(1)} \\
& G_{xxxy} = G_{dxy}^{(1)} + 2 G_{dxy}^{(2)} + G_{gaz}^{(1)} - G_{gbz}^{(1)} \\
& G_{yyyz} = G_{dyz}^{(1)} + 2 G_{dyz}^{(2)} + G_{gax}^{(1)} - G_{gbx}^{(1)} \\
& G_{yyxy} = G_{dxy}^{(1)} + 2 G_{dxy}^{(2)} - G_{gaz}^{(1)} - G_{gbz}^{(1)} \\
& G_{zzyz} = G_{dyz}^{(1)} + 2 G_{dyz}^{(2)} - G_{gax}^{(1)} - G_{gbx}^{(1)} \\
& G_{zzxy} = G_{dxy}^{(1)} + 2 G_{gbz}^{(1)} \\
& G_{yzzx} = G_{dxy}^{(2)} + 2 G_{gbz}^{(1)} \\
& G_{zxxy} = G_{dyz}^{(2)} + 2 G_{gbx}^{(1)}
\end{align*}
* Rank 4 tensor (ssa).
\begin{align*}
\begin{bmatrix} 0 & 0 & 0 & G_{xxyz} & 0 & G_{xxxy} \\ 0 & 0 & 0 & G_{yyyz} & 0 & G_{yyxy} \\ 0 & 0 & 0 & G_{zzyz} & 0 & G_{zzxy} \\ - G_{xxyz} & - G_{yyyz} & - G_{zzyz} & 0 & G_{yzzx} & 0 \\ 0 & 0 & 0 & - G_{yzzx} & 0 & G_{zxxy} \\ - G_{xxxy} & - G_{yyxy} & - G_{zzxy} & 0 & - G_{zxxy} & 0 \end{bmatrix}
\end{align*}
\begin{align*}
& G_{xxyz} = G_{dyz}^{(3)} - 4 Q_{fbx}^{(1)} \\
& G_{xxxy} = G_{dxy}^{(3)} - 2 Q_{faz}^{(1)} + 2 Q_{fbz}^{(1)} + 2 Q_{pz}^{(1)} \\
& G_{yyyz} = G_{dyz}^{(3)} - 2 Q_{fax}^{(1)} + 2 Q_{fbx}^{(1)} + 2 Q_{px}^{(1)} \\
& G_{yyxy} = G_{dxy}^{(3)} + 2 Q_{faz}^{(1)} + 2 Q_{fbz}^{(1)} - 2 Q_{pz}^{(1)} \\
& G_{zzyz} = G_{dyz}^{(3)} + 2 Q_{fax}^{(1)} + 2 Q_{fbx}^{(1)} - 2 Q_{px}^{(1)} \\
& G_{zzxy} = G_{dxy}^{(3)} - 4 Q_{fbz}^{(1)} \\
& G_{yzzx} = - 4 Q_{faz}^{(1)} - Q_{pz}^{(1)} \\
& G_{zxxy} = - 4 Q_{fax}^{(1)} - Q_{px}^{(1)}
\end{align*}
* Rank 4 tensor (aas).
\begin{align*}
\begin{bmatrix} 0 & G_{yzzx} & 0 \\ G_{yzzx} & 0 & G_{zxxy} \\ 0 & G_{zxxy} & 0 \end{bmatrix}
\end{align*}
\begin{align*}
& G_{yzzx} = 2 G_{dxy}^{(4)} \\
& G_{zxxy} = 2 G_{dyz}^{(4)}
\end{align*}
* Rank 4 tensor (aaa).
\begin{align*}
\begin{bmatrix} 0 & G_{yzzx} & 0 \\ - G_{yzzx} & 0 & G_{zxxy} \\ 0 & - G_{zxxy} & 0 \end{bmatrix}
\end{align*}
\begin{align*}
& G_{yzzx} = - Q_{pz}^{(2)} \\
& G_{zxxy} = - Q_{px}^{(2)}
\end{align*}
* Rank 4 tensor (sa).
\begin{align*}
\begin{bmatrix} G_{xxyz} & 0 & G_{xxxy} \\ G_{yyyz} & 0 & G_{yyxy} \\ G_{zzyz} & 0 & G_{zzxy} \\ 0 & G_{yzzx} & 0 \\ G_{zxyz} & 0 & G_{zxxy} \\ 0 & G_{xyzx} & 0 \end{bmatrix}
\end{align*}
\begin{align*}
& G_{xxyz} = 2 Q_{fax}^{(2)} + Q_{px}^{(3)} + 2 Q_{px}^{(4)} \\
& G_{xxxy} = - 2 G_{dxy}^{(5)} - Q_{faz}^{(2)} + Q_{fbz}^{(2)} + Q_{pz}^{(3)} \\
& G_{yyyz} = - 2 G_{dyz}^{(5)} - Q_{fax}^{(2)} + Q_{fbx}^{(2)} + Q_{px}^{(3)} \\
& G_{yyxy} = 2 G_{dxy}^{(5)} - Q_{faz}^{(2)} - Q_{fbz}^{(2)} + Q_{pz}^{(3)} \\
& G_{zzyz} = 2 G_{dyz}^{(5)} - Q_{fax}^{(2)} - Q_{fbx}^{(2)} + Q_{px}^{(3)} \\
& G_{zzxy} = 2 Q_{faz}^{(2)} + Q_{pz}^{(3)} + 2 Q_{pz}^{(4)} \\
& G_{yzzx} = - G_{dxy}^{(5)} - Q_{faz}^{(2)} - Q_{fbz}^{(2)} + Q_{pz}^{(4)} \\
& G_{zxyz} = G_{dxy}^{(5)} - Q_{faz}^{(2)} + Q_{fbz}^{(2)} + Q_{pz}^{(4)} \\
& G_{zxxy} = - G_{dyz}^{(5)} - Q_{fax}^{(2)} - Q_{fbx}^{(2)} + Q_{px}^{(4)} \\
& G_{xyzx} = G_{dyz}^{(5)} - Q_{fax}^{(2)} + Q_{fbx}^{(2)} + Q_{px}^{(4)}
\end{align*}
* Rank 4 tensor (as).
\begin{align*}
\begin{bmatrix} G_{yzxx} & G_{yzyy} & G_{yzzz} & 0 & G_{yzzx} & 0 \\ 0 & 0 & 0 & G_{zxyz} & 0 & G_{zxxy} \\ G_{xyxx} & G_{xyyy} & G_{xyzz} & 0 & G_{xyzx} & 0 \end{bmatrix}
\end{align*}
\begin{align*}
& G_{yzxx} = 2 Q_{fax}^{(3)} + Q_{px}^{(5)} + 2 Q_{px}^{(6)} \\
& G_{yzyy} = - 2 G_{dyz}^{(6)} - Q_{fax}^{(3)} + Q_{fbx}^{(3)} + Q_{px}^{(5)} \\
& G_{yzzz} = 2 G_{dyz}^{(6)} - Q_{fax}^{(3)} - Q_{fbx}^{(3)} + Q_{px}^{(5)} \\
& G_{yzzx} = G_{dxy}^{(6)} - Q_{faz}^{(3)} + Q_{fbz}^{(3)} + Q_{pz}^{(6)} \\
& G_{zxyz} = - G_{dxy}^{(6)} - Q_{faz}^{(3)} - Q_{fbz}^{(3)} + Q_{pz}^{(6)} \\
& G_{zxxy} = G_{dyz}^{(6)} - Q_{fax}^{(3)} + Q_{fbx}^{(3)} + Q_{px}^{(6)} \\
& G_{xyxx} = - 2 G_{dxy}^{(6)} - Q_{faz}^{(3)} + Q_{fbz}^{(3)} + Q_{pz}^{(5)} \\
& G_{xyyy} = 2 G_{dxy}^{(6)} - Q_{faz}^{(3)} - Q_{fbz}^{(3)} + Q_{pz}^{(5)} \\
& G_{xyzz} = 2 Q_{faz}^{(3)} + Q_{pz}^{(5)} + 2 Q_{pz}^{(6)} \\
& G_{xyzx} = - G_{dyz}^{(6)} - Q_{fax}^{(3)} - Q_{fbx}^{(3)} + Q_{px}^{(6)}
\end{align*}
* Rank 4 tensor (s).
\begin{align*}
\begin{bmatrix} 0 & 0 & 0 & G_{xxyz} & 0 & G_{xxxy} & G_{xxzy} & 0 & G_{xxyx} \\ 0 & 0 & 0 & G_{yyyz} & 0 & G_{yyxy} & G_{yyzy} & 0 & G_{yyyx} \\ 0 & 0 & 0 & G_{zzyz} & 0 & G_{zzxy} & G_{zzzy} & 0 & G_{zzyx} \\ G_{yzxx} & G_{yzyy} & G_{yzzz} & 0 & G_{yzzx} & 0 & 0 & G_{yzxz} & 0 \\ 0 & 0 & 0 & G_{zxyz} & 0 & G_{zxxy} & G_{zxzy} & 0 & G_{zxyx} \\ G_{xyxx} & G_{xyyy} & G_{xyzz} & 0 & G_{xyzx} & 0 & 0 & G_{xyxz} & 0 \end{bmatrix}
\end{align*}
\begin{align*}
& G_{xxyz} = G_{dyz}^{(1)} + G_{dyz}^{(3)} + 2 G_{gbx}^{(1)} + 2 Q_{fax}^{(2)} - 4 Q_{fbx}^{(1)} + Q_{px}^{(3)} + 2 Q_{px}^{(4)} \\
& G_{xxxy} = G_{dxy}^{(1)} + 2 G_{dxy}^{(2)} + G_{dxy}^{(3)} - 2 G_{dxy}^{(5)} + G_{gaz}^{(1)} - G_{gbz}^{(1)} - 2 Q_{faz}^{(1)} - Q_{faz}^{(2)} + 2 Q_{fbz}^{(1)} + Q_{fbz}^{(2)} + 2 Q_{pz}^{(1)} + Q_{pz}^{(3)} \\
& G_{xxzy} = G_{dyz}^{(1)} + G_{dyz}^{(3)} + 2 G_{gbx}^{(1)} - 2 Q_{fax}^{(2)} - 4 Q_{fbx}^{(1)} - Q_{px}^{(3)} - 2 Q_{px}^{(4)} \\
& G_{xxyx} = G_{dxy}^{(1)} + 2 G_{dxy}^{(2)} + G_{dxy}^{(3)} + 2 G_{dxy}^{(5)} + G_{gaz}^{(1)} - G_{gbz}^{(1)} - 2 Q_{faz}^{(1)} + Q_{faz}^{(2)} + 2 Q_{fbz}^{(1)} - Q_{fbz}^{(2)} + 2 Q_{pz}^{(1)} - Q_{pz}^{(3)} \\
& G_{yyyz} = G_{dyz}^{(1)} + 2 G_{dyz}^{(2)} + G_{dyz}^{(3)} - 2 G_{dyz}^{(5)} + G_{gax}^{(1)} - G_{gbx}^{(1)} - 2 Q_{fax}^{(1)} - Q_{fax}^{(2)} + 2 Q_{fbx}^{(1)} + Q_{fbx}^{(2)} + 2 Q_{px}^{(1)} + Q_{px}^{(3)} \\
& G_{yyxy} = G_{dxy}^{(1)} + 2 G_{dxy}^{(2)} + G_{dxy}^{(3)} + 2 G_{dxy}^{(5)} - G_{gaz}^{(1)} - G_{gbz}^{(1)} + 2 Q_{faz}^{(1)} - Q_{faz}^{(2)} + 2 Q_{fbz}^{(1)} - Q_{fbz}^{(2)} - 2 Q_{pz}^{(1)} + Q_{pz}^{(3)} \\
& G_{yyzy} = G_{dyz}^{(1)} + 2 G_{dyz}^{(2)} + G_{dyz}^{(3)} + 2 G_{dyz}^{(5)} + G_{gax}^{(1)} - G_{gbx}^{(1)} - 2 Q_{fax}^{(1)} + Q_{fax}^{(2)} + 2 Q_{fbx}^{(1)} - Q_{fbx}^{(2)} + 2 Q_{px}^{(1)} - Q_{px}^{(3)} \\
& G_{yyyx} = G_{dxy}^{(1)} + 2 G_{dxy}^{(2)} + G_{dxy}^{(3)} - 2 G_{dxy}^{(5)} - G_{gaz}^{(1)} - G_{gbz}^{(1)} + 2 Q_{faz}^{(1)} + Q_{faz}^{(2)} + 2 Q_{fbz}^{(1)} + Q_{fbz}^{(2)} - 2 Q_{pz}^{(1)} - Q_{pz}^{(3)} \\
& G_{zzyz} = G_{dyz}^{(1)} + 2 G_{dyz}^{(2)} + G_{dyz}^{(3)} + 2 G_{dyz}^{(5)} - G_{gax}^{(1)} - G_{gbx}^{(1)} + 2 Q_{fax}^{(1)} - Q_{fax}^{(2)} + 2 Q_{fbx}^{(1)} - Q_{fbx}^{(2)} - 2 Q_{px}^{(1)} + Q_{px}^{(3)} \\
& G_{zzxy} = G_{dxy}^{(1)} + G_{dxy}^{(3)} + 2 G_{gbz}^{(1)} + 2 Q_{faz}^{(2)} - 4 Q_{fbz}^{(1)} + Q_{pz}^{(3)} + 2 Q_{pz}^{(4)} \\
& G_{zzzy} = G_{dyz}^{(1)} + 2 G_{dyz}^{(2)} + G_{dyz}^{(3)} - 2 G_{dyz}^{(5)} - G_{gax}^{(1)} - G_{gbx}^{(1)} + 2 Q_{fax}^{(1)} + Q_{fax}^{(2)} + 2 Q_{fbx}^{(1)} + Q_{fbx}^{(2)} - 2 Q_{px}^{(1)} - Q_{px}^{(3)} \\
& G_{zzyx} = G_{dxy}^{(1)} + G_{dxy}^{(3)} + 2 G_{gbz}^{(1)} - 2 Q_{faz}^{(2)} - 4 Q_{fbz}^{(1)} - Q_{pz}^{(3)} - 2 Q_{pz}^{(4)} \\
& G_{yzxx} = G_{dyz}^{(1)} - G_{dyz}^{(3)} + 2 G_{gbx}^{(1)} + 4 Q_{fbx}^{(1)} \\
& G_{yzyy} = G_{dyz}^{(1)} + 2 G_{dyz}^{(2)} - G_{dyz}^{(3)} + G_{gax}^{(1)} - G_{gbx}^{(1)} + 2 Q_{fax}^{(1)} - 2 Q_{fbx}^{(1)} - 2 Q_{px}^{(1)} \\
& G_{yzzz} = G_{dyz}^{(1)} + 2 G_{dyz}^{(2)} - G_{dyz}^{(3)} - G_{gax}^{(1)} - G_{gbx}^{(1)} - 2 Q_{fax}^{(1)} - 2 Q_{fbx}^{(1)} + 2 Q_{px}^{(1)} \\
& G_{yzzx} = G_{dxy}^{(2)} - G_{dxy}^{(5)} + 2 G_{gbz}^{(1)} - 4 Q_{faz}^{(1)} - Q_{faz}^{(2)} - Q_{fbz}^{(2)} - Q_{pz}^{(1)} + Q_{pz}^{(4)} \\
& G_{yzxz} = G_{dxy}^{(2)} + G_{dxy}^{(5)} + 2 G_{gbz}^{(1)} - 4 Q_{faz}^{(1)} + Q_{faz}^{(2)} + Q_{fbz}^{(2)} - Q_{pz}^{(1)} - Q_{pz}^{(4)} \\
& G_{zxyz} = G_{dxy}^{(2)} + G_{dxy}^{(5)} + 2 G_{gbz}^{(1)} + 4 Q_{faz}^{(1)} - Q_{faz}^{(2)} + Q_{fbz}^{(2)} + Q_{pz}^{(1)} + Q_{pz}^{(4)} \\
& G_{zxxy} = G_{dyz}^{(2)} - G_{dyz}^{(5)} + 2 G_{gbx}^{(1)} - 4 Q_{fax}^{(1)} - Q_{fax}^{(2)} - Q_{fbx}^{(2)} - Q_{px}^{(1)} + Q_{px}^{(4)} \\
& G_{zxzy} = G_{dxy}^{(2)} - G_{dxy}^{(5)} + 2 G_{gbz}^{(1)} + 4 Q_{faz}^{(1)} + Q_{faz}^{(2)} - Q_{fbz}^{(2)} + Q_{pz}^{(1)} - Q_{pz}^{(4)} \\
& G_{zxyx} = G_{dyz}^{(2)} + G_{dyz}^{(5)} + 2 G_{gbx}^{(1)} - 4 Q_{fax}^{(1)} + Q_{fax}^{(2)} + Q_{fbx}^{(2)} - Q_{px}^{(1)} - Q_{px}^{(4)} \\
& G_{xyxx} = G_{dxy}^{(1)} + 2 G_{dxy}^{(2)} - G_{dxy}^{(3)} + G_{gaz}^{(1)} - G_{gbz}^{(1)} + 2 Q_{faz}^{(1)} - 2 Q_{fbz}^{(1)} - 2 Q_{pz}^{(1)} \\
& G_{xyyy} = G_{dxy}^{(1)} + 2 G_{dxy}^{(2)} - G_{dxy}^{(3)} - G_{gaz}^{(1)} - G_{gbz}^{(1)} - 2 Q_{faz}^{(1)} - 2 Q_{fbz}^{(1)} + 2 Q_{pz}^{(1)} \\
& G_{xyzz} = G_{dxy}^{(1)} - G_{dxy}^{(3)} + 2 G_{gbz}^{(1)} + 4 Q_{fbz}^{(1)} \\
& G_{xyzx} = G_{dyz}^{(2)} + G_{dyz}^{(5)} + 2 G_{gbx}^{(1)} + 4 Q_{fax}^{(1)} - Q_{fax}^{(2)} + Q_{fbx}^{(2)} + Q_{px}^{(1)} + Q_{px}^{(4)} \\
& G_{xyxz} = G_{dyz}^{(2)} - G_{dyz}^{(5)} + 2 G_{gbx}^{(1)} + 4 Q_{fax}^{(1)} + Q_{fax}^{(2)} - Q_{fbx}^{(2)} + Q_{px}^{(1)} - Q_{px}^{(4)}
\end{align*}
* Rank 4 tensor (a).
\begin{align*}
\begin{bmatrix} G_{yzxx} & G_{yzyy} & G_{yzzz} & 0 & G_{yzzx} & 0 & 0 & G_{yzxz} & 0 \\ 0 & 0 & 0 & G_{zxyz} & 0 & G_{zxxy} & G_{zxzy} & 0 & G_{zxyx} \\ G_{xyxx} & G_{xyyy} & G_{xyzz} & 0 & G_{xyzx} & 0 & 0 & G_{xyxz} & 0 \end{bmatrix}
\end{align*}
\begin{align*}
& G_{yzxx} = 2 Q_{fax}^{(3)} + Q_{px}^{(5)} + 2 Q_{px}^{(6)} \\
& G_{yzyy} = - 2 G_{dyz}^{(6)} - Q_{fax}^{(3)} + Q_{fbx}^{(3)} + Q_{px}^{(5)} \\
& G_{yzzz} = 2 G_{dyz}^{(6)} - Q_{fax}^{(3)} - Q_{fbx}^{(3)} + Q_{px}^{(5)} \\
& G_{yzzx} = 2 G_{dxy}^{(4)} + G_{dxy}^{(6)} - Q_{faz}^{(3)} + Q_{fbz}^{(3)} - Q_{pz}^{(2)} + Q_{pz}^{(6)} \\
& G_{yzxz} = - 2 G_{dxy}^{(4)} + G_{dxy}^{(6)} - Q_{faz}^{(3)} + Q_{fbz}^{(3)} + Q_{pz}^{(2)} + Q_{pz}^{(6)} \\
& G_{zxyz} = 2 G_{dxy}^{(4)} - G_{dxy}^{(6)} - Q_{faz}^{(3)} - Q_{fbz}^{(3)} + Q_{pz}^{(2)} + Q_{pz}^{(6)} \\
& G_{zxxy} = 2 G_{dyz}^{(4)} + G_{dyz}^{(6)} - Q_{fax}^{(3)} + Q_{fbx}^{(3)} - Q_{px}^{(2)} + Q_{px}^{(6)} \\
& G_{zxzy} = - 2 G_{dxy}^{(4)} - G_{dxy}^{(6)} - Q_{faz}^{(3)} - Q_{fbz}^{(3)} - Q_{pz}^{(2)} + Q_{pz}^{(6)} \\
& G_{zxyx} = - 2 G_{dyz}^{(4)} + G_{dyz}^{(6)} - Q_{fax}^{(3)} + Q_{fbx}^{(3)} + Q_{px}^{(2)} + Q_{px}^{(6)} \\
& G_{xyxx} = - 2 G_{dxy}^{(6)} - Q_{faz}^{(3)} + Q_{fbz}^{(3)} + Q_{pz}^{(5)} \\
& G_{xyyy} = 2 G_{dxy}^{(6)} - Q_{faz}^{(3)} - Q_{fbz}^{(3)} + Q_{pz}^{(5)} \\
& G_{xyzz} = 2 Q_{faz}^{(3)} + Q_{pz}^{(5)} + 2 Q_{pz}^{(6)} \\
& G_{xyzx} = 2 G_{dyz}^{(4)} - G_{dyz}^{(6)} - Q_{fax}^{(3)} - Q_{fbx}^{(3)} + Q_{px}^{(2)} + Q_{px}^{(6)} \\
& G_{xyxz} = - 2 G_{dyz}^{(4)} - G_{dyz}^{(6)} - Q_{fax}^{(3)} - Q_{fbx}^{(3)} - Q_{px}^{(2)} + Q_{px}^{(6)}
\end{align*}
* Rank 4 tensor (t).
\begin{align*}
\begin{bmatrix} 0 & G_{xxxy} & 0 \\ G_{yyyx} & 0 & G_{yyyz} \\ 0 & G_{zzzy} & 0 \\ 0 & G_{yyzy} & 0 \\ 0 & G_{zzxy} & 0 \\ G_{xxyx} & 0 & G_{xxyz} \\ G_{yzzx} & 0 & G_{yzzz} \\ 0 & G_{zxxy} & 0 \\ 0 & G_{xyyy} & 0 \\ - \frac{G_{yyyz}}{2} + \frac{G_{yyzy}}{2} + G_{zxxy} & 0 & \frac{G_{xxxy}}{2} - \frac{G_{xxyx}}{2} + G_{xyyy} - G_{yyyx} + G_{zzxy} \end{bmatrix}
\end{align*}
\begin{align*}
& G_{xxxy} = G_{dxy}^{(1)} + 2 G_{dxy}^{(2)} + G_{dxy}^{(3)} - 2 G_{dxy}^{(5)} + G_{gaz}^{(1)} - G_{gbz}^{(1)} \\
& G_{yyyx} = G_{dxy}^{(1)} + 2 G_{dxy}^{(2)} + G_{dxy}^{(3)} - 2 G_{dxy}^{(5)} - G_{gaz}^{(1)} - G_{gbz}^{(1)} \\
& G_{yyyz} = G_{dyz}^{(1)} + 2 G_{dyz}^{(2)} + G_{dyz}^{(3)} - 2 G_{dyz}^{(5)} + G_{gax}^{(1)} - G_{gbx}^{(1)} \\
& G_{zzzy} = G_{dyz}^{(1)} + 2 G_{dyz}^{(2)} + G_{dyz}^{(3)} - 2 G_{dyz}^{(5)} - G_{gax}^{(1)} - G_{gbx}^{(1)} \\
& G_{yyzy} = G_{dyz}^{(1)} + 2 G_{dyz}^{(2)} + G_{dyz}^{(3)} + 2 G_{dyz}^{(5)} + G_{gax}^{(1)} - G_{gbx}^{(1)} \\
& G_{zzxy} = G_{dxy}^{(1)} + G_{dxy}^{(3)} + 2 G_{gbz}^{(1)} \\
& G_{xxyx} = G_{dxy}^{(1)} + 2 G_{dxy}^{(2)} + G_{dxy}^{(3)} + 2 G_{dxy}^{(5)} + G_{gaz}^{(1)} - G_{gbz}^{(1)} \\
& G_{xxyz} = G_{dyz}^{(1)} + G_{dyz}^{(3)} + 2 G_{gbx}^{(1)} \\
& G_{yzzx} = G_{dxy}^{(2)} - G_{dxy}^{(5)} + 2 G_{gbz}^{(1)} \\
& G_{yzzz} = G_{dyz}^{(1)} + 2 G_{dyz}^{(2)} - G_{dyz}^{(3)} - G_{gax}^{(1)} - G_{gbx}^{(1)} \\
& G_{zxxy} = G_{dyz}^{(2)} - G_{dyz}^{(5)} + 2 G_{gbx}^{(1)} \\
& G_{xyyy} = G_{dxy}^{(1)} + 2 G_{dxy}^{(2)} - G_{dxy}^{(3)} - G_{gaz}^{(1)} - G_{gbz}^{(1)}
\end{align*}

\end{document}
