\documentclass[fleqn,8pt,landscape]{jsarticle}
\special{papersize=\the\paperwidth,\the\paperheight}

%%% package

\usepackage[usenames]{color}
\usepackage{amsmath}
\usepackage{breqn}
\usepackage{graphicx}
\usepackage{amssymb}
\usepackage{bm}
\usepackage{enumitem}
\usepackage{braket}
\usepackage{multirow}
\usepackage{booktabs}
\usepackage{longtable}

%%% layout setting

\paperwidth=356.4truemm
\paperheight=252.0truemm
\textwidth=335.59999999999997truemm
\textheight=224.2truemm
\oddsidemargin=-15truemm
\topmargin=-15truemm
\footskip=7truemm

%%% fixed

\hoffset=0truemm
\voffset=0truemm
\headheight=0truemm
\headsep=0truemm
\marginparsep=0truemm
\marginparwidth=0truemm

%%% main text

\begin{document}

\setcounter{MaxMatrixCols}{32}

\renewcommand{\tablename}{Table~}
\renewcommand{\figurename}{Figure~}
\begin{center}
\LARGE
MPG No. 28.1.107\quad$23$\quad[ Type I, cubic ] [M tensor]
\end{center}
* Rank 0 tensor.
\begin{align*}
\begin{bmatrix} M \end{bmatrix}
\end{align*}
\begin{align*}
& M = M_{s}^{(1)}
\end{align*}
* Rank 1 tensor.
* Rank 2 tensor (s).
\begin{align*}
\begin{bmatrix} M_{xx} & 0 & 0 \\ 0 & M_{xx} & 0 \\ 0 & 0 & M_{xx} \end{bmatrix}
\end{align*}
\begin{align*}
& M_{xx} = M_{s}^{(1)}
\end{align*}
* Rank 2 tensor (a).
* Rank 3 tensor (s).
\begin{align*}
\begin{bmatrix} 0 & 0 & 0 \\ 0 & 0 & 0 \\ 0 & 0 & 0 \\ M_{yzx} & 0 & 0 \\ 0 & M_{yzx} & 0 \\ 0 & 0 & M_{yzx} \end{bmatrix}
\end{align*}
\begin{align*}
& M_{yzx} = M_{f3}^{(1)}
\end{align*}
* Rank 3 tensor (a).
\begin{align*}
\begin{bmatrix} M_{yzx} & 0 & 0 \\ 0 & M_{yzx} & 0 \\ 0 & 0 & M_{yzx} \end{bmatrix}
\end{align*}
\begin{align*}
& M_{yzx} = T_{s}^{(1)}
\end{align*}
* Rank 4 tensor (sss).
\begin{align*}
\begin{bmatrix} M_{xxxx} & M_{xxyy} & M_{xxyy} & 0 & 0 & 0 \\ M_{xxyy} & M_{xxxx} & M_{xxyy} & 0 & 0 & 0 \\ M_{xxyy} & M_{xxyy} & M_{xxxx} & 0 & 0 & 0 \\ 0 & 0 & 0 & M_{yzyz} & 0 & 0 \\ 0 & 0 & 0 & 0 & M_{yzyz} & 0 \\ 0 & 0 & 0 & 0 & 0 & M_{yzyz} \end{bmatrix}
\end{align*}
\begin{align*}
& M_{xxxx} = 2 M_{g}^{(1)} + M_{s}^{(1)} + 2 M_{s}^{(2)} \\
& M_{xxyy} = - M_{g}^{(1)} + M_{s}^{(1)} \\
& M_{yzyz} = - M_{g}^{(1)} + M_{s}^{(2)}
\end{align*}
* Rank 4 tensor (ssa).
\begin{align*}
\begin{bmatrix} 0 & M_{xxyy} & - M_{xxyy} & 0 & 0 & 0 \\ - M_{xxyy} & 0 & M_{xxyy} & 0 & 0 & 0 \\ M_{xxyy} & - M_{xxyy} & 0 & 0 & 0 & 0 \\ 0 & 0 & 0 & 0 & 0 & 0 \\ 0 & 0 & 0 & 0 & 0 & 0 \\ 0 & 0 & 0 & 0 & 0 & 0 \end{bmatrix}
\end{align*}
\begin{align*}
& M_{xxyy} = 4 T_{f3}^{(1)}
\end{align*}
* Rank 4 tensor (aas).
\begin{align*}
\begin{bmatrix} M_{yzyz} & 0 & 0 \\ 0 & M_{yzyz} & 0 \\ 0 & 0 & M_{yzyz} \end{bmatrix}
\end{align*}
\begin{align*}
& M_{yzyz} = M_{s}^{(3)}
\end{align*}
* Rank 4 tensor (aaa).
* Rank 4 tensor (sa).
\begin{align*}
\begin{bmatrix} 0 & 0 & 0 \\ 0 & 0 & 0 \\ 0 & 0 & 0 \\ M_{yzyz} & 0 & 0 \\ 0 & M_{yzyz} & 0 \\ 0 & 0 & M_{yzyz} \end{bmatrix}
\end{align*}
\begin{align*}
& M_{yzyz} = T_{f3}^{(2)}
\end{align*}
* Rank 4 tensor (as).
\begin{align*}
\begin{bmatrix} 0 & 0 & 0 & M_{yzyz} & 0 & 0 \\ 0 & 0 & 0 & 0 & M_{yzyz} & 0 \\ 0 & 0 & 0 & 0 & 0 & M_{yzyz} \end{bmatrix}
\end{align*}
\begin{align*}
& M_{yzyz} = T_{f3}^{(3)}
\end{align*}
* Rank 4 tensor (s).
\begin{align*}
\begin{bmatrix} M_{xxxx} & M_{xxyy} & M_{xxzz} & 0 & 0 & 0 & 0 & 0 & 0 \\ M_{xxzz} & M_{xxxx} & M_{xxyy} & 0 & 0 & 0 & 0 & 0 & 0 \\ M_{xxyy} & M_{xxzz} & M_{xxxx} & 0 & 0 & 0 & 0 & 0 & 0 \\ 0 & 0 & 0 & M_{yzyz} & 0 & 0 & M_{yzzy} & 0 & 0 \\ 0 & 0 & 0 & 0 & M_{yzyz} & 0 & 0 & M_{yzzy} & 0 \\ 0 & 0 & 0 & 0 & 0 & M_{yzyz} & 0 & 0 & M_{yzzy} \end{bmatrix}
\end{align*}
\begin{align*}
& M_{xxxx} = 2 M_{g}^{(1)} + M_{s}^{(1)} + 2 M_{s}^{(2)} \\
& M_{xxyy} = - M_{g}^{(1)} + M_{s}^{(1)} + 4 T_{f3}^{(1)} \\
& M_{xxzz} = - M_{g}^{(1)} + M_{s}^{(1)} - 4 T_{f3}^{(1)} \\
& M_{yzyz} = - M_{g}^{(1)} + M_{s}^{(2)} + T_{f3}^{(2)} \\
& M_{yzzy} = - M_{g}^{(1)} + M_{s}^{(2)} - T_{f3}^{(2)}
\end{align*}
* Rank 4 tensor (a).
\begin{align*}
\begin{bmatrix} 0 & 0 & 0 & M_{yzyz} & 0 & 0 & M_{yzzy} & 0 & 0 \\ 0 & 0 & 0 & 0 & M_{yzyz} & 0 & 0 & M_{yzzy} & 0 \\ 0 & 0 & 0 & 0 & 0 & M_{yzyz} & 0 & 0 & M_{yzzy} \end{bmatrix}
\end{align*}
\begin{align*}
& M_{yzyz} = M_{s}^{(3)} + T_{f3}^{(3)} \\
& M_{yzzy} = - M_{s}^{(3)} + T_{f3}^{(3)}
\end{align*}
* Rank 4 tensor (t).
\begin{align*}
\begin{bmatrix} M_{xxxx} & 0 & 0 \\ 0 & M_{xxxx} & 0 \\ 0 & 0 & M_{xxxx} \\ 0 & 0 & M_{yyzz} \\ M_{yyzz} & 0 & 0 \\ 0 & M_{yyzz} & 0 \\ 0 & M_{yyzz} & 0 \\ 0 & 0 & M_{yyzz} \\ M_{yyzz} & 0 & 0 \\ 0 & 0 & 0 \end{bmatrix}
\end{align*}
\begin{align*}
& M_{xxxx} = 2 M_{g}^{(1)} + 3 M_{s}^{(1)} \\
& M_{yyzz} = - M_{g}^{(1)} + M_{s}^{(1)}
\end{align*}

\end{document}
