\documentclass[fleqn,8pt,landscape]{jsarticle}
\special{papersize=\the\paperwidth,\the\paperheight}

%%% package

\usepackage[usenames]{color}
\usepackage{amsmath}
\usepackage{breqn}
\usepackage{graphicx}
\usepackage{amssymb}
\usepackage{bm}
\usepackage{enumitem}
\usepackage{braket}
\usepackage{multirow}
\usepackage{booktabs}
\usepackage{longtable}

%%% layout setting

\paperwidth=356.4truemm
\paperheight=252.0truemm
\textwidth=335.59999999999997truemm
\textheight=224.2truemm
\oddsidemargin=-15truemm
\topmargin=-15truemm
\footskip=7truemm

%%% fixed

\hoffset=0truemm
\voffset=0truemm
\headheight=0truemm
\headsep=0truemm
\marginparsep=0truemm
\marginparwidth=0truemm

%%% main text

\begin{document}

\setcounter{MaxMatrixCols}{32}

\renewcommand{\tablename}{Table~}
\renewcommand{\figurename}{Figure~}
\begin{center}
\LARGE
MPG No. 20.3.73\quad$\bar{3}'m$\quad(-3'm1 setting)\quad[ Type III, trigonal ] [M tensor]
\end{center}
* Rank 0 tensor.
* Rank 1 tensor.
* Rank 2 tensor (s).
* Rank 2 tensor (a).
\begin{align*}
\begin{bmatrix} 0 & M_{xy} & 0 \\ - M_{xy} & 0 & 0 \\ 0 & 0 & 0 \end{bmatrix}
\end{align*}
\begin{align*}
& M_{xy} = T_{pz}^{(1)}
\end{align*}
* Rank 3 tensor (s).
* Rank 3 tensor (a).
* Rank 4 tensor (sss).
\begin{align*}
\begin{bmatrix} 0 & 0 & 0 & 0 & M_{xxzx} & 0 \\ 0 & 0 & 0 & 0 & - M_{xxzx} & 0 \\ 0 & 0 & 0 & 0 & 0 & 0 \\ 0 & 0 & 0 & 0 & 0 & - M_{xxzx} \\ M_{xxzx} & - M_{xxzx} & 0 & 0 & 0 & 0 \\ 0 & 0 & 0 & - M_{xxzx} & 0 & 0 \end{bmatrix}
\end{align*}
\begin{align*}
& M_{xxzx} = M_{ga}^{(1)}
\end{align*}
* Rank 4 tensor (ssa).
\begin{align*}
\begin{bmatrix} 0 & 0 & 0 & 0 & M_{xxzx} & M_{xxxy} \\ 0 & 0 & 0 & 0 & - M_{xxzx} & - M_{xxxy} \\ 0 & 0 & 0 & 0 & 0 & 0 \\ 0 & 0 & 0 & 0 & M_{yzzx} & M_{xxzx} \\ - M_{xxzx} & M_{xxzx} & 0 & - M_{yzzx} & 0 & 0 \\ - M_{xxxy} & M_{xxxy} & 0 & - M_{xxzx} & 0 & 0 \end{bmatrix}
\end{align*}
\begin{align*}
& M_{xxzx} = - 2 T_{f1}^{(1)} \\
& M_{xxxy} = - 2 T_{faz}^{(1)} + 2 T_{pz}^{(1)} \\
& M_{yzzx} = - 4 T_{faz}^{(1)} - T_{pz}^{(1)}
\end{align*}
* Rank 4 tensor (aas).
* Rank 4 tensor (aaa).
\begin{align*}
\begin{bmatrix} 0 & M_{yzzx} & 0 \\ - M_{yzzx} & 0 & 0 \\ 0 & 0 & 0 \end{bmatrix}
\end{align*}
\begin{align*}
& M_{yzzx} = - T_{pz}^{(2)}
\end{align*}
* Rank 4 tensor (sa).
\begin{align*}
\begin{bmatrix} 0 & M_{xxzx} & M_{xxxy} \\ 0 & - M_{xxzx} & M_{xxxy} \\ 0 & 0 & M_{zzxy} \\ 0 & M_{yzzx} & 0 \\ M_{yzzx} & 0 & 0 \\ M_{xxzx} & 0 & 0 \end{bmatrix}
\end{align*}
\begin{align*}
& M_{xxzx} = T_{f1}^{(2)} \\
& M_{xxxy} = - T_{faz}^{(2)} + T_{pz}^{(3)} \\
& M_{zzxy} = 2 T_{faz}^{(2)} + T_{pz}^{(3)} + 2 T_{pz}^{(4)} \\
& M_{yzzx} = - T_{faz}^{(2)} + T_{pz}^{(4)}
\end{align*}
* Rank 4 tensor (as).
\begin{align*}
\begin{bmatrix} 0 & 0 & 0 & 0 & M_{yzzx} & M_{yzxy} \\ M_{yzxy} & - M_{yzxy} & 0 & M_{yzzx} & 0 & 0 \\ M_{xyxx} & M_{xyxx} & M_{xyzz} & 0 & 0 & 0 \end{bmatrix}
\end{align*}
\begin{align*}
& M_{yzzx} = - T_{faz}^{(3)} + T_{pz}^{(6)} \\
& M_{yzxy} = T_{f1}^{(3)} \\
& M_{xyxx} = - T_{faz}^{(3)} + T_{pz}^{(5)} \\
& M_{xyzz} = 2 T_{faz}^{(3)} + T_{pz}^{(5)} + 2 T_{pz}^{(6)}
\end{align*}
* Rank 4 tensor (s).
\begin{align*}
\begin{bmatrix} 0 & 0 & 0 & 0 & M_{xxzx} & M_{xxxy} & 0 & M_{xxxz} & M_{xxyx} \\ 0 & 0 & 0 & 0 & - M_{xxzx} & - M_{xxyx} & 0 & - M_{xxxz} & - M_{xxxy} \\ 0 & 0 & 0 & 0 & 0 & M_{zzxy} & 0 & 0 & - M_{zzxy} \\ 0 & 0 & 0 & 0 & M_{yzzx} & M_{yzxy} & 0 & M_{yzxz} & M_{yzxy} \\ - M_{yzxy} & M_{yzxy} & 0 & - M_{yzxz} & 0 & 0 & - M_{yzzx} & 0 & 0 \\ - \frac{M_{xxxy}}{2} - \frac{M_{xxyx}}{2} & \frac{M_{xxxy}}{2} + \frac{M_{xxyx}}{2} & 0 & - M_{xxxz} & 0 & 0 & - M_{xxzx} & 0 & 0 \end{bmatrix}
\end{align*}
\begin{align*}
& M_{xxzx} = M_{ga}^{(1)} - 2 T_{f1}^{(1)} + T_{f1}^{(2)} \\
& M_{xxxy} = - 2 T_{faz}^{(1)} - T_{faz}^{(2)} + 2 T_{pz}^{(1)} + T_{pz}^{(3)} \\
& M_{xxxz} = M_{ga}^{(1)} - 2 T_{f1}^{(1)} - T_{f1}^{(2)} \\
& M_{xxyx} = - 2 T_{faz}^{(1)} + T_{faz}^{(2)} + 2 T_{pz}^{(1)} - T_{pz}^{(3)} \\
& M_{zzxy} = 2 T_{faz}^{(2)} + T_{pz}^{(3)} + 2 T_{pz}^{(4)} \\
& M_{yzzx} = - 4 T_{faz}^{(1)} - T_{faz}^{(2)} - T_{pz}^{(1)} + T_{pz}^{(4)} \\
& M_{yzxy} = - M_{ga}^{(1)} - 2 T_{f1}^{(1)} \\
& M_{yzxz} = - 4 T_{faz}^{(1)} + T_{faz}^{(2)} - T_{pz}^{(1)} - T_{pz}^{(4)}
\end{align*}
* Rank 4 tensor (a).
\begin{align*}
\begin{bmatrix} 0 & 0 & 0 & 0 & M_{yzzx} & M_{yzxy} & 0 & M_{yzxz} & M_{yzxy} \\ M_{yzxy} & - M_{yzxy} & 0 & M_{yzxz} & 0 & 0 & M_{yzzx} & 0 & 0 \\ M_{xyxx} & M_{xyxx} & M_{xyzz} & 0 & 0 & 0 & 0 & 0 & 0 \end{bmatrix}
\end{align*}
\begin{align*}
& M_{yzzx} = - T_{faz}^{(3)} - T_{pz}^{(2)} + T_{pz}^{(6)} \\
& M_{yzxy} = T_{f1}^{(3)} \\
& M_{yzxz} = - T_{faz}^{(3)} + T_{pz}^{(2)} + T_{pz}^{(6)} \\
& M_{xyxx} = - T_{faz}^{(3)} + T_{pz}^{(5)} \\
& M_{xyzz} = 2 T_{faz}^{(3)} + T_{pz}^{(5)} + 2 T_{pz}^{(6)}
\end{align*}
* Rank 4 tensor (t).
\begin{align*}
\begin{bmatrix} 0 & 0 & M_{xxxz} \\ 0 & 0 & 0 \\ 0 & 0 & 0 \\ - M_{xxxz} & 0 & 0 \\ 0 & 0 & 0 \\ 0 & 0 & 0 \\ 0 & 0 & 0 \\ M_{xxxz} & 0 & 0 \\ 0 & 0 & - M_{xxxz} \\ 0 & - M_{xxxz} & 0 \end{bmatrix}
\end{align*}
\begin{align*}
& M_{xxxz} = M_{ga}^{(1)}
\end{align*}

\end{document}
