\documentclass[fleqn,8pt,landscape]{jsarticle}
\special{papersize=\the\paperwidth,\the\paperheight}

%%% package

\usepackage[usenames]{color}
\usepackage{amsmath}
\usepackage{breqn}
\usepackage{graphicx}
\usepackage{amssymb}
\usepackage{bm}
\usepackage{enumitem}
\usepackage{braket}
\usepackage{multirow}
\usepackage{booktabs}
\usepackage{longtable}

%%% layout setting

\paperwidth=356.4truemm
\paperheight=252.0truemm
\textwidth=335.59999999999997truemm
\textheight=224.2truemm
\oddsidemargin=-15truemm
\topmargin=-15truemm
\footskip=7truemm

%%% fixed

\hoffset=0truemm
\voffset=0truemm
\headheight=0truemm
\headsep=0truemm
\marginparsep=0truemm
\marginparwidth=0truemm

%%% main text

\begin{document}

\setcounter{MaxMatrixCols}{32}

\renewcommand{\tablename}{Table~}
\renewcommand{\figurename}{Figure~}
\begin{center}
\LARGE
MPG No. 33.3.133\quad$\bar{4}'2'm$\quad(-4'm2' setting)\quad[ Type III, tetragonal ] [T tensor]
\end{center}
* Rank 0 tensor.
* Rank 1 tensor.
\begin{align*}
\begin{bmatrix} 0 & 0 & T_{z} \end{bmatrix}
\end{align*}
\begin{align*}
& T_{z} = T_{pz}^{(1)}
\end{align*}
* Rank 2 tensor (s).
\begin{align*}
\begin{bmatrix} T_{xx} & 0 & 0 \\ 0 & - T_{xx} & 0 \\ 0 & 0 & 0 \end{bmatrix}
\end{align*}
\begin{align*}
& T_{xx} = T_{dv}^{(1)}
\end{align*}
* Rank 2 tensor (a).
* Rank 3 tensor (s).
\begin{align*}
\begin{bmatrix} 0 & 0 & T_{xxz} \\ 0 & 0 & T_{xxz} \\ 0 & 0 & T_{zzz} \\ 0 & T_{yzy} & 0 \\ T_{yzy} & 0 & 0 \\ 0 & 0 & 0 \end{bmatrix}
\end{align*}
\begin{align*}
& T_{xxz} = - T_{faz}^{(1)} + T_{pz}^{(1)} \\
& T_{zzz} = 2 T_{faz}^{(1)} + T_{pz}^{(1)} + 2 T_{pz}^{(2)} \\
& T_{yzy} = - T_{faz}^{(1)} + T_{pz}^{(2)}
\end{align*}
* Rank 3 tensor (a).
\begin{align*}
\begin{bmatrix} 0 & T_{yzy} & 0 \\ - T_{yzy} & 0 & 0 \\ 0 & 0 & 0 \end{bmatrix}
\end{align*}
\begin{align*}
& T_{yzy} = T_{pz}^{(3)}
\end{align*}
* Rank 4 tensor (sss).
\begin{align*}
\begin{bmatrix} T_{xxxx} & 0 & T_{xxzz} & 0 & 0 & 0 \\ 0 & - T_{xxxx} & - T_{xxzz} & 0 & 0 & 0 \\ T_{xxzz} & - T_{xxzz} & 0 & 0 & 0 & 0 \\ 0 & 0 & 0 & T_{yzyz} & 0 & 0 \\ 0 & 0 & 0 & 0 & - T_{yzyz} & 0 \\ 0 & 0 & 0 & 0 & 0 & 0 \end{bmatrix}
\end{align*}
\begin{align*}
& T_{xxxx} = 2 T_{dv}^{(1)} + 4 T_{dv}^{(2)} + T_{gv}^{(1)} \\
& T_{xxzz} = T_{dv}^{(1)} - T_{gv}^{(1)} \\
& T_{yzyz} = - T_{dv}^{(2)} + T_{gv}^{(1)}
\end{align*}
* Rank 4 tensor (ssa).
\begin{align*}
\begin{bmatrix} 0 & T_{xxyy} & T_{xxzz} & 0 & 0 & 0 \\ - T_{xxyy} & 0 & - T_{xxzz} & 0 & 0 & 0 \\ - T_{xxzz} & T_{xxzz} & 0 & 0 & 0 & 0 \\ 0 & 0 & 0 & 0 & 0 & 0 \\ 0 & 0 & 0 & 0 & 0 & 0 \\ 0 & 0 & 0 & 0 & 0 & 0 \end{bmatrix}
\end{align*}
\begin{align*}
& T_{xxyy} = 4 M_{f3}^{(1)} - 2 T_{dv}^{(3)} \\
& T_{xxzz} = - 4 M_{f3}^{(1)} - T_{dv}^{(3)}
\end{align*}
* Rank 4 tensor (aas).
\begin{align*}
\begin{bmatrix} T_{yzyz} & 0 & 0 \\ 0 & - T_{yzyz} & 0 \\ 0 & 0 & 0 \end{bmatrix}
\end{align*}
\begin{align*}
& T_{yzyz} = 2 T_{dv}^{(4)}
\end{align*}
* Rank 4 tensor (aaa).
* Rank 4 tensor (sa).
\begin{align*}
\begin{bmatrix} 0 & 0 & 0 \\ 0 & 0 & 0 \\ 0 & 0 & 0 \\ T_{yzyz} & 0 & 0 \\ 0 & T_{yzyz} & 0 \\ 0 & 0 & T_{xyxy} \end{bmatrix}
\end{align*}
\begin{align*}
& T_{yzyz} = M_{f3}^{(2)} - T_{dv}^{(5)} \\
& T_{xyxy} = M_{f3}^{(2)} + 2 T_{dv}^{(5)}
\end{align*}
* Rank 4 tensor (as).
\begin{align*}
\begin{bmatrix} 0 & 0 & 0 & T_{yzyz} & 0 & 0 \\ 0 & 0 & 0 & 0 & T_{yzyz} & 0 \\ 0 & 0 & 0 & 0 & 0 & T_{xyxy} \end{bmatrix}
\end{align*}
\begin{align*}
& T_{yzyz} = M_{f3}^{(3)} - T_{dv}^{(6)} \\
& T_{xyxy} = M_{f3}^{(3)} + 2 T_{dv}^{(6)}
\end{align*}
* Rank 4 tensor (s).
\begin{align*}
\begin{bmatrix} T_{xxxx} & T_{xxyy} & T_{xxzz} & 0 & 0 & 0 & 0 & 0 & 0 \\ - T_{xxyy} & - T_{xxxx} & - T_{xxzz} & 0 & 0 & 0 & 0 & 0 & 0 \\ T_{zzxx} & - T_{zzxx} & 0 & 0 & 0 & 0 & 0 & 0 & 0 \\ 0 & 0 & 0 & T_{yzyz} & 0 & 0 & T_{yzzy} & 0 & 0 \\ 0 & 0 & 0 & 0 & - T_{yzzy} & 0 & 0 & - T_{yzyz} & 0 \\ 0 & 0 & 0 & 0 & 0 & T_{xyxy} & 0 & 0 & - T_{xyxy} \end{bmatrix}
\end{align*}
\begin{align*}
& T_{xxxx} = 2 T_{dv}^{(1)} + 4 T_{dv}^{(2)} + T_{gv}^{(1)} \\
& T_{xxyy} = 4 M_{f3}^{(1)} - 2 T_{dv}^{(3)} \\
& T_{xxzz} = - 4 M_{f3}^{(1)} + T_{dv}^{(1)} - T_{dv}^{(3)} - T_{gv}^{(1)} \\
& T_{zzxx} = 4 M_{f3}^{(1)} + T_{dv}^{(1)} + T_{dv}^{(3)} - T_{gv}^{(1)} \\
& T_{yzyz} = M_{f3}^{(2)} - T_{dv}^{(2)} - T_{dv}^{(5)} + T_{gv}^{(1)} \\
& T_{yzzy} = - M_{f3}^{(2)} - T_{dv}^{(2)} + T_{dv}^{(5)} + T_{gv}^{(1)} \\
& T_{xyxy} = M_{f3}^{(2)} + 2 T_{dv}^{(5)}
\end{align*}
* Rank 4 tensor (a).
\begin{align*}
\begin{bmatrix} 0 & 0 & 0 & T_{yzyz} & 0 & 0 & T_{yzzy} & 0 & 0 \\ 0 & 0 & 0 & 0 & T_{yzzy} & 0 & 0 & T_{yzyz} & 0 \\ 0 & 0 & 0 & 0 & 0 & T_{xyxy} & 0 & 0 & T_{xyxy} \end{bmatrix}
\end{align*}
\begin{align*}
& T_{yzyz} = M_{f3}^{(3)} + 2 T_{dv}^{(4)} - T_{dv}^{(6)} \\
& T_{yzzy} = M_{f3}^{(3)} - 2 T_{dv}^{(4)} - T_{dv}^{(6)} \\
& T_{xyxy} = M_{f3}^{(3)} + 2 T_{dv}^{(6)}
\end{align*}
* Rank 4 tensor (t).
\begin{align*}
\begin{bmatrix} T_{xxxx} & 0 & 0 \\ 0 & - T_{xxxx} & 0 \\ 0 & 0 & 0 \\ 0 & 0 & T_{yyzz} \\ T_{zzxx} & 0 & 0 \\ 0 & - T_{yyzz} - T_{zzxx} & 0 \\ 0 & T_{yzzy} & 0 \\ 0 & 0 & T_{zxxz} \\ - T_{yzzy} - T_{zxxz} & 0 & 0 \\ 0 & 0 & 0 \end{bmatrix}
\end{align*}
\begin{align*}
& T_{xxxx} = 2 T_{dv}^{(1)} + 4 T_{dv}^{(2)} + T_{gv}^{(1)} \\
& T_{yyzz} = - T_{dv}^{(1)} + T_{dv}^{(3)} + T_{gv}^{(1)} \\
& T_{zzxx} = T_{dv}^{(1)} + T_{dv}^{(3)} - T_{gv}^{(1)} \\
& T_{yzzy} = - T_{dv}^{(2)} + T_{dv}^{(5)} + T_{gv}^{(1)} \\
& T_{zxxz} = T_{dv}^{(2)} + T_{dv}^{(5)} - T_{gv}^{(1)}
\end{align*}

\end{document}
