\documentclass[fleqn,8pt,landscape]{jsarticle}
\special{papersize=\the\paperwidth,\the\paperheight}

%%% package

\usepackage[usenames]{color}
\usepackage{amsmath}
\usepackage{breqn}
\usepackage{graphicx}
\usepackage{amssymb}
\usepackage{bm}
\usepackage{enumitem}
\usepackage{braket}
\usepackage{multirow}
\usepackage{booktabs}
\usepackage{longtable}

%%% layout setting

\paperwidth=356.4truemm
\paperheight=252.0truemm
\textwidth=335.59999999999997truemm
\textheight=224.2truemm
\oddsidemargin=-15truemm
\topmargin=-15truemm
\footskip=7truemm

%%% fixed

\hoffset=0truemm
\voffset=0truemm
\headheight=0truemm
\headsep=0truemm
\marginparsep=0truemm
\marginparwidth=0truemm

%%% main text

\begin{document}

\setcounter{MaxMatrixCols}{32}

\renewcommand{\tablename}{Table~}
\renewcommand{\figurename}{Figure~}
\begin{center}
\LARGE
MPG No. 3.3.8\quad$2'$\quad[ Type III, monoclinic ] [M tensor]
\end{center}
* Rank 0 tensor.
* Rank 1 tensor.
\begin{align*}
\begin{bmatrix} M_{x} & 0 & M_{z} \end{bmatrix}
\end{align*}
\begin{align*}
& M_{x} = M_{px}^{(1)} \\
& M_{z} = M_{pz}^{(1)}
\end{align*}
* Rank 2 tensor (s).
\begin{align*}
\begin{bmatrix} 0 & M_{xy} & 0 \\ M_{xy} & 0 & M_{yz} \\ 0 & M_{yz} & 0 \end{bmatrix}
\end{align*}
\begin{align*}
& M_{xy} = M_{dxy}^{(1)} \\
& M_{yz} = M_{dyz}^{(1)}
\end{align*}
* Rank 2 tensor (a).
\begin{align*}
\begin{bmatrix} 0 & M_{xy} & 0 \\ - M_{xy} & 0 & M_{yz} \\ 0 & - M_{yz} & 0 \end{bmatrix}
\end{align*}
\begin{align*}
& M_{xy} = T_{pz}^{(1)} \\
& M_{yz} = T_{px}^{(1)}
\end{align*}
* Rank 3 tensor (s).
\begin{align*}
\begin{bmatrix} M_{xxx} & 0 & M_{xxz} \\ M_{yyx} & 0 & M_{yyz} \\ M_{zzx} & 0 & M_{zzz} \\ 0 & M_{yzy} & 0 \\ M_{zxx} & 0 & M_{zxz} \\ 0 & M_{xyy} & 0 \end{bmatrix}
\end{align*}
\begin{align*}
& M_{xxx} = 2 M_{fax}^{(1)} + M_{px}^{(1)} + 2 M_{px}^{(2)} \\
& M_{xxz} = - M_{faz}^{(1)} + M_{fbz}^{(1)} + M_{pz}^{(1)} - 2 T_{dxy}^{(1)} \\
& M_{yyx} = - M_{fax}^{(1)} + M_{fbx}^{(1)} + M_{px}^{(1)} - 2 T_{dyz}^{(1)} \\
& M_{yyz} = - M_{faz}^{(1)} - M_{fbz}^{(1)} + M_{pz}^{(1)} + 2 T_{dxy}^{(1)} \\
& M_{zzx} = - M_{fax}^{(1)} - M_{fbx}^{(1)} + M_{px}^{(1)} + 2 T_{dyz}^{(1)} \\
& M_{zzz} = 2 M_{faz}^{(1)} + M_{pz}^{(1)} + 2 M_{pz}^{(2)} \\
& M_{yzy} = - M_{faz}^{(1)} - M_{fbz}^{(1)} + M_{pz}^{(2)} - T_{dxy}^{(1)} \\
& M_{zxx} = - M_{faz}^{(1)} + M_{fbz}^{(1)} + M_{pz}^{(2)} + T_{dxy}^{(1)} \\
& M_{zxz} = - M_{fax}^{(1)} - M_{fbx}^{(1)} + M_{px}^{(2)} - T_{dyz}^{(1)} \\
& M_{xyy} = - M_{fax}^{(1)} + M_{fbx}^{(1)} + M_{px}^{(2)} + T_{dyz}^{(1)}
\end{align*}
* Rank 3 tensor (a).
\begin{align*}
\begin{bmatrix} 0 & M_{yzy} & 0 \\ M_{zxx} & 0 & M_{zxz} \\ 0 & M_{xyy} & 0 \end{bmatrix}
\end{align*}
\begin{align*}
& M_{yzy} = M_{pz}^{(3)} + T_{dxy}^{(2)} \\
& M_{zxx} = - M_{pz}^{(3)} + T_{dxy}^{(2)} \\
& M_{zxz} = M_{px}^{(3)} + T_{dyz}^{(2)} \\
& M_{xyy} = - M_{px}^{(3)} + T_{dyz}^{(2)}
\end{align*}
* Rank 4 tensor (sss).
\begin{align*}
\begin{bmatrix} 0 & 0 & 0 & M_{xxyz} & 0 & M_{xxxy} \\ 0 & 0 & 0 & M_{yyyz} & 0 & M_{yyxy} \\ 0 & 0 & 0 & M_{zzyz} & 0 & M_{zzxy} \\ M_{xxyz} & M_{yyyz} & M_{zzyz} & 0 & M_{yzzx} & 0 \\ 0 & 0 & 0 & M_{yzzx} & 0 & M_{zxxy} \\ M_{xxxy} & M_{yyxy} & M_{zzxy} & 0 & M_{zxxy} & 0 \end{bmatrix}
\end{align*}
\begin{align*}
& M_{xxyz} = M_{dyz}^{(1)} + 2 M_{gbx}^{(1)} \\
& M_{xxxy} = M_{dxy}^{(1)} + 2 M_{dxy}^{(2)} + M_{gaz}^{(1)} - M_{gbz}^{(1)} \\
& M_{yyyz} = M_{dyz}^{(1)} + 2 M_{dyz}^{(2)} + M_{gax}^{(1)} - M_{gbx}^{(1)} \\
& M_{yyxy} = M_{dxy}^{(1)} + 2 M_{dxy}^{(2)} - M_{gaz}^{(1)} - M_{gbz}^{(1)} \\
& M_{zzyz} = M_{dyz}^{(1)} + 2 M_{dyz}^{(2)} - M_{gax}^{(1)} - M_{gbx}^{(1)} \\
& M_{zzxy} = M_{dxy}^{(1)} + 2 M_{gbz}^{(1)} \\
& M_{yzzx} = M_{dxy}^{(2)} + 2 M_{gbz}^{(1)} \\
& M_{zxxy} = M_{dyz}^{(2)} + 2 M_{gbx}^{(1)}
\end{align*}
* Rank 4 tensor (ssa).
\begin{align*}
\begin{bmatrix} 0 & 0 & 0 & M_{xxyz} & 0 & M_{xxxy} \\ 0 & 0 & 0 & M_{yyyz} & 0 & M_{yyxy} \\ 0 & 0 & 0 & M_{zzyz} & 0 & M_{zzxy} \\ - M_{xxyz} & - M_{yyyz} & - M_{zzyz} & 0 & M_{yzzx} & 0 \\ 0 & 0 & 0 & - M_{yzzx} & 0 & M_{zxxy} \\ - M_{xxxy} & - M_{yyxy} & - M_{zzxy} & 0 & - M_{zxxy} & 0 \end{bmatrix}
\end{align*}
\begin{align*}
& M_{xxyz} = M_{dyz}^{(3)} - 4 T_{fbx}^{(1)} \\
& M_{xxxy} = M_{dxy}^{(3)} - 2 T_{faz}^{(1)} + 2 T_{fbz}^{(1)} + 2 T_{pz}^{(1)} \\
& M_{yyyz} = M_{dyz}^{(3)} - 2 T_{fax}^{(1)} + 2 T_{fbx}^{(1)} + 2 T_{px}^{(1)} \\
& M_{yyxy} = M_{dxy}^{(3)} + 2 T_{faz}^{(1)} + 2 T_{fbz}^{(1)} - 2 T_{pz}^{(1)} \\
& M_{zzyz} = M_{dyz}^{(3)} + 2 T_{fax}^{(1)} + 2 T_{fbx}^{(1)} - 2 T_{px}^{(1)} \\
& M_{zzxy} = M_{dxy}^{(3)} - 4 T_{fbz}^{(1)} \\
& M_{yzzx} = - 4 T_{faz}^{(1)} - T_{pz}^{(1)} \\
& M_{zxxy} = - 4 T_{fax}^{(1)} - T_{px}^{(1)}
\end{align*}
* Rank 4 tensor (aas).
\begin{align*}
\begin{bmatrix} 0 & M_{yzzx} & 0 \\ M_{yzzx} & 0 & M_{zxxy} \\ 0 & M_{zxxy} & 0 \end{bmatrix}
\end{align*}
\begin{align*}
& M_{yzzx} = 2 M_{dxy}^{(4)} \\
& M_{zxxy} = 2 M_{dyz}^{(4)}
\end{align*}
* Rank 4 tensor (aaa).
\begin{align*}
\begin{bmatrix} 0 & M_{yzzx} & 0 \\ - M_{yzzx} & 0 & M_{zxxy} \\ 0 & - M_{zxxy} & 0 \end{bmatrix}
\end{align*}
\begin{align*}
& M_{yzzx} = - T_{pz}^{(2)} \\
& M_{zxxy} = - T_{px}^{(2)}
\end{align*}
* Rank 4 tensor (sa).
\begin{align*}
\begin{bmatrix} M_{xxyz} & 0 & M_{xxxy} \\ M_{yyyz} & 0 & M_{yyxy} \\ M_{zzyz} & 0 & M_{zzxy} \\ 0 & M_{yzzx} & 0 \\ M_{zxyz} & 0 & M_{zxxy} \\ 0 & M_{xyzx} & 0 \end{bmatrix}
\end{align*}
\begin{align*}
& M_{xxyz} = 2 T_{fax}^{(2)} + T_{px}^{(3)} + 2 T_{px}^{(4)} \\
& M_{xxxy} = - 2 M_{dxy}^{(5)} - T_{faz}^{(2)} + T_{fbz}^{(2)} + T_{pz}^{(3)} \\
& M_{yyyz} = - 2 M_{dyz}^{(5)} - T_{fax}^{(2)} + T_{fbx}^{(2)} + T_{px}^{(3)} \\
& M_{yyxy} = 2 M_{dxy}^{(5)} - T_{faz}^{(2)} - T_{fbz}^{(2)} + T_{pz}^{(3)} \\
& M_{zzyz} = 2 M_{dyz}^{(5)} - T_{fax}^{(2)} - T_{fbx}^{(2)} + T_{px}^{(3)} \\
& M_{zzxy} = 2 T_{faz}^{(2)} + T_{pz}^{(3)} + 2 T_{pz}^{(4)} \\
& M_{yzzx} = - M_{dxy}^{(5)} - T_{faz}^{(2)} - T_{fbz}^{(2)} + T_{pz}^{(4)} \\
& M_{zxyz} = M_{dxy}^{(5)} - T_{faz}^{(2)} + T_{fbz}^{(2)} + T_{pz}^{(4)} \\
& M_{zxxy} = - M_{dyz}^{(5)} - T_{fax}^{(2)} - T_{fbx}^{(2)} + T_{px}^{(4)} \\
& M_{xyzx} = M_{dyz}^{(5)} - T_{fax}^{(2)} + T_{fbx}^{(2)} + T_{px}^{(4)}
\end{align*}
* Rank 4 tensor (as).
\begin{align*}
\begin{bmatrix} M_{yzxx} & M_{yzyy} & M_{yzzz} & 0 & M_{yzzx} & 0 \\ 0 & 0 & 0 & M_{zxyz} & 0 & M_{zxxy} \\ M_{xyxx} & M_{xyyy} & M_{xyzz} & 0 & M_{xyzx} & 0 \end{bmatrix}
\end{align*}
\begin{align*}
& M_{yzxx} = 2 T_{fax}^{(3)} + T_{px}^{(5)} + 2 T_{px}^{(6)} \\
& M_{yzyy} = - 2 M_{dyz}^{(6)} - T_{fax}^{(3)} + T_{fbx}^{(3)} + T_{px}^{(5)} \\
& M_{yzzz} = 2 M_{dyz}^{(6)} - T_{fax}^{(3)} - T_{fbx}^{(3)} + T_{px}^{(5)} \\
& M_{yzzx} = M_{dxy}^{(6)} - T_{faz}^{(3)} + T_{fbz}^{(3)} + T_{pz}^{(6)} \\
& M_{zxyz} = - M_{dxy}^{(6)} - T_{faz}^{(3)} - T_{fbz}^{(3)} + T_{pz}^{(6)} \\
& M_{zxxy} = M_{dyz}^{(6)} - T_{fax}^{(3)} + T_{fbx}^{(3)} + T_{px}^{(6)} \\
& M_{xyxx} = - 2 M_{dxy}^{(6)} - T_{faz}^{(3)} + T_{fbz}^{(3)} + T_{pz}^{(5)} \\
& M_{xyyy} = 2 M_{dxy}^{(6)} - T_{faz}^{(3)} - T_{fbz}^{(3)} + T_{pz}^{(5)} \\
& M_{xyzz} = 2 T_{faz}^{(3)} + T_{pz}^{(5)} + 2 T_{pz}^{(6)} \\
& M_{xyzx} = - M_{dyz}^{(6)} - T_{fax}^{(3)} - T_{fbx}^{(3)} + T_{px}^{(6)}
\end{align*}
* Rank 4 tensor (s).
\begin{align*}
\begin{bmatrix} 0 & 0 & 0 & M_{xxyz} & 0 & M_{xxxy} & M_{xxzy} & 0 & M_{xxyx} \\ 0 & 0 & 0 & M_{yyyz} & 0 & M_{yyxy} & M_{yyzy} & 0 & M_{yyyx} \\ 0 & 0 & 0 & M_{zzyz} & 0 & M_{zzxy} & M_{zzzy} & 0 & M_{zzyx} \\ M_{yzxx} & M_{yzyy} & M_{yzzz} & 0 & M_{yzzx} & 0 & 0 & M_{yzxz} & 0 \\ 0 & 0 & 0 & M_{zxyz} & 0 & M_{zxxy} & M_{zxzy} & 0 & M_{zxyx} \\ M_{xyxx} & M_{xyyy} & M_{xyzz} & 0 & M_{xyzx} & 0 & 0 & M_{xyxz} & 0 \end{bmatrix}
\end{align*}
\begin{align*}
& M_{xxyz} = M_{dyz}^{(1)} + M_{dyz}^{(3)} + 2 M_{gbx}^{(1)} + 2 T_{fax}^{(2)} - 4 T_{fbx}^{(1)} + T_{px}^{(3)} + 2 T_{px}^{(4)} \\
& M_{xxxy} = M_{dxy}^{(1)} + 2 M_{dxy}^{(2)} + M_{dxy}^{(3)} - 2 M_{dxy}^{(5)} + M_{gaz}^{(1)} - M_{gbz}^{(1)} - 2 T_{faz}^{(1)} - T_{faz}^{(2)} + 2 T_{fbz}^{(1)} + T_{fbz}^{(2)} + 2 T_{pz}^{(1)} + T_{pz}^{(3)} \\
& M_{xxzy} = M_{dyz}^{(1)} + M_{dyz}^{(3)} + 2 M_{gbx}^{(1)} - 2 T_{fax}^{(2)} - 4 T_{fbx}^{(1)} - T_{px}^{(3)} - 2 T_{px}^{(4)} \\
& M_{xxyx} = M_{dxy}^{(1)} + 2 M_{dxy}^{(2)} + M_{dxy}^{(3)} + 2 M_{dxy}^{(5)} + M_{gaz}^{(1)} - M_{gbz}^{(1)} - 2 T_{faz}^{(1)} + T_{faz}^{(2)} + 2 T_{fbz}^{(1)} - T_{fbz}^{(2)} + 2 T_{pz}^{(1)} - T_{pz}^{(3)} \\
& M_{yyyz} = M_{dyz}^{(1)} + 2 M_{dyz}^{(2)} + M_{dyz}^{(3)} - 2 M_{dyz}^{(5)} + M_{gax}^{(1)} - M_{gbx}^{(1)} - 2 T_{fax}^{(1)} - T_{fax}^{(2)} + 2 T_{fbx}^{(1)} + T_{fbx}^{(2)} + 2 T_{px}^{(1)} + T_{px}^{(3)} \\
& M_{yyxy} = M_{dxy}^{(1)} + 2 M_{dxy}^{(2)} + M_{dxy}^{(3)} + 2 M_{dxy}^{(5)} - M_{gaz}^{(1)} - M_{gbz}^{(1)} + 2 T_{faz}^{(1)} - T_{faz}^{(2)} + 2 T_{fbz}^{(1)} - T_{fbz}^{(2)} - 2 T_{pz}^{(1)} + T_{pz}^{(3)} \\
& M_{yyzy} = M_{dyz}^{(1)} + 2 M_{dyz}^{(2)} + M_{dyz}^{(3)} + 2 M_{dyz}^{(5)} + M_{gax}^{(1)} - M_{gbx}^{(1)} - 2 T_{fax}^{(1)} + T_{fax}^{(2)} + 2 T_{fbx}^{(1)} - T_{fbx}^{(2)} + 2 T_{px}^{(1)} - T_{px}^{(3)} \\
& M_{yyyx} = M_{dxy}^{(1)} + 2 M_{dxy}^{(2)} + M_{dxy}^{(3)} - 2 M_{dxy}^{(5)} - M_{gaz}^{(1)} - M_{gbz}^{(1)} + 2 T_{faz}^{(1)} + T_{faz}^{(2)} + 2 T_{fbz}^{(1)} + T_{fbz}^{(2)} - 2 T_{pz}^{(1)} - T_{pz}^{(3)} \\
& M_{zzyz} = M_{dyz}^{(1)} + 2 M_{dyz}^{(2)} + M_{dyz}^{(3)} + 2 M_{dyz}^{(5)} - M_{gax}^{(1)} - M_{gbx}^{(1)} + 2 T_{fax}^{(1)} - T_{fax}^{(2)} + 2 T_{fbx}^{(1)} - T_{fbx}^{(2)} - 2 T_{px}^{(1)} + T_{px}^{(3)} \\
& M_{zzxy} = M_{dxy}^{(1)} + M_{dxy}^{(3)} + 2 M_{gbz}^{(1)} + 2 T_{faz}^{(2)} - 4 T_{fbz}^{(1)} + T_{pz}^{(3)} + 2 T_{pz}^{(4)} \\
& M_{zzzy} = M_{dyz}^{(1)} + 2 M_{dyz}^{(2)} + M_{dyz}^{(3)} - 2 M_{dyz}^{(5)} - M_{gax}^{(1)} - M_{gbx}^{(1)} + 2 T_{fax}^{(1)} + T_{fax}^{(2)} + 2 T_{fbx}^{(1)} + T_{fbx}^{(2)} - 2 T_{px}^{(1)} - T_{px}^{(3)} \\
& M_{zzyx} = M_{dxy}^{(1)} + M_{dxy}^{(3)} + 2 M_{gbz}^{(1)} - 2 T_{faz}^{(2)} - 4 T_{fbz}^{(1)} - T_{pz}^{(3)} - 2 T_{pz}^{(4)} \\
& M_{yzxx} = M_{dyz}^{(1)} - M_{dyz}^{(3)} + 2 M_{gbx}^{(1)} + 4 T_{fbx}^{(1)} \\
& M_{yzyy} = M_{dyz}^{(1)} + 2 M_{dyz}^{(2)} - M_{dyz}^{(3)} + M_{gax}^{(1)} - M_{gbx}^{(1)} + 2 T_{fax}^{(1)} - 2 T_{fbx}^{(1)} - 2 T_{px}^{(1)} \\
& M_{yzzz} = M_{dyz}^{(1)} + 2 M_{dyz}^{(2)} - M_{dyz}^{(3)} - M_{gax}^{(1)} - M_{gbx}^{(1)} - 2 T_{fax}^{(1)} - 2 T_{fbx}^{(1)} + 2 T_{px}^{(1)} \\
& M_{yzzx} = M_{dxy}^{(2)} - M_{dxy}^{(5)} + 2 M_{gbz}^{(1)} - 4 T_{faz}^{(1)} - T_{faz}^{(2)} - T_{fbz}^{(2)} - T_{pz}^{(1)} + T_{pz}^{(4)} \\
& M_{yzxz} = M_{dxy}^{(2)} + M_{dxy}^{(5)} + 2 M_{gbz}^{(1)} - 4 T_{faz}^{(1)} + T_{faz}^{(2)} + T_{fbz}^{(2)} - T_{pz}^{(1)} - T_{pz}^{(4)} \\
& M_{zxyz} = M_{dxy}^{(2)} + M_{dxy}^{(5)} + 2 M_{gbz}^{(1)} + 4 T_{faz}^{(1)} - T_{faz}^{(2)} + T_{fbz}^{(2)} + T_{pz}^{(1)} + T_{pz}^{(4)} \\
& M_{zxxy} = M_{dyz}^{(2)} - M_{dyz}^{(5)} + 2 M_{gbx}^{(1)} - 4 T_{fax}^{(1)} - T_{fax}^{(2)} - T_{fbx}^{(2)} - T_{px}^{(1)} + T_{px}^{(4)} \\
& M_{zxzy} = M_{dxy}^{(2)} - M_{dxy}^{(5)} + 2 M_{gbz}^{(1)} + 4 T_{faz}^{(1)} + T_{faz}^{(2)} - T_{fbz}^{(2)} + T_{pz}^{(1)} - T_{pz}^{(4)} \\
& M_{zxyx} = M_{dyz}^{(2)} + M_{dyz}^{(5)} + 2 M_{gbx}^{(1)} - 4 T_{fax}^{(1)} + T_{fax}^{(2)} + T_{fbx}^{(2)} - T_{px}^{(1)} - T_{px}^{(4)} \\
& M_{xyxx} = M_{dxy}^{(1)} + 2 M_{dxy}^{(2)} - M_{dxy}^{(3)} + M_{gaz}^{(1)} - M_{gbz}^{(1)} + 2 T_{faz}^{(1)} - 2 T_{fbz}^{(1)} - 2 T_{pz}^{(1)} \\
& M_{xyyy} = M_{dxy}^{(1)} + 2 M_{dxy}^{(2)} - M_{dxy}^{(3)} - M_{gaz}^{(1)} - M_{gbz}^{(1)} - 2 T_{faz}^{(1)} - 2 T_{fbz}^{(1)} + 2 T_{pz}^{(1)} \\
& M_{xyzz} = M_{dxy}^{(1)} - M_{dxy}^{(3)} + 2 M_{gbz}^{(1)} + 4 T_{fbz}^{(1)} \\
& M_{xyzx} = M_{dyz}^{(2)} + M_{dyz}^{(5)} + 2 M_{gbx}^{(1)} + 4 T_{fax}^{(1)} - T_{fax}^{(2)} + T_{fbx}^{(2)} + T_{px}^{(1)} + T_{px}^{(4)} \\
& M_{xyxz} = M_{dyz}^{(2)} - M_{dyz}^{(5)} + 2 M_{gbx}^{(1)} + 4 T_{fax}^{(1)} + T_{fax}^{(2)} - T_{fbx}^{(2)} + T_{px}^{(1)} - T_{px}^{(4)}
\end{align*}
* Rank 4 tensor (a).
\begin{align*}
\begin{bmatrix} M_{yzxx} & M_{yzyy} & M_{yzzz} & 0 & M_{yzzx} & 0 & 0 & M_{yzxz} & 0 \\ 0 & 0 & 0 & M_{zxyz} & 0 & M_{zxxy} & M_{zxzy} & 0 & M_{zxyx} \\ M_{xyxx} & M_{xyyy} & M_{xyzz} & 0 & M_{xyzx} & 0 & 0 & M_{xyxz} & 0 \end{bmatrix}
\end{align*}
\begin{align*}
& M_{yzxx} = 2 T_{fax}^{(3)} + T_{px}^{(5)} + 2 T_{px}^{(6)} \\
& M_{yzyy} = - 2 M_{dyz}^{(6)} - T_{fax}^{(3)} + T_{fbx}^{(3)} + T_{px}^{(5)} \\
& M_{yzzz} = 2 M_{dyz}^{(6)} - T_{fax}^{(3)} - T_{fbx}^{(3)} + T_{px}^{(5)} \\
& M_{yzzx} = 2 M_{dxy}^{(4)} + M_{dxy}^{(6)} - T_{faz}^{(3)} + T_{fbz}^{(3)} - T_{pz}^{(2)} + T_{pz}^{(6)} \\
& M_{yzxz} = - 2 M_{dxy}^{(4)} + M_{dxy}^{(6)} - T_{faz}^{(3)} + T_{fbz}^{(3)} + T_{pz}^{(2)} + T_{pz}^{(6)} \\
& M_{zxyz} = 2 M_{dxy}^{(4)} - M_{dxy}^{(6)} - T_{faz}^{(3)} - T_{fbz}^{(3)} + T_{pz}^{(2)} + T_{pz}^{(6)} \\
& M_{zxxy} = 2 M_{dyz}^{(4)} + M_{dyz}^{(6)} - T_{fax}^{(3)} + T_{fbx}^{(3)} - T_{px}^{(2)} + T_{px}^{(6)} \\
& M_{zxzy} = - 2 M_{dxy}^{(4)} - M_{dxy}^{(6)} - T_{faz}^{(3)} - T_{fbz}^{(3)} - T_{pz}^{(2)} + T_{pz}^{(6)} \\
& M_{zxyx} = - 2 M_{dyz}^{(4)} + M_{dyz}^{(6)} - T_{fax}^{(3)} + T_{fbx}^{(3)} + T_{px}^{(2)} + T_{px}^{(6)} \\
& M_{xyxx} = - 2 M_{dxy}^{(6)} - T_{faz}^{(3)} + T_{fbz}^{(3)} + T_{pz}^{(5)} \\
& M_{xyyy} = 2 M_{dxy}^{(6)} - T_{faz}^{(3)} - T_{fbz}^{(3)} + T_{pz}^{(5)} \\
& M_{xyzz} = 2 T_{faz}^{(3)} + T_{pz}^{(5)} + 2 T_{pz}^{(6)} \\
& M_{xyzx} = 2 M_{dyz}^{(4)} - M_{dyz}^{(6)} - T_{fax}^{(3)} - T_{fbx}^{(3)} + T_{px}^{(2)} + T_{px}^{(6)} \\
& M_{xyxz} = - 2 M_{dyz}^{(4)} - M_{dyz}^{(6)} - T_{fax}^{(3)} - T_{fbx}^{(3)} - T_{px}^{(2)} + T_{px}^{(6)}
\end{align*}
* Rank 4 tensor (t).
\begin{align*}
\begin{bmatrix} 0 & M_{xxxy} & 0 \\ M_{yyyx} & 0 & M_{yyyz} \\ 0 & M_{zzzy} & 0 \\ 0 & M_{yyzy} & 0 \\ 0 & M_{zzxy} & 0 \\ M_{xxyx} & 0 & M_{xxyz} \\ M_{yzzx} & 0 & M_{yzzz} \\ 0 & M_{zxxy} & 0 \\ 0 & M_{xyyy} & 0 \\ - \frac{M_{yyyz}}{2} + \frac{M_{yyzy}}{2} + M_{zxxy} & 0 & \frac{M_{xxxy}}{2} - \frac{M_{xxyx}}{2} + M_{xyyy} - M_{yyyx} + M_{zzxy} \end{bmatrix}
\end{align*}
\begin{align*}
& M_{xxxy} = M_{dxy}^{(1)} + 2 M_{dxy}^{(2)} + M_{dxy}^{(3)} - 2 M_{dxy}^{(5)} + M_{gaz}^{(1)} - M_{gbz}^{(1)} \\
& M_{yyyx} = M_{dxy}^{(1)} + 2 M_{dxy}^{(2)} + M_{dxy}^{(3)} - 2 M_{dxy}^{(5)} - M_{gaz}^{(1)} - M_{gbz}^{(1)} \\
& M_{yyyz} = M_{dyz}^{(1)} + 2 M_{dyz}^{(2)} + M_{dyz}^{(3)} - 2 M_{dyz}^{(5)} + M_{gax}^{(1)} - M_{gbx}^{(1)} \\
& M_{zzzy} = M_{dyz}^{(1)} + 2 M_{dyz}^{(2)} + M_{dyz}^{(3)} - 2 M_{dyz}^{(5)} - M_{gax}^{(1)} - M_{gbx}^{(1)} \\
& M_{yyzy} = M_{dyz}^{(1)} + 2 M_{dyz}^{(2)} + M_{dyz}^{(3)} + 2 M_{dyz}^{(5)} + M_{gax}^{(1)} - M_{gbx}^{(1)} \\
& M_{zzxy} = M_{dxy}^{(1)} + M_{dxy}^{(3)} + 2 M_{gbz}^{(1)} \\
& M_{xxyx} = M_{dxy}^{(1)} + 2 M_{dxy}^{(2)} + M_{dxy}^{(3)} + 2 M_{dxy}^{(5)} + M_{gaz}^{(1)} - M_{gbz}^{(1)} \\
& M_{xxyz} = M_{dyz}^{(1)} + M_{dyz}^{(3)} + 2 M_{gbx}^{(1)} \\
& M_{yzzx} = M_{dxy}^{(2)} - M_{dxy}^{(5)} + 2 M_{gbz}^{(1)} \\
& M_{yzzz} = M_{dyz}^{(1)} + 2 M_{dyz}^{(2)} - M_{dyz}^{(3)} - M_{gax}^{(1)} - M_{gbx}^{(1)} \\
& M_{zxxy} = M_{dyz}^{(2)} - M_{dyz}^{(5)} + 2 M_{gbx}^{(1)} \\
& M_{xyyy} = M_{dxy}^{(1)} + 2 M_{dxy}^{(2)} - M_{dxy}^{(3)} - M_{gaz}^{(1)} - M_{gbz}^{(1)}
\end{align*}

\end{document}
