\documentclass[fleqn,10pt]{jsarticle}

%%% package

\usepackage[usenames]{color}
\usepackage{amsmath}
\usepackage{breqn}
\usepackage{graphicx}
\usepackage{amssymb}
\usepackage{bm}
\usepackage{enumerate}
\usepackage{braket}
\usepackage{multirow}
\usepackage{booktabs}
\usepackage{longtable}

%%% layout setting

\paperwidth=210truemm
\paperheight=297truemm
\textwidth=169.2truemm
\textheight=249.2truemm
\oddsidemargin=-5truemm
\topmargin=-5truemm
\footskip=7truemm

%%% fixed

\hoffset=0truemm
\voffset=0truemm
\headheight=0truemm
\headsep=0truemm
\marginparsep=0truemm
\marginparwidth=0truemm

%%% main text

\begin{document}

\setcounter{MaxMatrixCols}{16}

\begin{center}
\LARGE
Response Tensors up to 4th rank in $O$
\end{center}
\begin{center}\LARGE --- polar tensors ---\end{center}
\begin{align*}
C^{(0,Q)} = \begin{pmatrix} C^{(0,Q)} \end{pmatrix}
\end{align*}
\begin{quote}
\begin{align*}
& C^{(0,Q)} = Q_{0}
\end{align*}
\end{quote}
\begin{align*}
S^{(2,Q)} = \begin{pmatrix} S^{(2,Q)}_{xx} & 0 & 0 \\ 0 & S^{(2,Q)}_{xx} & 0 \\ 0 & 0 & S^{(2,Q)}_{xx} \end{pmatrix}
\end{align*}
\begin{quote}
\begin{align*}
& S^{(2,Q)}_{xx} = Q_{0}
\end{align*}
\end{quote}
\begin{align*}
A^{(3,Q)} = \begin{pmatrix} A^{(3,Q)}_{4x} & 0 & 0 \\ 0 & A^{(3,Q)}_{4x} & 0 \\ 0 & 0 & A^{(3,Q)}_{4x} \end{pmatrix}
\end{align*}
\begin{quote}
\begin{align*}
& A^{(3,Q)}_{4x} = G_{0}
\end{align*}
\end{quote}
\begin{align*}
S^{(4,Q)} = \begin{pmatrix} S^{(4,Q)}_{11} & S^{(4,Q)}_{12} & S^{(4,Q)}_{12} & 0 & 0 & 0 \\ S^{(4,Q)}_{12} & S^{(4,Q)}_{11} & S^{(4,Q)}_{12} & 0 & 0 & 0 \\ S^{(4,Q)}_{12} & S^{(4,Q)}_{12} & S^{(4,Q)}_{11} & 0 & 0 & 0 \\ 0 & 0 & 0 & S^{(4,Q)}_{44} & 0 & 0 \\ 0 & 0 & 0 & 0 & S^{(4,Q)}_{44} & 0 \\ 0 & 0 & 0 & 0 & 0 & S^{(4,Q)}_{44} \end{pmatrix}
\end{align*}
\begin{quote}
\begin{align*}
& S^{(4,Q)}_{11} = Q_{0}[1] + 2 Q_{0}[2] + 2 Q_{4} \\
& S^{(4,Q)}_{12} = Q_{0}[1] - Q_{4} \\
& S^{(4,Q)}_{44} = Q_{0}[2] - Q_{4}
\end{align*}
\end{quote}
\begin{align*}
A^{(4,Q)} = \begin{pmatrix} A^{(4,Q)}_{xx} & 0 & 0 \\ 0 & A^{(4,Q)}_{xx} & 0 \\ 0 & 0 & A^{(4,Q)}_{xx} \end{pmatrix}
\end{align*}
\begin{quote}
\begin{align*}
& A^{(4,Q)}_{xx} = Q_{0}[3]
\end{align*}
\end{quote}
\newpage
\begin{center}\LARGE --- axial tensors ---\end{center}
\begin{align*}
C^{(0,G)} = \begin{pmatrix} C^{(0,G)} \end{pmatrix}
\end{align*}
\begin{quote}
\begin{align*}
& C^{(0,G)} = G_{0}
\end{align*}
\end{quote}
\begin{align*}
S^{(2,G)} = \begin{pmatrix} S^{(2,G)}_{xx} & 0 & 0 \\ 0 & S^{(2,G)}_{xx} & 0 \\ 0 & 0 & S^{(2,G)}_{xx} \end{pmatrix}
\end{align*}
\begin{quote}
\begin{align*}
& S^{(2,G)}_{xx} = G_{0}
\end{align*}
\end{quote}
\begin{align*}
A^{(3,G)} = \begin{pmatrix} A^{(3,G)}_{4x} & 0 & 0 \\ 0 & A^{(3,G)}_{4x} & 0 \\ 0 & 0 & A^{(3,G)}_{4x} \end{pmatrix}
\end{align*}
\begin{quote}
\begin{align*}
& A^{(3,G)}_{4x} = Q_{0}
\end{align*}
\end{quote}
\begin{align*}
S^{(4,G)} = \begin{pmatrix} S^{(4,G)}_{11} & S^{(4,G)}_{12} & S^{(4,G)}_{12} & 0 & 0 & 0 \\ S^{(4,G)}_{12} & S^{(4,G)}_{11} & S^{(4,G)}_{12} & 0 & 0 & 0 \\ S^{(4,G)}_{12} & S^{(4,G)}_{12} & S^{(4,G)}_{11} & 0 & 0 & 0 \\ 0 & 0 & 0 & S^{(4,G)}_{44} & 0 & 0 \\ 0 & 0 & 0 & 0 & S^{(4,G)}_{44} & 0 \\ 0 & 0 & 0 & 0 & 0 & S^{(4,G)}_{44} \end{pmatrix}
\end{align*}
\begin{quote}
\begin{align*}
& S^{(4,G)}_{11} = G_{0}[1] + 2 G_{0}[2] + 2 G_{4} \\
& S^{(4,G)}_{12} = G_{0}[1] - G_{4} \\
& S^{(4,G)}_{44} = G_{0}[2] - G_{4}
\end{align*}
\end{quote}
\begin{align*}
A^{(4,G)} = \begin{pmatrix} A^{(4,G)}_{xx} & 0 & 0 \\ 0 & A^{(4,G)}_{xx} & 0 \\ 0 & 0 & A^{(4,G)}_{xx} \end{pmatrix}
\end{align*}
\begin{quote}
\begin{align*}
& A^{(4,G)}_{xx} = G_{0}[3]
\end{align*}
\end{quote}

\end{document}
