\documentclass[fleqn,10pt]{jsarticle}

%%% package

\usepackage[usenames]{color}
\usepackage{amsmath}
\usepackage{breqn}
\usepackage{graphicx}
\usepackage{amssymb}
\usepackage{bm}
\usepackage{enumerate}
\usepackage{braket}
\usepackage{multirow}
\usepackage{booktabs}
\usepackage{longtable}

%%% layout setting

\paperwidth=210truemm
\paperheight=297truemm
\textwidth=169.2truemm
\textheight=249.2truemm
\oddsidemargin=-5truemm
\topmargin=-5truemm
\footskip=7truemm

%%% fixed

\hoffset=0truemm
\voffset=0truemm
\headheight=0truemm
\headsep=0truemm
\marginparsep=0truemm
\marginparwidth=0truemm

%%% main text

\begin{document}

\setcounter{MaxMatrixCols}{16}

\begin{center}
\LARGE
Response Tensors up to 4th rank in $C_{i}$
\end{center}
\begin{center}\LARGE --- polar tensors ---\end{center}
\begin{align*}
C^{(0,Q)} = \begin{pmatrix} C^{(0,Q)} \end{pmatrix}
\end{align*}
\begin{quote}
\begin{align*}
& C^{(0,Q)} = Q_{0}
\end{align*}
\end{quote}
\begin{align*}
S^{(2,Q)} = \begin{pmatrix} S^{(2,Q)}_{xx} & S^{(2,Q)}_{xy} & S^{(2,Q)}_{xz} \\ S^{(2,Q)}_{xy} & S^{(2,Q)}_{yy} & S^{(2,Q)}_{yz} \\ S^{(2,Q)}_{xz} & S^{(2,Q)}_{yz} & S^{(2,Q)}_{zz} \end{pmatrix}
\end{align*}
\begin{quote}
\begin{align*}
& S^{(2,Q)}_{xx} = Q_{0} - Q_{u} + Q_{v} \\
& S^{(2,Q)}_{xy} = Q_{xy} \\
& S^{(2,Q)}_{xz} = Q_{zx} \\
& S^{(2,Q)}_{yy} = Q_{0} - Q_{u} - Q_{v} \\
& S^{(2,Q)}_{yz} = Q_{yz} \\
& S^{(2,Q)}_{zz} = Q_{0} + 2 Q_{u}
\end{align*}
\end{quote}
\begin{align*}
A^{(2,Q)} = \begin{pmatrix} 0 & A^{(2,Q)}_{xy} & A^{(2,Q)}_{xz} \\ - A^{(2,Q)}_{xy} & 0 & A^{(2,Q)}_{yz} \\ - A^{(2,Q)}_{xz} & - A^{(2,Q)}_{yz} & 0 \end{pmatrix}
\end{align*}
\begin{quote}
\begin{align*}
& A^{(2,Q)}_{xy} = G_{z} \\
& A^{(2,Q)}_{xz} = - G_{y} \\
& A^{(2,Q)}_{yz} = G_{x}
\end{align*}
\end{quote}
\begin{align*}
S^{(4,Q)} = \begin{pmatrix} S^{(4,Q)}_{11} & S^{(4,Q)}_{12} & S^{(4,Q)}_{13} & S^{(4,Q)}_{14} & S^{(4,Q)}_{15} & S^{(4,Q)}_{16} \\ S^{(4,Q)}_{12} & S^{(4,Q)}_{22} & S^{(4,Q)}_{23} & S^{(4,Q)}_{24} & S^{(4,Q)}_{25} & S^{(4,Q)}_{26} \\ S^{(4,Q)}_{13} & S^{(4,Q)}_{23} & S^{(4,Q)}_{33} & S^{(4,Q)}_{34} & S^{(4,Q)}_{35} & S^{(4,Q)}_{36} \\ S^{(4,Q)}_{14} & S^{(4,Q)}_{24} & S^{(4,Q)}_{34} & S^{(4,Q)}_{44} & S^{(4,Q)}_{45} & S^{(4,Q)}_{46} \\ S^{(4,Q)}_{15} & S^{(4,Q)}_{25} & S^{(4,Q)}_{35} & S^{(4,Q)}_{45} & S^{(4,Q)}_{55} & S^{(4,Q)}_{56} \\ S^{(4,Q)}_{16} & S^{(4,Q)}_{26} & S^{(4,Q)}_{36} & S^{(4,Q)}_{46} & S^{(4,Q)}_{56} & S^{(4,Q)}_{66} \end{pmatrix}
\end{align*}
\begin{quote}
\begin{align*}
& S^{(4,Q)}_{11} = Q_{0}[1] + 2 Q_{0}[2] - Q_{4u} + Q_{4v} + 2 Q_{4} - 2 Q_{u}[1] - 4 Q_{u}[2] + 2 Q_{v}[1] + 4 Q_{v}[2] \\
& S^{(4,Q)}_{12} = Q_{0}[1] + 2 Q_{4u} - Q_{4} - 2 Q_{u}[1] \\
& S^{(4,Q)}_{13} = Q_{0}[1] - Q_{4u} - Q_{4v} - Q_{4} + Q_{u}[1] + Q_{v}[1] \\
& S^{(4,Q)}_{14} = 2 Q_{4x}^{\beta} + Q_{yz}[1] \\
& S^{(4,Q)}_{15} = - Q_{4y}^{\alpha} - Q_{4y}^{\beta} + Q_{zx}[1] + 2 Q_{zx}[2] \\
& S^{(4,Q)}_{16} = Q_{4z}^{\alpha} - Q_{4z}^{\beta} + Q_{xy}[1] + 2 Q_{xy}[2] \\
& S^{(4,Q)}_{22} = Q_{0}[1] + 2 Q_{0}[2] - Q_{4u} - Q_{4v} + 2 Q_{4} - 2 Q_{u}[1] - 4 Q_{u}[2] - 2 Q_{v}[1] - 4 Q_{v}[2] \\
& S^{(4,Q)}_{23} = Q_{0}[1] - Q_{4u} + Q_{4v} - Q_{4} + Q_{u}[1] - Q_{v}[1] \\
& S^{(4,Q)}_{24} = Q_{4x}^{\alpha} - Q_{4x}^{\beta} + Q_{yz}[1] + 2 Q_{yz}[2] \\
& S^{(4,Q)}_{25} = 2 Q_{4y}^{\beta} + Q_{zx}[1] \\
& S^{(4,Q)}_{26} = - Q_{4z}^{\alpha} - Q_{4z}^{\beta} + Q_{xy}[1] + 2 Q_{xy}[2] \\
& S^{(4,Q)}_{33} = Q_{0}[1] + 2 Q_{0}[2] + 2 Q_{4u} + 2 Q_{4} + 4 Q_{u}[1] + 8 Q_{u}[2] \\
& S^{(4,Q)}_{34} = - Q_{4x}^{\alpha} - Q_{4x}^{\beta} + Q_{yz}[1] + 2 Q_{yz}[2] \\
& S^{(4,Q)}_{35} = Q_{4y}^{\alpha} - Q_{4y}^{\beta} + Q_{zx}[1] + 2 Q_{zx}[2] \\
& S^{(4,Q)}_{36} = 2 Q_{4z}^{\beta} + Q_{xy}[1] \\
& S^{(4,Q)}_{44} = Q_{0}[2] - Q_{4u} + Q_{4v} - Q_{4} + Q_{u}[2] - Q_{v}[2] \\
& S^{(4,Q)}_{45} = 2 Q_{4z}^{\beta} + Q_{xy}[2] \\
& S^{(4,Q)}_{46} = 2 Q_{4y}^{\beta} + Q_{zx}[2] \\
& S^{(4,Q)}_{55} = Q_{0}[2] - Q_{4u} - Q_{4v} - Q_{4} + Q_{u}[2] + Q_{v}[2] \\
& S^{(4,Q)}_{56} = 2 Q_{4x}^{\beta} + Q_{yz}[2] \\
& S^{(4,Q)}_{66} = Q_{0}[2] + 2 Q_{4u} - Q_{4} - 2 Q_{u}[2]
\end{align*}
\end{quote}
\begin{align*}
\bar{S}^{(4,Q)} = \begin{pmatrix} 0 & \bar{S}^{(4,Q)}_{12} & \bar{S}^{(4,Q)}_{13} & \bar{S}^{(4,Q)}_{14} & \bar{S}^{(4,Q)}_{15} & \bar{S}^{(4,Q)}_{16} \\ - \bar{S}^{(4,Q)}_{12} & 0 & \bar{S}^{(4,Q)}_{23} & \bar{S}^{(4,Q)}_{24} & \bar{S}^{(4,Q)}_{25} & \bar{S}^{(4,Q)}_{26} \\ - \bar{S}^{(4,Q)}_{13} & - \bar{S}^{(4,Q)}_{23} & 0 & \bar{S}^{(4,Q)}_{34} & \bar{S}^{(4,Q)}_{35} & \bar{S}^{(4,Q)}_{36} \\ - \bar{S}^{(4,Q)}_{14} & - \bar{S}^{(4,Q)}_{24} & - \bar{S}^{(4,Q)}_{34} & 0 & \bar{S}^{(4,Q)}_{45} & \bar{S}^{(4,Q)}_{46} \\ - \bar{S}^{(4,Q)}_{15} & - \bar{S}^{(4,Q)}_{25} & - \bar{S}^{(4,Q)}_{35} & - \bar{S}^{(4,Q)}_{45} & 0 & \bar{S}^{(4,Q)}_{56} \\ - \bar{S}^{(4,Q)}_{16} & - \bar{S}^{(4,Q)}_{26} & - \bar{S}^{(4,Q)}_{36} & - \bar{S}^{(4,Q)}_{46} & - \bar{S}^{(4,Q)}_{56} & 0 \end{pmatrix}
\end{align*}
\begin{quote}
\begin{align*}
& \bar{S}^{(4,Q)}_{12} = 4 G_{xyz}[1] - 2 Q_{v}[3] \\
& \bar{S}^{(4,Q)}_{13} = - 4 G_{xyz}[1] + 3 Q_{u}[3] - Q_{v}[3] \\
& \bar{S}^{(4,Q)}_{14} = - 4 G_{x}^{\beta}[1] + Q_{yz}[3] \\
& \bar{S}^{(4,Q)}_{15} = - 2 G_{y}[1] + 2 G_{y}^{\alpha}[1] + 2 G_{y}^{\beta}[1] + Q_{zx}[3] \\
& \bar{S}^{(4,Q)}_{16} = 2 G_{z}[1] - 2 G_{z}^{\alpha}[1] + 2 G_{z}^{\beta}[1] + Q_{xy}[3] \\
& \bar{S}^{(4,Q)}_{23} = 4 G_{xyz}[1] + 3 Q_{u}[3] + Q_{v}[3] \\
& \bar{S}^{(4,Q)}_{24} = 2 G_{x}[1] - 2 G_{x}^{\alpha}[1] + 2 G_{x}^{\beta}[1] + Q_{yz}[3] \\
& \bar{S}^{(4,Q)}_{25} = - 4 G_{y}^{\beta}[1] + Q_{zx}[3] \\
& \bar{S}^{(4,Q)}_{26} = - 2 G_{z}[1] + 2 G_{z}^{\alpha}[1] + 2 G_{z}^{\beta}[1] + Q_{xy}[3] \\
& \bar{S}^{(4,Q)}_{34} = - 2 G_{x}[1] + 2 G_{x}^{\alpha}[1] + 2 G_{x}^{\beta}[1] + Q_{yz}[3] \\
& \bar{S}^{(4,Q)}_{35} = 2 G_{y}[1] - 2 G_{y}^{\alpha}[1] + 2 G_{y}^{\beta}[1] + Q_{zx}[3] \\
& \bar{S}^{(4,Q)}_{36} = - 4 G_{z}^{\beta}[1] + Q_{xy}[3] \\
& \bar{S}^{(4,Q)}_{45} = - G_{z}[1] - 4 G_{z}^{\alpha}[1] \\
& \bar{S}^{(4,Q)}_{46} = G_{y}[1] + 4 G_{y}^{\alpha}[1] \\
& \bar{S}^{(4,Q)}_{56} = - G_{x}[1] - 4 G_{x}^{\alpha}[1]
\end{align*}
\end{quote}
\begin{align*}
A^{(4,Q)} = \begin{pmatrix} A^{(4,Q)}_{xx} & A^{(4,Q)}_{xy} & A^{(4,Q)}_{xz} \\ A^{(4,Q)}_{xy} & A^{(4,Q)}_{yy} & A^{(4,Q)}_{yz} \\ A^{(4,Q)}_{xz} & A^{(4,Q)}_{yz} & A^{(4,Q)}_{zz} \end{pmatrix}
\end{align*}
\begin{quote}
\begin{align*}
& A^{(4,Q)}_{xx} = Q_{0}[3] - 2 Q_{u}[6] + 2 Q_{v}[6] \\
& A^{(4,Q)}_{xy} = 2 Q_{xy}[6] \\
& A^{(4,Q)}_{xz} = 2 Q_{zx}[6] \\
& A^{(4,Q)}_{yy} = Q_{0}[3] - 2 Q_{u}[6] - 2 Q_{v}[6] \\
& A^{(4,Q)}_{yz} = 2 Q_{yz}[6] \\
& A^{(4,Q)}_{zz} = Q_{0}[3] + 4 Q_{u}[6]
\end{align*}
\end{quote}
\begin{align*}
\bar{A}^{(4,Q)} = \begin{pmatrix} 0 & \bar{A}^{(4,Q)}_{xy} & \bar{A}^{(4,Q)}_{xz} \\ - \bar{A}^{(4,Q)}_{xy} & 0 & \bar{A}^{(4,Q)}_{yz} \\ - \bar{A}^{(4,Q)}_{xz} & - \bar{A}^{(4,Q)}_{yz} & 0 \end{pmatrix}
\end{align*}
\begin{quote}
\begin{align*}
& \bar{A}^{(4,Q)}_{xy} = G_{z}[6] \\
& \bar{A}^{(4,Q)}_{xz} = - G_{y}[6] \\
& \bar{A}^{(4,Q)}_{yz} = G_{x}[6]
\end{align*}
\end{quote}
\begin{align*}
M^{(4,Q)} = \begin{pmatrix} M^{(4,Q)}_{1x} & M^{(4,Q)}_{1y} & M^{(4,Q)}_{1z} \\ M^{(4,Q)}_{2x} & M^{(4,Q)}_{2y} & M^{(4,Q)}_{2z} \\ M^{(4,Q)}_{3x} & M^{(4,Q)}_{3y} & M^{(4,Q)}_{3z} \\ M^{(4,Q)}_{4x} & M^{(4,Q)}_{4y} & M^{(4,Q)}_{4z} \\ M^{(4,Q)}_{5x} & M^{(4,Q)}_{5y} & M^{(4,Q)}_{5z} \\ M^{(4,Q)}_{6x} & M^{(4,Q)}_{6y} & M^{(4,Q)}_{6z} \end{pmatrix}
\end{align*}
\begin{quote}
\begin{align*}
& M^{(4,Q)}_{1x} = 2 G_{x}[2] + G_{x}[3] + 2 G_{x}^{\alpha}[2] \\
& M^{(4,Q)}_{1y} = G_{y}[3] - G_{y}^{\alpha}[2] - G_{y}^{\beta}[2] + 2 Q_{zx}[4] \\
& M^{(4,Q)}_{1z} = G_{z}[3] - G_{z}^{\alpha}[2] + G_{z}^{\beta}[2] - 2 Q_{xy}[4] \\
& M^{(4,Q)}_{2x} = G_{x}[3] - G_{x}^{\alpha}[2] + G_{x}^{\beta}[2] - 2 Q_{yz}[4] \\
& M^{(4,Q)}_{2y} = 2 G_{y}[2] + G_{y}[3] + 2 G_{y}^{\alpha}[2] \\
& M^{(4,Q)}_{2z} = G_{z}[3] - G_{z}^{\alpha}[2] - G_{z}^{\beta}[2] + 2 Q_{xy}[4] \\
& M^{(4,Q)}_{3x} = G_{x}[3] - G_{x}^{\alpha}[2] - G_{x}^{\beta}[2] + 2 Q_{yz}[4] \\
& M^{(4,Q)}_{3y} = G_{y}[3] - G_{y}^{\alpha}[2] + G_{y}^{\beta}[2] - 2 Q_{zx}[4] \\
& M^{(4,Q)}_{3z} = 2 G_{z}[2] + G_{z}[3] + 2 G_{z}^{\alpha}[2] \\
& M^{(4,Q)}_{4x} = G_{xyz}[2] - 3 Q_{u}[4] - Q_{v}[4] \\
& M^{(4,Q)}_{4y} = G_{z}[2] - G_{z}^{\alpha}[2] - G_{z}^{\beta}[2] - Q_{xy}[4] \\
& M^{(4,Q)}_{4z} = G_{y}[2] - G_{y}^{\alpha}[2] + G_{y}^{\beta}[2] + Q_{zx}[4] \\
& M^{(4,Q)}_{5x} = G_{z}[2] - G_{z}^{\alpha}[2] + G_{z}^{\beta}[2] + Q_{xy}[4] \\
& M^{(4,Q)}_{5y} = G_{xyz}[2] + 3 Q_{u}[4] - Q_{v}[4] \\
& M^{(4,Q)}_{5z} = G_{x}[2] - G_{x}^{\alpha}[2] - G_{x}^{\beta}[2] - Q_{yz}[4] \\
& M^{(4,Q)}_{6x} = G_{y}[2] - G_{y}^{\alpha}[2] - G_{y}^{\beta}[2] - Q_{zx}[4] \\
& M^{(4,Q)}_{6y} = G_{x}[2] - G_{x}^{\alpha}[2] + G_{x}^{\beta}[2] + Q_{yz}[4] \\
& M^{(4,Q)}_{6z} = G_{xyz}[2] + 2 Q_{v}[4]
\end{align*}
\end{quote}
\begin{align*}
\bar{M}^{(4,Q)} = \begin{pmatrix} \bar{M}^{(4,Q)}_{x1} & \bar{M}^{(4,Q)}_{x2} & \bar{M}^{(4,Q)}_{x3} & \bar{M}^{(4,Q)}_{x4} & \bar{M}^{(4,Q)}_{x5} & \bar{M}^{(4,Q)}_{x6} \\ \bar{M}^{(4,Q)}_{y1} & \bar{M}^{(4,Q)}_{y2} & \bar{M}^{(4,Q)}_{y3} & \bar{M}^{(4,Q)}_{y4} & \bar{M}^{(4,Q)}_{y5} & \bar{M}^{(4,Q)}_{y6} \\ \bar{M}^{(4,Q)}_{z1} & \bar{M}^{(4,Q)}_{z2} & \bar{M}^{(4,Q)}_{z3} & \bar{M}^{(4,Q)}_{z4} & \bar{M}^{(4,Q)}_{z5} & \bar{M}^{(4,Q)}_{z6} \end{pmatrix}
\end{align*}
\begin{quote}
\begin{align*}
& \bar{M}^{(4,Q)}_{x1} = 2 G_{x}[4] + G_{x}[5] + 2 G_{x}^{\alpha}[3] \\
& \bar{M}^{(4,Q)}_{x2} = G_{x}[5] - G_{x}^{\alpha}[3] + G_{x}^{\beta}[3] - 2 Q_{yz}[5] \\
& \bar{M}^{(4,Q)}_{x3} = G_{x}[5] - G_{x}^{\alpha}[3] - G_{x}^{\beta}[3] + 2 Q_{yz}[5] \\
& \bar{M}^{(4,Q)}_{x4} = G_{xyz}[3] - 3 Q_{u}[5] - Q_{v}[5] \\
& \bar{M}^{(4,Q)}_{x5} = G_{z}[4] - G_{z}^{\alpha}[3] + G_{z}^{\beta}[3] + Q_{xy}[5] \\
& \bar{M}^{(4,Q)}_{x6} = G_{y}[4] - G_{y}^{\alpha}[3] - G_{y}^{\beta}[3] - Q_{zx}[5] \\
& \bar{M}^{(4,Q)}_{y1} = G_{y}[5] - G_{y}^{\alpha}[3] - G_{y}^{\beta}[3] + 2 Q_{zx}[5] \\
& \bar{M}^{(4,Q)}_{y2} = 2 G_{y}[4] + G_{y}[5] + 2 G_{y}^{\alpha}[3] \\
& \bar{M}^{(4,Q)}_{y3} = G_{y}[5] - G_{y}^{\alpha}[3] + G_{y}^{\beta}[3] - 2 Q_{zx}[5] \\
& \bar{M}^{(4,Q)}_{y4} = G_{z}[4] - G_{z}^{\alpha}[3] - G_{z}^{\beta}[3] - Q_{xy}[5] \\
& \bar{M}^{(4,Q)}_{y5} = G_{xyz}[3] + 3 Q_{u}[5] - Q_{v}[5] \\
& \bar{M}^{(4,Q)}_{y6} = G_{x}[4] - G_{x}^{\alpha}[3] + G_{x}^{\beta}[3] + Q_{yz}[5] \\
& \bar{M}^{(4,Q)}_{z1} = G_{z}[5] - G_{z}^{\alpha}[3] + G_{z}^{\beta}[3] - 2 Q_{xy}[5] \\
& \bar{M}^{(4,Q)}_{z2} = G_{z}[5] - G_{z}^{\alpha}[3] - G_{z}^{\beta}[3] + 2 Q_{xy}[5] \\
& \bar{M}^{(4,Q)}_{z3} = 2 G_{z}[4] + G_{z}[5] + 2 G_{z}^{\alpha}[3] \\
& \bar{M}^{(4,Q)}_{z4} = G_{y}[4] - G_{y}^{\alpha}[3] + G_{y}^{\beta}[3] + Q_{zx}[5] \\
& \bar{M}^{(4,Q)}_{z5} = G_{x}[4] - G_{x}^{\alpha}[3] - G_{x}^{\beta}[3] - Q_{yz}[5] \\
& \bar{M}^{(4,Q)}_{z6} = G_{xyz}[3] + 2 Q_{v}[5]
\end{align*}
\end{quote}
\newpage
\begin{center}\LARGE --- axial tensors ---\end{center}
\begin{align*}
C^{(1,G)} = \begin{pmatrix} C^{(1,G)}_{x} & C^{(1,G)}_{y} & C^{(1,G)}_{z} \end{pmatrix}
\end{align*}
\begin{quote}
\begin{align*}
& C^{(1,G)}_{x} = G_{x} \\
& C^{(1,G)}_{y} = G_{y} \\
& C^{(1,G)}_{z} = G_{z}
\end{align*}
\end{quote}
\begin{align*}
S^{(3,G)} = \begin{pmatrix} S^{(3,G)}_{1x} & S^{(3,G)}_{1y} & S^{(3,G)}_{1z} \\ S^{(3,G)}_{2x} & S^{(3,G)}_{2y} & S^{(3,G)}_{2z} \\ S^{(3,G)}_{3x} & S^{(3,G)}_{3y} & S^{(3,G)}_{3z} \\ S^{(3,G)}_{4x} & S^{(3,G)}_{4y} & S^{(3,G)}_{4z} \\ S^{(3,G)}_{5x} & S^{(3,G)}_{5y} & S^{(3,G)}_{5z} \\ S^{(3,G)}_{6x} & S^{(3,G)}_{6y} & S^{(3,G)}_{6z} \end{pmatrix}
\end{align*}
\begin{quote}
\begin{align*}
& S^{(3,G)}_{1x} = 2 G_{x}[1] + G_{x}[2] + 2 G_{x}^{\alpha} \\
& S^{(3,G)}_{1y} = G_{y}[2] - G_{y}^{\alpha} - G_{y}^{\beta} + 2 Q_{zx}[1] \\
& S^{(3,G)}_{1z} = G_{z}[2] - G_{z}^{\alpha} + G_{z}^{\beta} - 2 Q_{xy}[1] \\
& S^{(3,G)}_{2x} = G_{x}[2] - G_{x}^{\alpha} + G_{x}^{\beta} - 2 Q_{yz}[1] \\
& S^{(3,G)}_{2y} = 2 G_{y}[1] + G_{y}[2] + 2 G_{y}^{\alpha} \\
& S^{(3,G)}_{2z} = G_{z}[2] - G_{z}^{\alpha} - G_{z}^{\beta} + 2 Q_{xy}[1] \\
& S^{(3,G)}_{3x} = G_{x}[2] - G_{x}^{\alpha} - G_{x}^{\beta} + 2 Q_{yz}[1] \\
& S^{(3,G)}_{3y} = G_{y}[2] - G_{y}^{\alpha} + G_{y}^{\beta} - 2 Q_{zx}[1] \\
& S^{(3,G)}_{3z} = 2 G_{z}[1] + G_{z}[2] + 2 G_{z}^{\alpha} \\
& S^{(3,G)}_{4x} = G_{xyz} - 3 Q_{u}[1] - Q_{v}[1] \\
& S^{(3,G)}_{4y} = G_{z}[1] - G_{z}^{\alpha} - G_{z}^{\beta} - Q_{xy}[1] \\
& S^{(3,G)}_{4z} = G_{y}[1] - G_{y}^{\alpha} + G_{y}^{\beta} + Q_{zx}[1] \\
& S^{(3,G)}_{5x} = G_{z}[1] - G_{z}^{\alpha} + G_{z}^{\beta} + Q_{xy}[1] \\
& S^{(3,G)}_{5y} = G_{xyz} + 3 Q_{u}[1] - Q_{v}[1] \\
& S^{(3,G)}_{5z} = G_{x}[1] - G_{x}^{\alpha} - G_{x}^{\beta} - Q_{yz}[1] \\
& S^{(3,G)}_{6x} = G_{y}[1] - G_{y}^{\alpha} - G_{y}^{\beta} - Q_{zx}[1] \\
& S^{(3,G)}_{6y} = G_{x}[1] - G_{x}^{\alpha} + G_{x}^{\beta} + Q_{yz}[1] \\
& S^{(3,G)}_{6z} = G_{xyz} + 2 Q_{v}[1]
\end{align*}
\end{quote}
\begin{align*}
A^{(3,G)} = \begin{pmatrix} A^{(3,G)}_{4x} & A^{(3,G)}_{4y} & A^{(3,G)}_{4z} \\ A^{(3,G)}_{5x} & A^{(3,G)}_{5y} & A^{(3,G)}_{5z} \\ A^{(3,G)}_{6x} & A^{(3,G)}_{6y} & A^{(3,G)}_{6z} \end{pmatrix}
\end{align*}
\begin{quote}
\begin{align*}
& A^{(3,G)}_{4x} = Q_{0} - Q_{u}[2] + Q_{v}[2] \\
& A^{(3,G)}_{4y} = G_{z}[3] + Q_{xy}[2] \\
& A^{(3,G)}_{4z} = - G_{y}[3] + Q_{zx}[2] \\
& A^{(3,G)}_{5x} = - G_{z}[3] + Q_{xy}[2] \\
& A^{(3,G)}_{5y} = Q_{0} - Q_{u}[2] - Q_{v}[2] \\
& A^{(3,G)}_{5z} = G_{x}[3] + Q_{yz}[2] \\
& A^{(3,G)}_{6x} = G_{y}[3] + Q_{zx}[2] \\
& A^{(3,G)}_{6y} = - G_{x}[3] + Q_{yz}[2] \\
& A^{(3,G)}_{6z} = Q_{0} + 2 Q_{u}[2]
\end{align*}
\end{quote}

\end{document}
