\documentclass[fleqn,10pt]{jsarticle}

%%% package

\usepackage[usenames]{color}
\usepackage{amsmath}
\usepackage{breqn}
\usepackage{graphicx}
\usepackage{amssymb}
\usepackage{bm}
\usepackage{enumerate}
\usepackage{braket}
\usepackage{multirow}
\usepackage{booktabs}
\usepackage{longtable}

%%% layout setting

\paperwidth=210truemm
\paperheight=297truemm
\textwidth=169.2truemm
\textheight=249.2truemm
\oddsidemargin=-5truemm
\topmargin=-5truemm
\footskip=7truemm

%%% fixed

\hoffset=0truemm
\voffset=0truemm
\headheight=0truemm
\headsep=0truemm
\marginparsep=0truemm
\marginparwidth=0truemm

%%% main text

\begin{document}

\setcounter{MaxMatrixCols}{16}

\begin{center}
\LARGE
Response Tensors up to 4th rank in $D_{6}$
\end{center}
\begin{center}\LARGE --- polar tensors ---\end{center}
\begin{align*}
C^{(0,Q)} = \begin{pmatrix} C^{(0,Q)} \end{pmatrix}
\end{align*}
\begin{quote}
\begin{align*}
& C^{(0,Q)} = Q_{0}
\end{align*}
\end{quote}
\begin{align*}
S^{(2,Q)} = \begin{pmatrix} S^{(2,Q)}_{xx} & 0 & 0 \\ 0 & S^{(2,Q)}_{xx} & 0 \\ 0 & 0 & S^{(2,Q)}_{zz} \end{pmatrix}
\end{align*}
\begin{quote}
\begin{align*}
& S^{(2,Q)}_{xx} = Q_{0} - Q_{u} \\
& S^{(2,Q)}_{zz} = Q_{0} + 2 Q_{u}
\end{align*}
\end{quote}
\begin{align*}
S^{(3,Q)} = \begin{pmatrix} 0 & 0 & 0 \\ 0 & 0 & 0 \\ 0 & 0 & 0 \\ S^{(3,Q)}_{4x} & 0 & 0 \\ 0 & - S^{(3,Q)}_{4x} & 0 \\ 0 & 0 & 0 \end{pmatrix}
\end{align*}
\begin{quote}
\begin{align*}
& S^{(3,Q)}_{4x} = - 3 G_{u}[1]
\end{align*}
\end{quote}
\begin{align*}
A^{(3,Q)} = \begin{pmatrix} A^{(3,Q)}_{4x} & 0 & 0 \\ 0 & A^{(3,Q)}_{4x} & 0 \\ 0 & 0 & A^{(3,Q)}_{6z} \end{pmatrix}
\end{align*}
\begin{quote}
\begin{align*}
& A^{(3,Q)}_{4x} = G_{0} - G_{u}[2] \\
& A^{(3,Q)}_{6z} = G_{0} + 2 G_{u}[2]
\end{align*}
\end{quote}
\begin{align*}
S^{(4,Q)} = \begin{pmatrix} S^{(4,Q)}_{11} & S^{(4,Q)}_{12} & S^{(4,Q)}_{13} & 0 & 0 & 0 \\ S^{(4,Q)}_{12} & S^{(4,Q)}_{11} & S^{(4,Q)}_{13} & 0 & 0 & 0 \\ S^{(4,Q)}_{13} & S^{(4,Q)}_{13} & S^{(4,Q)}_{33} & 0 & 0 & 0 \\ 0 & 0 & 0 & S^{(4,Q)}_{44} & 0 & 0 \\ 0 & 0 & 0 & 0 & S^{(4,Q)}_{44} & 0 \\ 0 & 0 & 0 & 0 & 0 & \frac{S^{(4,Q)}_{11}}{2} - \frac{S^{(4,Q)}_{12}}{2} \end{pmatrix}
\end{align*}
\begin{quote}
\begin{align*}
& S^{(4,Q)}_{11} = Q_{0}[1] + 2 Q_{0}[2] + 3 Q_{4} - 2 Q_{u}[1] - 4 Q_{u}[2] \\
& S^{(4,Q)}_{12} = Q_{0}[1] + Q_{4} - 2 Q_{u}[1] \\
& S^{(4,Q)}_{13} = Q_{0}[1] - 4 Q_{4} + Q_{u}[1] \\
& S^{(4,Q)}_{33} = Q_{0}[1] + 2 Q_{0}[2] + 8 Q_{4} + 4 Q_{u}[1] + 8 Q_{u}[2] \\
& S^{(4,Q)}_{44} = Q_{0}[2] - 4 Q_{4} + Q_{u}[2]
\end{align*}
\end{quote}
\begin{align*}
\bar{S}^{(4,Q)} = \begin{pmatrix} 0 & 0 & \bar{S}^{(4,Q)}_{13} & 0 & 0 & 0 \\ 0 & 0 & \bar{S}^{(4,Q)}_{13} & 0 & 0 & 0 \\ - \bar{S}^{(4,Q)}_{13} & - \bar{S}^{(4,Q)}_{13} & 0 & 0 & 0 & 0 \\ 0 & 0 & 0 & 0 & 0 & 0 \\ 0 & 0 & 0 & 0 & 0 & 0 \\ 0 & 0 & 0 & 0 & 0 & 0 \end{pmatrix}
\end{align*}
\begin{quote}
\begin{align*}
& \bar{S}^{(4,Q)}_{13} = 3 Q_{u}[3]
\end{align*}
\end{quote}
\begin{align*}
A^{(4,Q)} = \begin{pmatrix} A^{(4,Q)}_{xx} & 0 & 0 \\ 0 & A^{(4,Q)}_{xx} & 0 \\ 0 & 0 & A^{(4,Q)}_{zz} \end{pmatrix}
\end{align*}
\begin{quote}
\begin{align*}
& A^{(4,Q)}_{xx} = Q_{0}[3] - 2 Q_{u}[6] \\
& A^{(4,Q)}_{zz} = Q_{0}[3] + 4 Q_{u}[6]
\end{align*}
\end{quote}
\begin{align*}
M^{(4,Q)} = \begin{pmatrix} 0 & 0 & 0 \\ 0 & 0 & 0 \\ 0 & 0 & 0 \\ M^{(4,Q)}_{4x} & 0 & 0 \\ 0 & - M^{(4,Q)}_{4x} & 0 \\ 0 & 0 & 0 \end{pmatrix}
\end{align*}
\begin{quote}
\begin{align*}
& M^{(4,Q)}_{4x} = - 3 Q_{u}[4]
\end{align*}
\end{quote}
\begin{align*}
\bar{M}^{(4,Q)} = \begin{pmatrix} 0 & 0 & 0 & \bar{M}^{(4,Q)}_{x4} & 0 & 0 \\ 0 & 0 & 0 & 0 & - \bar{M}^{(4,Q)}_{x4} & 0 \\ 0 & 0 & 0 & 0 & 0 & 0 \end{pmatrix}
\end{align*}
\begin{quote}
\begin{align*}
& \bar{M}^{(4,Q)}_{x4} = - 3 Q_{u}[5]
\end{align*}
\end{quote}
\newpage
\begin{center}\LARGE --- axial tensors ---\end{center}
\begin{align*}
C^{(0,G)} = \begin{pmatrix} C^{(0,G)} \end{pmatrix}
\end{align*}
\begin{quote}
\begin{align*}
& C^{(0,G)} = G_{0}
\end{align*}
\end{quote}
\begin{align*}
S^{(2,G)} = \begin{pmatrix} S^{(2,G)}_{xx} & 0 & 0 \\ 0 & S^{(2,G)}_{xx} & 0 \\ 0 & 0 & S^{(2,G)}_{zz} \end{pmatrix}
\end{align*}
\begin{quote}
\begin{align*}
& S^{(2,G)}_{xx} = G_{0} - G_{u} \\
& S^{(2,G)}_{zz} = G_{0} + 2 G_{u}
\end{align*}
\end{quote}
\begin{align*}
S^{(3,G)} = \begin{pmatrix} 0 & 0 & 0 \\ 0 & 0 & 0 \\ 0 & 0 & 0 \\ S^{(3,G)}_{4x} & 0 & 0 \\ 0 & - S^{(3,G)}_{4x} & 0 \\ 0 & 0 & 0 \end{pmatrix}
\end{align*}
\begin{quote}
\begin{align*}
& S^{(3,G)}_{4x} = - 3 Q_{u}[1]
\end{align*}
\end{quote}
\begin{align*}
A^{(3,G)} = \begin{pmatrix} A^{(3,G)}_{4x} & 0 & 0 \\ 0 & A^{(3,G)}_{4x} & 0 \\ 0 & 0 & A^{(3,G)}_{6z} \end{pmatrix}
\end{align*}
\begin{quote}
\begin{align*}
& A^{(3,G)}_{4x} = Q_{0} - Q_{u}[2] \\
& A^{(3,G)}_{6z} = Q_{0} + 2 Q_{u}[2]
\end{align*}
\end{quote}
\begin{align*}
S^{(4,G)} = \begin{pmatrix} S^{(4,G)}_{11} & S^{(4,G)}_{12} & S^{(4,G)}_{13} & 0 & 0 & 0 \\ S^{(4,G)}_{12} & S^{(4,G)}_{11} & S^{(4,G)}_{13} & 0 & 0 & 0 \\ S^{(4,G)}_{13} & S^{(4,G)}_{13} & S^{(4,G)}_{33} & 0 & 0 & 0 \\ 0 & 0 & 0 & S^{(4,G)}_{44} & 0 & 0 \\ 0 & 0 & 0 & 0 & S^{(4,G)}_{44} & 0 \\ 0 & 0 & 0 & 0 & 0 & \frac{S^{(4,G)}_{11}}{2} - \frac{S^{(4,G)}_{12}}{2} \end{pmatrix}
\end{align*}
\begin{quote}
\begin{align*}
& S^{(4,G)}_{11} = G_{0}[1] + 2 G_{0}[2] + 3 G_{4} - 2 G_{u}[1] - 4 G_{u}[2] \\
& S^{(4,G)}_{12} = G_{0}[1] + G_{4} - 2 G_{u}[1] \\
& S^{(4,G)}_{13} = G_{0}[1] - 4 G_{4} + G_{u}[1] \\
& S^{(4,G)}_{33} = G_{0}[1] + 2 G_{0}[2] + 8 G_{4} + 4 G_{u}[1] + 8 G_{u}[2] \\
& S^{(4,G)}_{44} = G_{0}[2] - 4 G_{4} + G_{u}[2]
\end{align*}
\end{quote}
\begin{align*}
\bar{S}^{(4,G)} = \begin{pmatrix} 0 & 0 & \bar{S}^{(4,G)}_{13} & 0 & 0 & 0 \\ 0 & 0 & \bar{S}^{(4,G)}_{13} & 0 & 0 & 0 \\ - \bar{S}^{(4,G)}_{13} & - \bar{S}^{(4,G)}_{13} & 0 & 0 & 0 & 0 \\ 0 & 0 & 0 & 0 & 0 & 0 \\ 0 & 0 & 0 & 0 & 0 & 0 \\ 0 & 0 & 0 & 0 & 0 & 0 \end{pmatrix}
\end{align*}
\begin{quote}
\begin{align*}
& \bar{S}^{(4,G)}_{13} = 3 G_{u}[3]
\end{align*}
\end{quote}
\begin{align*}
A^{(4,G)} = \begin{pmatrix} A^{(4,G)}_{xx} & 0 & 0 \\ 0 & A^{(4,G)}_{xx} & 0 \\ 0 & 0 & A^{(4,G)}_{zz} \end{pmatrix}
\end{align*}
\begin{quote}
\begin{align*}
& A^{(4,G)}_{xx} = G_{0}[3] - 2 G_{u}[6] \\
& A^{(4,G)}_{zz} = G_{0}[3] + 4 G_{u}[6]
\end{align*}
\end{quote}
\begin{align*}
M^{(4,G)} = \begin{pmatrix} 0 & 0 & 0 \\ 0 & 0 & 0 \\ 0 & 0 & 0 \\ M^{(4,G)}_{4x} & 0 & 0 \\ 0 & - M^{(4,G)}_{4x} & 0 \\ 0 & 0 & 0 \end{pmatrix}
\end{align*}
\begin{quote}
\begin{align*}
& M^{(4,G)}_{4x} = - 3 G_{u}[4]
\end{align*}
\end{quote}
\begin{align*}
\bar{M}^{(4,G)} = \begin{pmatrix} 0 & 0 & 0 & \bar{M}^{(4,G)}_{x4} & 0 & 0 \\ 0 & 0 & 0 & 0 & - \bar{M}^{(4,G)}_{x4} & 0 \\ 0 & 0 & 0 & 0 & 0 & 0 \end{pmatrix}
\end{align*}
\begin{quote}
\begin{align*}
& \bar{M}^{(4,G)}_{x4} = - 3 G_{u}[5]
\end{align*}
\end{quote}

\end{document}
