\documentclass[fleqn,8pt,landscape]{jsarticle}
\special{papersize=\the\paperwidth,\the\paperheight}

%%% package

\usepackage[usenames]{color}
\usepackage{amsmath}
\usepackage{breqn}
\usepackage{graphicx}
\usepackage{amssymb}
\usepackage{bm}
\usepackage{enumitem}
\usepackage{braket}
\usepackage{multirow}
\usepackage{booktabs}
\usepackage{longtable}

%%% layout setting

\paperwidth=356.4truemm
\paperheight=252.0truemm
\textwidth=335.59999999999997truemm
\textheight=224.2truemm
\oddsidemargin=-15truemm
\topmargin=-15truemm
\footskip=7truemm

%%% fixed

\hoffset=0truemm
\voffset=0truemm
\headheight=0truemm
\headsep=0truemm
\marginparsep=0truemm
\marginparwidth=0truemm

%%% main text

\begin{document}

\setcounter{MaxMatrixCols}{32}

\renewcommand{\tablename}{Table~}
\renewcommand{\figurename}{Figure~}
\begin{center}
\LARGE
MPG No. 15.9.137\quad$4'/m'm'm$\quad(4'/m'mm' setting)\quad[ Type III, tetragonal ] [M tensor]
\end{center}
* Rank 0 tensor.
* Rank 1 tensor.
* Rank 2 tensor (s).
\begin{align*}
\begin{bmatrix} 0 & M_{xy} & 0 \\ M_{xy} & 0 & 0 \\ 0 & 0 & 0 \end{bmatrix}
\end{align*}
\begin{align*}
& M_{xy} = M_{dxy}^{(1)}
\end{align*}
* Rank 2 tensor (a).
* Rank 3 tensor (s).
* Rank 3 tensor (a).
* Rank 4 tensor (sss).
\begin{align*}
\begin{bmatrix} 0 & 0 & 0 & 0 & 0 & M_{xxxy} \\ 0 & 0 & 0 & 0 & 0 & M_{xxxy} \\ 0 & 0 & 0 & 0 & 0 & M_{zzxy} \\ 0 & 0 & 0 & 0 & M_{yzzx} & 0 \\ 0 & 0 & 0 & M_{yzzx} & 0 & 0 \\ M_{xxxy} & M_{xxxy} & M_{zzxy} & 0 & 0 & 0 \end{bmatrix}
\end{align*}
\begin{align*}
& M_{xxxy} = M_{dxy}^{(1)} + 2 M_{dxy}^{(2)} - M_{gbz}^{(1)} \\
& M_{zzxy} = M_{dxy}^{(1)} + 2 M_{gbz}^{(1)} \\
& M_{yzzx} = M_{dxy}^{(2)} + 2 M_{gbz}^{(1)}
\end{align*}
* Rank 4 tensor (ssa).
\begin{align*}
\begin{bmatrix} 0 & 0 & 0 & 0 & 0 & M_{xxxy} \\ 0 & 0 & 0 & 0 & 0 & M_{xxxy} \\ 0 & 0 & 0 & 0 & 0 & M_{zzxy} \\ 0 & 0 & 0 & 0 & 0 & 0 \\ 0 & 0 & 0 & 0 & 0 & 0 \\ - M_{xxxy} & - M_{xxxy} & - M_{zzxy} & 0 & 0 & 0 \end{bmatrix}
\end{align*}
\begin{align*}
& M_{xxxy} = M_{dxy}^{(3)} + 2 T_{fbz}^{(1)} \\
& M_{zzxy} = M_{dxy}^{(3)} - 4 T_{fbz}^{(1)}
\end{align*}
* Rank 4 tensor (aas).
\begin{align*}
\begin{bmatrix} 0 & M_{yzzx} & 0 \\ M_{yzzx} & 0 & 0 \\ 0 & 0 & 0 \end{bmatrix}
\end{align*}
\begin{align*}
& M_{yzzx} = 2 M_{dxy}^{(4)}
\end{align*}
* Rank 4 tensor (aaa).
* Rank 4 tensor (sa).
\begin{align*}
\begin{bmatrix} 0 & 0 & M_{xxxy} \\ 0 & 0 & - M_{xxxy} \\ 0 & 0 & 0 \\ 0 & M_{yzzx} & 0 \\ - M_{yzzx} & 0 & 0 \\ 0 & 0 & 0 \end{bmatrix}
\end{align*}
\begin{align*}
& M_{xxxy} = - 2 M_{dxy}^{(5)} + T_{fbz}^{(2)} \\
& M_{yzzx} = - M_{dxy}^{(5)} - T_{fbz}^{(2)}
\end{align*}
* Rank 4 tensor (as).
\begin{align*}
\begin{bmatrix} 0 & 0 & 0 & 0 & M_{yzzx} & 0 \\ 0 & 0 & 0 & - M_{yzzx} & 0 & 0 \\ M_{xyxx} & - M_{xyxx} & 0 & 0 & 0 & 0 \end{bmatrix}
\end{align*}
\begin{align*}
& M_{yzzx} = M_{dxy}^{(6)} + T_{fbz}^{(3)} \\
& M_{xyxx} = - 2 M_{dxy}^{(6)} + T_{fbz}^{(3)}
\end{align*}
* Rank 4 tensor (s).
\begin{align*}
\begin{bmatrix} 0 & 0 & 0 & 0 & 0 & M_{xxxy} & 0 & 0 & M_{xxyx} \\ 0 & 0 & 0 & 0 & 0 & M_{xxyx} & 0 & 0 & M_{xxxy} \\ 0 & 0 & 0 & 0 & 0 & M_{zzxy} & 0 & 0 & M_{zzxy} \\ 0 & 0 & 0 & 0 & M_{yzzx} & 0 & 0 & M_{yzxz} & 0 \\ 0 & 0 & 0 & M_{yzxz} & 0 & 0 & M_{yzzx} & 0 & 0 \\ M_{xyxx} & M_{xyxx} & M_{xyzz} & 0 & 0 & 0 & 0 & 0 & 0 \end{bmatrix}
\end{align*}
\begin{align*}
& M_{xxxy} = M_{dxy}^{(1)} + 2 M_{dxy}^{(2)} + M_{dxy}^{(3)} - 2 M_{dxy}^{(5)} - M_{gbz}^{(1)} + 2 T_{fbz}^{(1)} + T_{fbz}^{(2)} \\
& M_{xxyx} = M_{dxy}^{(1)} + 2 M_{dxy}^{(2)} + M_{dxy}^{(3)} + 2 M_{dxy}^{(5)} - M_{gbz}^{(1)} + 2 T_{fbz}^{(1)} - T_{fbz}^{(2)} \\
& M_{zzxy} = M_{dxy}^{(1)} + M_{dxy}^{(3)} + 2 M_{gbz}^{(1)} - 4 T_{fbz}^{(1)} \\
& M_{yzzx} = M_{dxy}^{(2)} - M_{dxy}^{(5)} + 2 M_{gbz}^{(1)} - T_{fbz}^{(2)} \\
& M_{yzxz} = M_{dxy}^{(2)} + M_{dxy}^{(5)} + 2 M_{gbz}^{(1)} + T_{fbz}^{(2)} \\
& M_{xyxx} = M_{dxy}^{(1)} + 2 M_{dxy}^{(2)} - M_{dxy}^{(3)} - M_{gbz}^{(1)} - 2 T_{fbz}^{(1)} \\
& M_{xyzz} = M_{dxy}^{(1)} - M_{dxy}^{(3)} + 2 M_{gbz}^{(1)} + 4 T_{fbz}^{(1)}
\end{align*}
* Rank 4 tensor (a).
\begin{align*}
\begin{bmatrix} 0 & 0 & 0 & 0 & M_{yzzx} & 0 & 0 & M_{yzxz} & 0 \\ 0 & 0 & 0 & - M_{yzxz} & 0 & 0 & - M_{yzzx} & 0 & 0 \\ M_{xyxx} & - M_{xyxx} & 0 & 0 & 0 & 0 & 0 & 0 & 0 \end{bmatrix}
\end{align*}
\begin{align*}
& M_{yzzx} = 2 M_{dxy}^{(4)} + M_{dxy}^{(6)} + T_{fbz}^{(3)} \\
& M_{yzxz} = - 2 M_{dxy}^{(4)} + M_{dxy}^{(6)} + T_{fbz}^{(3)} \\
& M_{xyxx} = - 2 M_{dxy}^{(6)} + T_{fbz}^{(3)}
\end{align*}
* Rank 4 tensor (t).
\begin{align*}
\begin{bmatrix} 0 & M_{xxxy} & 0 \\ M_{xxxy} & 0 & 0 \\ 0 & 0 & 0 \\ 0 & 0 & 0 \\ 0 & M_{zzxy} & 0 \\ M_{xxyx} & 0 & 0 \\ M_{yzzx} & 0 & 0 \\ 0 & 0 & 0 \\ 0 & M_{xyyy} & 0 \\ 0 & 0 & - \frac{M_{xxxy}}{2} - \frac{M_{xxyx}}{2} + M_{xyyy} + M_{zzxy} \end{bmatrix}
\end{align*}
\begin{align*}
& M_{xxxy} = M_{dxy}^{(1)} + 2 M_{dxy}^{(2)} + M_{dxy}^{(3)} - 2 M_{dxy}^{(5)} - M_{gbz}^{(1)} \\
& M_{zzxy} = M_{dxy}^{(1)} + M_{dxy}^{(3)} + 2 M_{gbz}^{(1)} \\
& M_{xxyx} = M_{dxy}^{(1)} + 2 M_{dxy}^{(2)} + M_{dxy}^{(3)} + 2 M_{dxy}^{(5)} - M_{gbz}^{(1)} \\
& M_{yzzx} = M_{dxy}^{(2)} - M_{dxy}^{(5)} + 2 M_{gbz}^{(1)} \\
& M_{xyyy} = M_{dxy}^{(1)} + 2 M_{dxy}^{(2)} - M_{dxy}^{(3)} - M_{gbz}^{(1)}
\end{align*}

\end{document}
